VHDL_Hoare_Typed.thy
@@ -50,7 +50,7 @@ function eval_world_raw :: "nat \<Rightarrow> 'signal worldline_init \<Rightarro
 | "eval_world_raw t w (Bsig sig)          = snd w sig t"
 | "eval_world_raw t w (Btrue)             = Bv True"
 | "eval_world_raw t w (Bfalse)            = Bv False"               
-| "eval_world_raw t w (Bsig_delayed sig dly) = snd w sig (t - dly)"
+| "eval_world_raw t w (Bsig_delayed sig dly) = (if t - dly < t then snd w sig (t - dly) else if 0 < t then snd w sig (t - 1) else fst w sig)"
 | "eval_world_raw t w (Bsig_event sig)    = Bv (sig \<in> event_of (t, w))"
 | "eval_world_raw t w (Bnot e)            = (case eval_world_raw t w e of 
                                                     Bv bool   \<Rightarrow> Bv (\<not> bool)
@@ -64,7 +64,8 @@ function eval_world_raw :: "nat \<Rightarrow> 'signal worldline_init \<Rightarro
 
 
 | "eval_world_raw t w (Bshiftl e n)       = (case eval_world_raw t w e of 
-                                                    Lv ki bs  \<Rightarrow> Lv ki (drop n (bs @ replicate n False)))"
+                                                    Lv Uns bs  \<Rightarrow> Lv Uns (drop n (bs @ replicate n False))
+                                                  | Lv Sig bs  \<Rightarrow> Lv Sig (drop n (bs @ replicate n False)))"
 
 | "eval_world_raw t w (Bshiftr e n)       = (case eval_world_raw t w e of 
                                                     Lv Uns bs \<Rightarrow> Lv Uns (take (length bs) (replicate n False   @ bs))
@@ -145,7 +146,7 @@ next
   show ?case 
     apply (rule bexp_wt_cases_del[OF 13(1)])
     using 13 unfolding wityping_def wtyping_def 
-    by (metis eval_world_raw.simps(13) ty.distinct(1) type_of.elims)
+    by (metis eval_world_raw.simps(13) styping_def ty.distinct(1) type_of.elims)
 next
   case (14 t w sig)
   show ?case  by auto
@@ -201,7 +202,33 @@ lemma bexp_wt_sub:
   assumes "bexp_wt \<Gamma> (Bsub e1 e2) (Lty ki len)"
   shows   "\<exists>len1 len2. bexp_wt \<Gamma> e1 (Lty ki len1) \<and> bexp_wt \<Gamma> e2 (Lty ki len2) \<and> len = max len1 len2 \<and> (ki = Uns \<or> ki = Sig)"
   by (rule bexp_wt_cases_sub[OF assms]) blast+
-  
+
+lemma card_slice:
+  assumes "l < len" and "r \<le> l"
+  shows "card {i. i < len \<and> i \<in> {len - Suc l..len - Suc r}} = Suc (l - r)" (is "card ?lhs = _")
+  using assms
+proof -
+  have "\<forall>i \<in> {len - Suc l .. len - Suc r}. i < len"
+  proof (rule)
+    fix i
+    assume "i \<in> {len - Suc l .. len - Suc r}"
+    hence "len - Suc l \<le> i" and "i \<le> len - Suc r"
+      by auto
+    thus "i < len"
+      using assms by linarith
+  qed
+  hence "{len - Suc l .. len - Suc r} \<subseteq> {i. i < len}"
+    by auto
+  have "?lhs = ({len - Suc l .. len - Suc r})"
+    using assms by auto
+  hence "card ?lhs = card {len - Suc l .. len - Suc r}"
+    by auto
+  also have "... = Suc (l - r)"
+    unfolding card_atLeastAtMost using assms by auto
+  finally show ?thesis
+    by auto
+qed
+
 lemma eval_world_raw_lv: 
   assumes "bexp_wt \<Gamma> exp (Lty ki len)" and "wityping \<Gamma> w"
   shows   "\<exists>bs. eval_world_raw t w exp = Lv ki bs \<and> length bs = len"
@@ -281,7 +308,7 @@ next
   show ?case 
     apply (rule bexp_wt_cases_del[OF 13(1)])
     using 13 unfolding wityping_def wtyping_def 
-    by (metis (no_types, hide_lams) eval_world_raw.simps(13) ty.distinct(1) ty.inject type_of.elims)
+    by (smt eval_world_raw.simps(13) styping_def ty.distinct(1) ty.inject type_of.elims)
 next
   case (14 t w sig)
   show ?case  
@@ -296,36 +323,39 @@ next
   case (16 t w sig l r)
   show ?case 
     apply (rule bexp_wt_cases(8)[OF 16(2)])
-    using 16 sorry
+    using 16 
+    apply (auto split:val.split)
+    unfolding length_nths using card_slice by auto
 next
   case (17 t w sig idx)
-  then show ?case bexp_wt_cases(8)
-    (* by (metis (no_types, lifting) bexp_wt_cases(10) bexp_wt_cases(9) eval_world_raw.simps(10) eval_world_raw.simps(17) is_Bv_def ty.simps(3) type_of.simps(1) val.case_eq_if wityping_def wtyping_def) *)
+  then show ?case
+    using bexp_wt_cases(10) by fastforce
 next
   case (18 t w e n)
-  then show ?case 
-    (* by (meson bexp_wt_cases(14) ty.distinct(1)) *)
+  show ?case 
+    apply (rule bexp_wt_cases(14)[OF 18(2)])
+     apply (auto split:val.split)
+    using 18 by auto
 next
   case (19 t w e n)
-  then show ?case 
-    (* by (meson bexp_wt_cases(15) ty.distinct(1)) *)
+  show ?case 
+    apply (rule bexp_wt_cases(15)[OF 19(2)])
+     apply (auto split:val.split)
+    using 19 by auto
 next
   case (20 t w th guard el)
   hence *: "\<exists>v. eval_world_raw t w guard = Bv v"
-    using bexp_wt_cases_when by blast
+    using bexp_wt_cases_when  by (metis eval_world_raw_bv)
   show ?case 
     apply (rule bexp_wt_cases_when[OF 20(4)])
     using * 20  by (smt eval_world_raw.simps(20) val.simps(5))
 next
   case (21 t w sign val)
   then show ?case 
-    using bexp_wt_cases_lit 
-    (* by blast *)
+    using bexp_wt_cases_lit  by fastforce
 qed  
 
-
-
-lemma
+lemma eval_world_raw_correctness_if:
   assumes "eval_world_raw t w exp = res" 
   assumes "wityping \<Gamma> w" and  "bexp_wt \<Gamma> exp ty"
   shows   "beval_world_raw w t exp res"
@@ -351,74 +381,1792 @@ proof (induct arbitrary: res ty rule: eval_world_raw.induct)
     case vector
     hence "bexp_wt \<Gamma> e1 (Lty ki len)" and "bexp_wt \<Gamma> e2 (Lty ki len)"
       using 1(5) bexp_wt.cases by auto
-    then obtain res1 res2 where "eval_world_raw t w e1 = Lv ki res1" and "eval_world_raw t w e2 = Lv ki res2"
-      using eval_world_raw_
-    then show ?thesis sorry
+    then obtain res1 res2 where "eval_world_raw t w e1 = Lv ki res1" and "length res1 = len" 
+                            and "eval_world_raw t w e2 = Lv ki res2" and "length res2 = len"
+      using eval_world_raw_lv using "1.prems"(2) by blast
+    hence " beval_world_raw w t e1 (Lv ki res1) \<and>  beval_world_raw w t e2 (Lv ki res2)"
+      using "1.hyps"(1) "1.prems"(2) \<open>bexp_wt \<Gamma> e1 (Lty ki len)\<close> "1.hyps"(2) \<open>bexp_wt \<Gamma> e2 (Lty ki len)\<close> 
+      by blast
+    moreover have "res = Lv ki (map2 (\<and>) res1 res2)"
+      using 1(3) `eval_world_raw t w e1 = Lv ki res1` `eval_world_raw t w e2 = Lv ki res2` 
+      by auto
+    ultimately show ?thesis 
+      by (metis \<open>length res1 = len\<close> \<open>length res2 = len\<close> beval_raw.intros(9) beval_world_raw.cases
+      beval_world_raw.intros)  
   qed
 next
   case (2 t w e1 e2)
-  then show ?case sorry
+  then consider (bool) "ty = Bty" | (vector) ki len where "ty = Lty ki len"
+    by (meson ty.exhaust)
+  then show ?case 
+  proof (cases)
+    case bool
+    hence "bexp_wt \<Gamma> e1 Bty" and "bexp_wt \<Gamma> e2 Bty"
+      using 2(5) bexp_wt.cases by auto
+    then obtain res1 res2 where "eval_world_raw t w e1 = Bv res1" and "eval_world_raw t w e2 = Bv res2"
+      using eval_world_raw_bv  using "2.prems"(2) by blast
+    hence " beval_world_raw w t e1 (Bv res1)" and " beval_world_raw w t e2 (Bv res2)"
+      using "2.hyps" "2.prems" \<open>bexp_wt \<Gamma> e1 Bty\<close> \<open>bexp_wt \<Gamma> e2 Bty\<close> by blast+
+    moreover have "res = Bv (res1 \<or> res2)"
+      using "2.prems"(1) \<open>eval_world_raw t w e1 = Bv res1\<close> \<open>eval_world_raw t w e2 = Bv res2\<close> by auto
+    ultimately show ?thesis 
+      by (meson beval_raw.intros(10) beval_world_raw.cases beval_world_raw.intros)
+  next
+    case vector
+    hence "bexp_wt \<Gamma> e1 (Lty ki len)" and "bexp_wt \<Gamma> e2 (Lty ki len)"
+      using 2(5) bexp_wt.cases by auto
+    then obtain res1 res2 where "eval_world_raw t w e1 = Lv ki res1" and "length res1 = len" 
+                            and "eval_world_raw t w e2 = Lv ki res2" and "length res2 = len"
+      using eval_world_raw_lv using "2.prems"(2) by blast
+    hence " beval_world_raw w t e1 (Lv ki res1) \<and>  beval_world_raw w t e2 (Lv ki res2)"
+      using "2.hyps"(1) "2.prems"(2) \<open>bexp_wt \<Gamma> e1 (Lty ki len)\<close> "2.hyps"(2) \<open>bexp_wt \<Gamma> e2 (Lty ki len)\<close> 
+      by blast
+    moreover have "res = Lv ki (map2 (\<or>) res1 res2)"
+      using 2(3) `eval_world_raw t w e1 = Lv ki res1` `eval_world_raw t w e2 = Lv ki res2` 
+      by auto
+    ultimately show ?thesis 
+      by (metis \<open>length res1 = len\<close> \<open>length res2 = len\<close> beval_raw.intros(11) beval_world_raw.cases beval_world_raw.intros) 
+  qed
 next
   case (3 t w e1 e2)
-  then show ?case sorry
+  then consider (bool) "ty = Bty" | (vector) ki len where "ty = Lty ki len"
+    by (meson ty.exhaust)
+  then show ?case 
+  proof (cases)
+    case bool
+    hence "bexp_wt \<Gamma> e1 Bty" and "bexp_wt \<Gamma> e2 Bty"
+      using 3(5) bexp_wt.cases by auto
+    then obtain res1 res2 where "eval_world_raw t w e1 = Bv res1" and "eval_world_raw t w e2 = Bv res2"
+      using eval_world_raw_bv  using "3.prems"(2) by blast
+    hence " beval_world_raw w t e1 (Bv res1)" and " beval_world_raw w t e2 (Bv res2)"
+      using "3.hyps" "3.prems" \<open>bexp_wt \<Gamma> e1 Bty\<close> \<open>bexp_wt \<Gamma> e2 Bty\<close> by blast+
+    moreover have "res = Bv (\<not> (res1 \<and> res2))"
+      using "3.prems"(1) \<open>eval_world_raw t w e1 = Bv res1\<close> \<open>eval_world_raw t w e2 = Bv res2\<close> by auto
+    ultimately show ?thesis 
+      by (meson beval_raw.intros(12) beval_world_raw.cases beval_world_raw.intros)
+  next
+    case vector
+    hence "bexp_wt \<Gamma> e1 (Lty ki len)" and "bexp_wt \<Gamma> e2 (Lty ki len)"
+      using 3(5) bexp_wt.cases by auto
+    then obtain res1 res2 where "eval_world_raw t w e1 = Lv ki res1" and "length res1 = len" 
+                            and "eval_world_raw t w e2 = Lv ki res2" and "length res2 = len"
+      using eval_world_raw_lv using "3.prems"(2) by blast
+    hence " beval_world_raw w t e1 (Lv ki res1) \<and>  beval_world_raw w t e2 (Lv ki res2)"
+      using "3.hyps"(1) "3.prems"(2) \<open>bexp_wt \<Gamma> e1 (Lty ki len)\<close> "3.hyps"(2) \<open>bexp_wt \<Gamma> e2 (Lty ki len)\<close> 
+      by blast
+    moreover have "res = Lv ki (map2 (\<lambda>x y. \<not> (x \<and> y)) res1 res2)"
+      using 3(3) `eval_world_raw t w e1 = Lv ki res1` `eval_world_raw t w e2 = Lv ki res2` 
+      by auto
+    ultimately show ?thesis 
+      by (metis \<open>length res1 = len\<close> \<open>length res2 = len\<close> beval_raw.intros(13) beval_world_raw.cases beval_world_raw.intros)
+  qed
 next
   case (4 t w e1 e2)
-  then show ?case sorry
+  then consider (bool) "ty = Bty" | (vector) ki len where "ty = Lty ki len"
+    by (meson ty.exhaust)
+  then show ?case 
+  proof (cases)
+    case bool
+    hence "bexp_wt \<Gamma> e1 Bty" and "bexp_wt \<Gamma> e2 Bty"
+      using 4(5) bexp_wt.cases by auto
+    then obtain res1 res2 where "eval_world_raw t w e1 = Bv res1" and "eval_world_raw t w e2 = Bv res2"
+      using eval_world_raw_bv  using "4.prems"(2) by blast
+    hence " beval_world_raw w t e1 (Bv res1)" and " beval_world_raw w t e2 (Bv res2)"
+      using "4.hyps" "4.prems" \<open>bexp_wt \<Gamma> e1 Bty\<close> \<open>bexp_wt \<Gamma> e2 Bty\<close> by blast+
+    moreover have "res = Bv (\<not> (res1 \<or> res2))"
+      using "4.prems"(1) \<open>eval_world_raw t w e1 = Bv res1\<close> \<open>eval_world_raw t w e2 = Bv res2\<close> by auto
+    ultimately show ?thesis 
+      by (meson beval_raw.intros(14) beval_world_raw.cases beval_world_raw.intros)
+  next
+    case vector
+    hence "bexp_wt \<Gamma> e1 (Lty ki len)" and "bexp_wt \<Gamma> e2 (Lty ki len)"
+      using 4(5) bexp_wt.cases by auto
+    then obtain res1 res2 where "eval_world_raw t w e1 = Lv ki res1" and "length res1 = len" 
+                            and "eval_world_raw t w e2 = Lv ki res2" and "length res2 = len"
+      using eval_world_raw_lv using "4.prems"(2) by blast
+    hence " beval_world_raw w t e1 (Lv ki res1) \<and>  beval_world_raw w t e2 (Lv ki res2)"
+      using "4.hyps"(1) "4.prems"(2) \<open>bexp_wt \<Gamma> e1 (Lty ki len)\<close> "4.hyps"(2) \<open>bexp_wt \<Gamma> e2 (Lty ki len)\<close> 
+      by blast
+    moreover have "res = Lv ki (map2 (\<lambda>x y. \<not> (x \<or> y)) res1 res2)"
+      using 4(3) `eval_world_raw t w e1 = Lv ki res1` `eval_world_raw t w e2 = Lv ki res2` 
+      by auto
+    ultimately show ?thesis
+      by (metis \<open>length res1 = len\<close> \<open>length res2 = len\<close> beval_raw.intros(15) beval_world_raw.cases beval_world_raw.intros)
+  qed
 next
   case (5 t w e1 e2)
-  then show ?case sorry
+  then consider (bool) "ty = Bty" | (vector) ki len where "ty = Lty ki len"
+    by (meson ty.exhaust)
+  then show ?case 
+  proof (cases)
+    case bool
+    hence "bexp_wt \<Gamma> e1 Bty" and "bexp_wt \<Gamma> e2 Bty"
+      using 5(5) bexp_wt.cases by auto
+    then obtain res1 res2 where "eval_world_raw t w e1 = Bv res1" and "eval_world_raw t w e2 = Bv res2"
+      using eval_world_raw_bv  using "5.prems"(2) by blast
+    hence " beval_world_raw w t e1 (Bv res1)" and " beval_world_raw w t e2 (Bv res2)"
+      using "5.hyps" "5.prems" \<open>bexp_wt \<Gamma> e1 Bty\<close> \<open>bexp_wt \<Gamma> e2 Bty\<close> by blast+
+    moreover have "res = Bv (xor res1 res2)"
+      using "5.prems"(1) \<open>eval_world_raw t w e1 = Bv res1\<close> \<open>eval_world_raw t w e2 = Bv res2\<close> by auto
+    ultimately show ?thesis 
+      by (meson beval_raw.intros(16) beval_world_raw.cases beval_world_raw.intros)
+  next
+    case vector
+    hence "bexp_wt \<Gamma> e1 (Lty ki len)" and "bexp_wt \<Gamma> e2 (Lty ki len)"
+      using 5(5) bexp_wt.cases by auto
+    then obtain res1 res2 where "eval_world_raw t w e1 = Lv ki res1" and "length res1 = len" 
+                            and "eval_world_raw t w e2 = Lv ki res2" and "length res2 = len"
+      using eval_world_raw_lv using "5.prems"(2) by blast
+    hence " beval_world_raw w t e1 (Lv ki res1) \<and>  beval_world_raw w t e2 (Lv ki res2)"
+      using "5.hyps"(1) "5.prems"(2) \<open>bexp_wt \<Gamma> e1 (Lty ki len)\<close> "5.hyps"(2) \<open>bexp_wt \<Gamma> e2 (Lty ki len)\<close> 
+      by blast
+    moreover have "res = Lv ki (map2 xor res1 res2)"
+      using 5(3) `eval_world_raw t w e1 = Lv ki res1` `eval_world_raw t w e2 = Lv ki res2` 
+      by auto
+    ultimately show ?thesis 
+      by (metis \<open>length res1 = len\<close> \<open>length res2 = len\<close> beval_raw.intros(17) beval_world_raw.cases beval_world_raw.intros)
+  qed
 next
   case (6 t w e1 e2)
-  then show ?case sorry
+  then consider (bool) "ty = Bty" | (vector) ki len where "ty = Lty ki len"
+    by (meson ty.exhaust)
+  then show ?case 
+  proof (cases)
+    case bool
+    hence "bexp_wt \<Gamma> e1 Bty" and "bexp_wt \<Gamma> e2 Bty"
+      using 6(5) bexp_wt.cases by auto
+    then obtain res1 res2 where "eval_world_raw t w e1 = Bv res1" and "eval_world_raw t w e2 = Bv res2"
+      using eval_world_raw_bv  using "6.prems"(2) by blast
+    hence " beval_world_raw w t e1 (Bv res1)" and " beval_world_raw w t e2 (Bv res2)"
+      using "6.hyps" "6.prems" \<open>bexp_wt \<Gamma> e1 Bty\<close> \<open>bexp_wt \<Gamma> e2 Bty\<close> by blast+
+    moreover have "res = Bv (\<not> (xor res1 res2))"
+      using "6.prems"(1) \<open>eval_world_raw t w e1 = Bv res1\<close> \<open>eval_world_raw t w e2 = Bv res2\<close> by auto
+    ultimately show ?thesis 
+      by (meson beval_raw.intros(18) beval_world_raw.cases beval_world_raw.intros)
+  next
+    case vector
+    hence "bexp_wt \<Gamma> e1 (Lty ki len)" and "bexp_wt \<Gamma> e2 (Lty ki len)"
+      using 6(5) bexp_wt.cases by auto
+    then obtain res1 res2 where "eval_world_raw t w e1 = Lv ki res1" and "length res1 = len" 
+                            and "eval_world_raw t w e2 = Lv ki res2" and "length res2 = len"
+      using eval_world_raw_lv using "6.prems"(2) by blast
+    hence " beval_world_raw w t e1 (Lv ki res1) \<and>  beval_world_raw w t e2 (Lv ki res2)"
+      using "6.hyps"(1) "6.prems"(2) \<open>bexp_wt \<Gamma> e1 (Lty ki len)\<close> "6.hyps"(2) \<open>bexp_wt \<Gamma> e2 (Lty ki len)\<close> 
+      by blast
+    moreover have "res = Lv ki (map2 (\<lambda>x y. \<not> xor x y) res1 res2)"
+      using 6(3) `eval_world_raw t w e1 = Lv ki res1` `eval_world_raw t w e2 = Lv ki res2` 
+      by auto
+    ultimately show ?thesis 
+      by (metis \<open>length res1 = len\<close> \<open>length res2 = len\<close> beval_raw.intros(19) beval_world_raw.cases beval_world_raw.intros)
+  qed
 next
   case (7 t w e1 e2)
-  then show ?case sorry
+  obtain res1 res2 where " eval_world_raw t w e1 = res1" and " eval_world_raw t w e2 = res2"
+    by auto
+  obtain ki len1 len2 where "bexp_wt \<Gamma> e1 (Lty ki len1)" and "bexp_wt \<Gamma> e2 (Lty ki len2)" and 
+    "ty = Lty ki (max len1 len2)" using bexp_wt_cases_add[OF ` bexp_wt \<Gamma> (Badd e1 e2) ty`] by metis
+  hence IH1: "beval_world_raw w t e1 res1" and IH2: "beval_world_raw w t e2 res2"
+    using 7(1)[OF `eval_world_raw t w e1 = res1` `wityping \<Gamma> w`]  7(2)[OF `eval_world_raw t w e2 = res2` `wityping \<Gamma> w`]
+    by auto
+  let ?len1 = "length (lval_of res1)"
+  let ?len2 = "length (lval_of res2)"
+  have "?len1 = len1" and "?len2 = len2"
+    using IH1 `bexp_wt \<Gamma> e1 (Lty ki len1)` `bexp_wt \<Gamma> e2 (Lty ki len2)` IH2 
+    by (metis (no_types, lifting) "7.prems"(2) beval_raw_preserve_well_typedness
+    beval_world_raw_cases ty.distinct(1) ty.inject type_of.simps(1) type_of.simps(2) val.exhaust_sel
+    wityping_def wityping_ensure_styping wityping_ensure_ttyping)+    
+
+  consider (Uns) "ki = Uns" | (Sig) "ki = Sig"
+    using `ty = Lty ki (max len1 len2)` "7.prems"(3) bexp_wt_add by blast
+  thus ?case
+  proof (cases)
+    case Uns
+    then obtain bs1 bs2 where "res1 = Lv Uns bs1" and "length bs1 = len1" and "res2 = Lv Uns bs2" and "length bs2 = len2"
+      using "7.prems"(2) \<open>bexp_wt \<Gamma> e1 (Lty ki len1)\<close> \<open>eval_world_raw t w e1 = res1\<close> eval_world_raw_lv 
+      by (metis \<open>bexp_wt \<Gamma> e2 (Lty ki len2)\<close> \<open>eval_world_raw t w e2 = res2\<close>)
+    hence "res = Lv Uns (bin_to_bl (max len1 len2) ((bl_to_bin bs1) + (bl_to_bin bs2)))"
+      using 7(3) `eval_world_raw t w e1 = res1` `eval_world_raw t w e2 = res2` by auto
+    then show ?thesis 
+      using IH1 IH2 `res1 = Lv Uns bs1` `res2 = Lv Uns bs2`
+      by (metis \<open>length bs1 = len1\<close> \<open>length bs2 = len2\<close> beval_raw.intros(22) beval_world_raw.cases beval_world_raw.intros)
+  next
+    case Sig
+    then obtain bs1 bs2 where "res1 = Lv Sig bs1" and "length bs1 = len1" and "res2 = Lv Sig bs2" and "length bs2 = len2"
+      using "7.prems"(2) \<open>bexp_wt \<Gamma> e1 (Lty ki len1)\<close> \<open>eval_world_raw t w e1 = res1\<close> eval_world_raw_lv 
+      by (metis \<open>bexp_wt \<Gamma> e2 (Lty ki len2)\<close> \<open>eval_world_raw t w e2 = res2\<close>)
+    hence "res = Lv Sig (bin_to_bl (max len1 len2) ((sbl_to_bin bs1) + (sbl_to_bin bs2)))"
+      using 7(3) `eval_world_raw t w e1 = res1` `eval_world_raw t w e2 = res2` by auto
+    then show ?thesis 
+      using IH1 IH2 `res1 = Lv Sig bs1` `res2 = Lv Sig bs2`
+      by (metis \<open>length bs1 = len1\<close> \<open>length bs2 = len2\<close> beval_raw.intros(23) beval_world_raw.cases beval_world_raw.intros)
+  qed
 next
-  case (8 t w e1 e2)
-  then show ?case sorry
+  case (8 t w e1 e2)  
+  obtain res1 res2 where " eval_world_raw t w e1 = res1" and " eval_world_raw t w e2 = res2"
+    by auto
+  obtain ki len1 len2 where "bexp_wt \<Gamma> e1 (Lty ki len1)" and "bexp_wt \<Gamma> e2 (Lty ki len2)" and 
+    "ty = Lty ki (len1 + len2)" using bexp_wt_cases_mult[OF ` bexp_wt \<Gamma> (Bmult e1 e2) ty`] by metis
+  hence IH1: "beval_world_raw w t e1 res1" and IH2: "beval_world_raw w t e2 res2"
+    using 8(1)[OF `eval_world_raw t w e1 = res1` `wityping \<Gamma> w`]  8(2)[OF `eval_world_raw t w e2 = res2` `wityping \<Gamma> w`]
+    by auto
+  let ?len1 = "length (lval_of res1)"
+  let ?len2 = "length (lval_of res2)"
+  have "?len1 = len1" and "?len2 = len2"
+    using IH1 `bexp_wt \<Gamma> e1 (Lty ki len1)` `bexp_wt \<Gamma> e2 (Lty ki len2)` IH2 
+    by (metis (no_types, lifting) "8.prems"(2) beval_raw_preserve_well_typedness
+    beval_world_raw_cases ty.distinct(1) ty.inject type_of.simps(1) type_of.simps(2) val.exhaust_sel
+    wityping_def wityping_ensure_styping wityping_ensure_ttyping)+    
+
+  consider (Uns) "ki = Uns" | (Sig) "ki = Sig"
+    using `ty = Lty ki (len1 + len2)` "8.prems"(3) bexp_wt_mult by blast
+  thus ?case
+  proof (cases)
+    case Uns
+    then obtain bs1 bs2 where "res1 = Lv Uns bs1" and "length bs1 = len1" and "res2 = Lv Uns bs2" and "length bs2 = len2"
+      using "8.prems"(2) \<open>bexp_wt \<Gamma> e1 (Lty ki len1)\<close> \<open>eval_world_raw t w e1 = res1\<close> eval_world_raw_lv 
+      by (metis \<open>bexp_wt \<Gamma> e2 (Lty ki len2)\<close> \<open>eval_world_raw t w e2 = res2\<close>)
+    hence "res = Lv Uns (bin_to_bl (len1 + len2) ((bl_to_bin bs1) * (bl_to_bin bs2)))"
+      using 8(3) `eval_world_raw t w e1 = res1` `eval_world_raw t w e2 = res2` by auto
+    then show ?thesis 
+      using IH1 IH2 `res1 = Lv Uns bs1` `res2 = Lv Uns bs2`
+      by (metis \<open>length bs1 = len1\<close> \<open>length bs2 = len2\<close> beval_raw.intros(24) beval_world_raw.cases beval_world_raw.intros)
+  next
+    case Sig
+    then obtain bs1 bs2 where "res1 = Lv Sig bs1" and "length bs1 = len1" and "res2 = Lv Sig bs2" and "length bs2 = len2"
+      using "8.prems"(2) \<open>bexp_wt \<Gamma> e1 (Lty ki len1)\<close> \<open>eval_world_raw t w e1 = res1\<close> eval_world_raw_lv 
+      by (metis \<open>bexp_wt \<Gamma> e2 (Lty ki len2)\<close> \<open>eval_world_raw t w e2 = res2\<close>)
+    hence "res = Lv Sig (bin_to_bl (len1 + len2) ((sbl_to_bin bs1) * (sbl_to_bin bs2)))"
+      using 8(3) `eval_world_raw t w e1 = res1` `eval_world_raw t w e2 = res2` by auto
+    then show ?thesis 
+      using IH1 IH2 `res1 = Lv Sig bs1` `res2 = Lv Sig bs2` 
+      by (metis \<open>length bs1 = len1\<close> \<open>length bs2 = len2\<close> beval_raw.intros(25) beval_world_raw.cases beval_world_raw.intros)
+  qed
 next
   case (9 t w e1 e2)
-  then show ?case sorry
+  obtain res1 res2 where " eval_world_raw t w e1 = res1" and " eval_world_raw t w e2 = res2"
+    by auto
+  obtain ki len1 len2 where "bexp_wt \<Gamma> e1 (Lty ki len1)" and "bexp_wt \<Gamma> e2 (Lty ki len2)" and 
+    "ty = Lty ki (max len1 len2)" using bexp_wt_cases_sub[OF ` bexp_wt \<Gamma> (Bsub e1 e2) ty`] by metis
+  hence IH1: "beval_world_raw w t e1 res1" and IH2: "beval_world_raw w t e2 res2"
+    using 9(1)[OF `eval_world_raw t w e1 = res1` `wityping \<Gamma> w`]  9(2)[OF `eval_world_raw t w e2 = res2` `wityping \<Gamma> w`]
+    by auto
+  let ?len1 = "length (lval_of res1)"
+  let ?len2 = "length (lval_of res2)"
+  have "?len1 = len1" and "?len2 = len2"
+    using IH1 `bexp_wt \<Gamma> e1 (Lty ki len1)` `bexp_wt \<Gamma> e2 (Lty ki len2)` IH2 
+    by (metis (no_types, lifting) "9.prems"(2) beval_raw_preserve_well_typedness
+    beval_world_raw_cases ty.distinct(1) ty.inject type_of.simps(1) type_of.simps(2) val.exhaust_sel
+    wityping_def wityping_ensure_styping wityping_ensure_ttyping)+    
+
+  consider (Uns) "ki = Uns" | (Sig) "ki = Sig"
+    using `ty = Lty ki (max len1 len2)` "9.prems"(3) bexp_wt_sub by blast
+  thus ?case
+  proof (cases)
+    case Uns
+    then obtain bs1 bs2 where "res1 = Lv Uns bs1" and "length bs1 = len1" and "res2 = Lv Uns bs2" and "length bs2 = len2"
+      using "9.prems"(2) \<open>bexp_wt \<Gamma> e1 (Lty ki len1)\<close> \<open>eval_world_raw t w e1 = res1\<close> eval_world_raw_lv 
+      by (metis \<open>bexp_wt \<Gamma> e2 (Lty ki len2)\<close> \<open>eval_world_raw t w e2 = res2\<close>)
+    hence "res = Lv Uns (bin_to_bl (max len1 len2) ((bl_to_bin bs1) - (bl_to_bin bs2)))"
+      using 9(3) `eval_world_raw t w e1 = res1` `eval_world_raw t w e2 = res2` by auto
+    then show ?thesis 
+      using IH1 IH2 `res1 = Lv Uns bs1` `res2 = Lv Uns bs2`
+      by (metis \<open>length bs1 = len1\<close> \<open>length bs2 = len2\<close> beval_raw.intros(26) beval_world_raw.cases beval_world_raw.intros)
+  next
+    case Sig
+    then obtain bs1 bs2 where "res1 = Lv Sig bs1" and "length bs1 = len1" and "res2 = Lv Sig bs2" and "length bs2 = len2"
+      using "9.prems"(2) \<open>bexp_wt \<Gamma> e1 (Lty ki len1)\<close> \<open>eval_world_raw t w e1 = res1\<close> eval_world_raw_lv 
+      by (metis \<open>bexp_wt \<Gamma> e2 (Lty ki len2)\<close> \<open>eval_world_raw t w e2 = res2\<close>)
+    hence "res = Lv Sig (bin_to_bl (max len1 len2) ((sbl_to_bin bs1) - (sbl_to_bin bs2)))"
+      using 9(3) `eval_world_raw t w e1 = res1` `eval_world_raw t w e2 = res2` by auto
+    then show ?thesis 
+      using IH1 IH2 `res1 = Lv Sig bs1` `res2 = Lv Sig bs2`
+      by (metis \<open>length bs1 = len1\<close> \<open>length bs2 = len2\<close> beval_raw.intros(27) beval_world_raw.cases beval_world_raw.intros)
+  qed
 next
   case (10 t w sig)
-  then show ?case sorry
+  then show ?case 
+    by (auto intro!: beval_world_raw.intros beval_raw.intros simp add: state_of_world_def)
 next
-case (11 t w)
-  then show ?case sorry
+  case (11 t w)
+  then show ?case 
+    by (auto intro!: beval_world_raw.intros beval_raw.intros)
 next
   case (12 t w)
-then show ?case sorry
+  then show ?case 
+    by (auto intro!: beval_world_raw.intros beval_raw.intros)
 next
   case (13 t w sig dly)
-  then show ?case sorry
+  have res_def: "res = (if t - dly < t then snd w sig (t - dly) else if 0 < t then snd w sig (t - 1) else fst w sig)"
+    using 13 by auto
+                
+  have "t - dly < t \<or> t - dly = t"
+    by linarith
+  moreover
+  { assume "t - dly < t"
+    hence "signal_of (fst w sig) (derivative_hist_raw w t) sig (t - dly) = snd w sig (t - dly)"
+      using signal_of_derivative_hist_raw  by metis
+    also have "... = res"
+      unfolding res_def using `t - dly < t` by auto
+    finally have "signal_of (fst w sig) (derivative_hist_raw w t) sig (t - dly) = res" 
+      by auto }
+  moreover
+  { assume "t - dly = t"
+    have "0 < t \<or> t = 0" by auto
+    moreover
+    { assume " 0 < t"
+      hence "signal_of (fst w sig) (derivative_hist_raw w t) sig (t - dly) = snd w sig (t - 1)"
+        using `t - dly = t` signal_of_derivative_hist_raw2  by (metis diff_le_self)
+      also have "... = res"
+        unfolding res_def using `t - dly = t` `0 < t` by auto
+      finally have "signal_of (fst w sig) (derivative_hist_raw w t) sig (t - dly) = res" 
+        by auto }
+    moreover
+    { assume "t = 0"
+      hence "signal_of (fst w sig) (derivative_hist_raw w t) sig (t - dly) = fst w sig"
+        using signal_of_derivative_hist_raw3  by (metis \<open>t - dly = t\<close> diff_le_self)
+      also have "... = res"
+        unfolding res_def using `t = 0` by auto
+      finally have "signal_of (fst w sig) (derivative_hist_raw w t) sig (t - dly) = res" 
+        by auto }
+    ultimately have "signal_of (fst w sig) (derivative_hist_raw w t) sig (t - dly) = res" 
+      by auto }
+  ultimately have "signal_of (fst w sig) (derivative_hist_raw w t) sig (t - dly) = res"
+    by auto         
+  thus ?case
+    by (meson beval_raw.intros(4) beval_world_raw.intros)
 next
   case (14 t w sig)
-  then show ?case sorry
+  then show ?case 
+    by (auto intro!: beval_world_raw.intros beval_raw.intros simp add: event_of_world_def event_of_alt_def)
+       (smt beval_raw.intros(5) mem_Collect_eq)+
 next
   case (15 t w e)
-  then show ?case sorry
+  hence "bexp_wt \<Gamma> e ty"
+    using bexp_wt_cases(1) by blast
+  obtain bool ki bs where "eval_world_raw t w e = Bv bool \<or> eval_world_raw t w e = Lv ki bs"
+    using val.exhaust_sel by blast
+  moreover
+  { assume "eval_world_raw t w e = Bv bool"
+    hence " beval_world_raw w t e (Bv bool)"
+      using 15(1) "15.prems"(2) \<open>bexp_wt \<Gamma> e ty\<close> by blast
+    hence " res = Bv (\<not> bool)"
+      using 15(2) `eval_world_raw t w e = Bv bool` by auto
+    hence ?case
+      using `beval_world_raw w t e (Bv bool)` beval_raw.intros(6)
+      by (intro beval_world_raw.intros) blast+ }
+  moreover
+  { assume "eval_world_raw t w e = Lv ki bs"
+    hence  "res = Lv ki (map Not bs)"
+      using 15(2) by auto
+    hence IH : "beval_world_raw w t e (Lv ki bs)"
+      using 15  \<open>bexp_wt \<Gamma> e ty\<close> \<open>eval_world_raw t w e = Lv ki bs\<close> by blast
+    hence ?case
+      using `res = Lv ki (map Not bs)` beval_raw.intros(7)
+      by (intro beval_world_raw.intros) blast+ }
+  ultimately show ?case
+    by auto
 next
   case (16 t w sig l r)
-  then show ?case sorry
+  then obtain ki bs where *: "eval_world_raw t w (Bsig sig) = Lv ki bs"
+    by (meson bexp_wt_cases(8) eval_world_raw_lv)
+  hence IH: "beval_world_raw w t (Bsig sig) (Lv ki bs)"
+    using 16  bexp_wt.intros(3) by fastforce
+  have "res = Lv ki (nths bs {length bs - l - 1..length bs - r - 1})"
+    using * 16 unfolding eval_world_raw.simps by auto
+  then show ?case 
+    using IH beval_raw.intros(20) 
+    by (metis beval_world_raw.cases beval_world_raw.intros)
 next
   case (17 t w sig idx)
-  then show ?case sorry
+  then obtain ki bs where *: "eval_world_raw t w (Bsig sig) = Lv ki bs"
+    by (meson bexp_wt_cases eval_world_raw_lv)
+  hence IH: " beval_world_raw w t (Bsig sig) (Lv ki bs)"
+    using 17  using bexp_wt.intros(3) by fastforce
+  have "eval_world_raw t w (Bsig sig) = snd w sig t"
+    by simp
+  hence "res = Bv (bs ! idx)"
+    using 17 * unfolding eval_world_raw.simps by auto
+  then show ?case 
+    using IH beval_raw.intros(21)
+    by (metis beval_world_raw.cases beval_world_raw.intros)
 next
   case (18 t w e n)
-  then show ?case sorry
+  then obtain ki bs where *: "eval_world_raw t w e = Lv ki bs" 
+    by (meson bexp_wt_cases(14) eval_world_raw_lv)
+  hence IH : "beval_world_raw w t e (Lv ki bs)"
+    using 18  by (metis bexp_wt_cases(14))
+  have "ki = Uns \<or> ki = Sig"
+    using `bexp_wt \<Gamma> (Bshiftl e n) ty` 
+    by (metis "*" "18.prems"(2) bexp_wt_cases(14) eval_world_raw_lv val.inject(2))
+  hence "res =  Lv ki (drop n (bs @ replicate n False))"
+    using * 18 unfolding eval_world_raw.simps by auto
+  then show ?case 
+    using IH 
+    by (smt "18.prems"(2) "18.prems"(3) beval_raw.intros(28) beval_raw.intros(29) 
+        beval_raw_preserve_well_typedness beval_world_raw.cases beval_world_raw.intros 
+        bexp_wt_cases(14) ty.inject type_of.simps(2) wityping_def wityping_ensure_styping 
+        wityping_ensure_ttyping)
 next
   case (19 t w e n)
-  then show ?case sorry
+  then obtain ki bs where *: "eval_world_raw t w e = Lv ki bs"
+    by (meson bexp_wt_cases(15) eval_world_raw_lv)
+  hence IH : "beval_world_raw w t e (Lv ki bs)"
+    using 19  by (metis bexp_wt_cases(15))
+  have "ki = Uns \<or> ki = Sig"
+    using `bexp_wt \<Gamma> (Bshiftr e n) ty` 
+    by (metis "*" "19.prems"(2) bexp_wt_cases(15) eval_world_raw_lv val.inject(2))
+  moreover
+  { assume "ki = Uns"
+    hence "res = Lv Uns (take (length bs) (replicate n False @ bs))"
+      using 19(2) * unfolding eval_world_raw.simps by auto
+    hence ?case
+      using IH unfolding `ki = Uns` 
+      by (meson beval_raw.intros(30) beval_world_raw.cases beval_world_raw.intros) }
+  moreover
+  { assume "ki = Sig"
+    hence "res = Lv Sig (take (length bs) (replicate n (hd bs) @ bs))"
+      using 19(2) * unfolding eval_world_raw.simps by auto
+    hence ?case
+      using IH unfolding `ki = Sig` 
+      by (meson beval_raw.intros(31) beval_world_raw.cases beval_world_raw.intros) }
+  ultimately show ?case by auto
 next
   case (20 t w th guard el)
-  then show ?case sorry
+  hence "bexp_wt \<Gamma> guard Bty"
+    using bexp_wt_cases_when[OF 20(6)] by auto
+  have " eval_world_raw t w guard = Bv True \<or>  eval_world_raw t w guard = Bv False"
+    by (metis "20.prems"(2) \<open>bexp_wt \<Gamma> guard Bty\<close> eval_world_raw_bv val.inject(1))
+  moreover
+  { assume "eval_world_raw t w guard = Bv True"
+    hence IH0: "beval_world_raw w t guard (Bv True)"
+      using 20(1)  "20.prems"(2) \<open>bexp_wt \<Gamma> guard Bty\<close> by blast
+    have "res = eval_world_raw t w th"
+      using `eval_world_raw t w guard = Bv True` 20(4) by auto
+    hence " beval_world_raw w t th res"
+      using 20(2)  "20.prems"(2) "20.prems"(3) \<open>eval_world_raw t w guard = Bv True\<close> bexp_wt_cases_when by blast
+    hence ?case
+      using IH0  by (meson beval_raw.intros(32) beval_world_raw.cases beval_world_raw.intros) }
+  moreover
+  { assume "eval_world_raw t w guard = Bv False"
+    hence IH0: "beval_world_raw w t guard (Bv False)"
+      using 20(1)  "20.prems"(2) \<open>bexp_wt \<Gamma> guard Bty\<close> by blast
+    have "res = eval_world_raw t w el"
+      using `eval_world_raw t w guard = Bv False` 20(4) by auto
+    hence " beval_world_raw w t el res"
+      using 20(3)  "20.prems"(2) "20.prems"(3) \<open>eval_world_raw t w guard = Bv False\<close> bexp_wt_cases_when by blast  
+    hence ?case
+      by (meson IH0 beval_raw.intros(33) beval_world_raw.cases beval_world_raw.intros) }
+  ultimately show ?case
+    by auto
 next
   case (21 t w sign val)
-  then show ?case sorry
+  then show ?case 
+    by (metis beval_raw.intros(34) beval_world_raw.intros eval_world_raw.simps(21))
 qed
   
+lemma eval_world_raw_correctness_only_if:
+  assumes "beval_world_raw w t exp res"
+  assumes "wityping \<Gamma> w" and  "bexp_wt \<Gamma> exp ty"
+  shows   "eval_world_raw t w exp = res" 
+  using assms
+  by (metis beval_raw_deterministic beval_world_raw.cases eval_world_raw_correctness_if)
 
+section \<open>Typed hoare logic for sequential statements\<close>
 
+abbreviation eval_world_raw2 where "eval_world_raw2 tw exp \<equiv> eval_world_raw (fst tw) (snd tw) exp"
+                                                                    
+inductive
+  seq_hoare3 :: "'signal tyenv \<Rightarrow> 'signal assn2 \<Rightarrow> 'signal seq_stmt \<Rightarrow> 'signal assn2 \<Rightarrow> bool" ("  (1_) \<turnstile> ([(1_)]/ (_)/ [(1_)])" 50)
+  where
+  Null3: " \<Gamma> \<turnstile> [P] Bnull [P]"
 
+| Assign3: "\<Gamma> \<turnstile> [\<lambda>tw. P(tw[sig, dly :=\<^sub>2 eval_world_raw2 tw exp])] Bassign_trans sig exp dly [P]"
+
+| AssignI3: "\<Gamma> \<turnstile> [\<lambda>tw. P( tw\<lbrakk>sig, dly :=\<^sub>2 eval_world_raw2 tw exp\<rbrakk>)] Bassign_inert sig exp dly [P]"
+
+| Comp3: "\<lbrakk> \<Gamma> \<turnstile> [P] s1 [Q]; \<Gamma> \<turnstile> [Q] s2 [R]\<rbrakk> \<Longrightarrow> \<Gamma> \<turnstile> [P] Bcomp s1 s2 [R]"
+
+| If3: "\<lbrakk>\<Gamma> \<turnstile> [\<lambda>tw. P tw \<and> eval_world_raw2 tw g = (Bv True)] s1 [Q];
+         \<Gamma> \<turnstile> [\<lambda>tw. P tw \<and> eval_world_raw2 tw g = (Bv False)] s2 [Q]\<rbrakk>
+        \<Longrightarrow>  \<Gamma> \<turnstile> [P] Bguarded g s1 s2 [Q]"
+
+| Conseq3: "\<lbrakk>\<forall>tw. wityping \<Gamma> (snd tw) \<and> P' tw \<longrightarrow> P tw; \<Gamma> \<turnstile> [P] s [Q]; \<forall>tw. Q tw \<longrightarrow> Q' tw\<rbrakk> \<Longrightarrow> \<Gamma> \<turnstile> [P'] s [Q']"
+
+| Conj3: "\<Gamma> \<turnstile> [P] s [Q1] \<Longrightarrow>  \<Gamma> \<turnstile> [P] s [Q2] \<Longrightarrow>  \<Gamma> \<turnstile> [P] s [\<lambda>tw. Q1 tw \<and> Q2 tw]"
+
+| Bcase_empty_choices3: " \<Gamma> \<turnstile> [P] Bcase exp [] [P]"
+
+| Bcase_others3: " \<Gamma> \<turnstile> [P] ss [Q] \<Longrightarrow>  \<Gamma> \<turnstile> [P] Bcase exp ((Others, ss) # choices) [Q]"
+
+| Bcase_if3: "\<Gamma> \<turnstile> [\<lambda>tw.  P tw \<and> (eval_world_raw2 tw exp = eval_world_raw2 tw exp')] ss [Q]
+  \<Longrightarrow> \<Gamma> \<turnstile> [\<lambda>tw. P tw \<and> (eval_world_raw2 tw exp \<noteq> eval_world_raw2 tw exp')] Bcase exp choices [Q]
+  \<Longrightarrow>  \<Gamma> \<turnstile> [P] Bcase exp ((Explicit exp', ss) # choices) [Q]"
+
+lemma seq_hoare3_soundness:
+  assumes "\<Gamma> \<turnstile> [P] ss [Q]"
+  assumes "seq_wt \<Gamma> ss" and  "nonneg_delay ss"
+  shows   "\<Gamma> \<Turnstile> [P] ss [Q]"
+  using assms
+proof (induction rule:seq_hoare3.induct)
+  case (Null3 P)
+  then show ?case 
+    unfolding seq_hoare_valid2_wt_def 
+    using world_seq_exec_bnull world_seq_exec_deterministic by blast
+next
+  case (Assign3 \<Gamma> P sig dly exp)
+  then obtain ty where "bexp_wt \<Gamma> exp ty" and "0 < dly"
+    by auto
+  then show ?case 
+    unfolding seq_hoare_valid2_wt_def 
+    by (metis beval_world_raw2_def eval_world_raw_correctness_only_if lift_world_trans_worldline_upd2)
+next
+  case (AssignI3 \<Gamma> P sig dly exp)
+  then obtain ty where "bexp_wt \<Gamma> exp ty" and "0 < dly"
+    by auto
+  then show ?case 
+    unfolding seq_hoare_valid2_wt_def 
+    by (metis beval_world_raw2_def eval_world_raw_correctness_only_if lift_world_inert_worldline_upd2)
+next
+  case (Comp3 \<Gamma> P s1 Q s2 R)
+  hence " \<Gamma> \<Turnstile> [P] s1 [Q]" and " \<Gamma> \<Turnstile> [Q] s2 [R]"
+    using nonneg_delay.simps(2) by blast+
+  then show ?case 
+    unfolding seq_hoare_valid2_wt_def using Comp3(6) world_seq_exec_comp
+    by (smt Comp3.prems(1) nonneg_delay.simps(2) seq_hoare_valid2_def seq_stmt_preserve_wityping_hoare 
+        seq_wt_cases(2) soundness_hoare2 world_seq_exec_alt_cases(2) world_seq_exec_alt_imp_world_seq_exec 
+        world_seq_exec_imp_world_seq_exec_alt)
+next
+  case (If3 \<Gamma> P g s1 Q s2)
+  have "nonneg_delay s1" and "nonneg_delay s2"
+    using If3  nonneg_delay.simps(3) by blast+
+  have "\<Gamma> \<Turnstile> [\<lambda>a. P a \<and> eval_world_raw2 a g = Bv True] s1 [Q]" and " \<Gamma> \<Turnstile> [\<lambda>a. P a \<and> eval_world_raw2 a g = Bv False] s2 [Q]"
+    using If3 nonneg_delay.simps(3) by blast+
+  then show ?case 
+    unfolding seq_hoare_valid2_wt_def world_seq_exec_alt_def[OF If3(6), THEN sym]
+    world_seq_exec_alt_def[OF `nonneg_delay s1`, THEN sym] world_seq_exec_alt_def[OF `nonneg_delay s2`, THEN sym]
+    by (metis If3.prems(1) beval_world_raw2_def eval_world_raw_correctness_only_if seq_wt_cases(3) world_seq_exec_alt_cases(3))
+next
+  case (Conseq3 \<Gamma> P' P s Q Q')
+  hence " \<Gamma> \<Turnstile> [P] s [Q]"  by blast
+  then show ?case 
+    using Conseq3(1) Conseq3(3) unfolding seq_hoare_valid2_wt_def  by blast 
+next
+  case (Conj3 \<Gamma> P s Q1 Q2)
+  hence "\<Gamma> \<Turnstile> [P] s [Q1]" and "\<Gamma> \<Turnstile> [P] s [Q1]"
+    by blast+
+  then show ?case 
+    unfolding seq_hoare_valid2_wt_def  
+    by (metis Conj3.IH(2) Conj3.prems(1) Conj3.prems(2) seq_hoare_valid2_wt_def)
+next 
+  case (Bcase_empty_choices3 \<Gamma> P exp)
+  then show ?case 
+    unfolding seq_hoare_valid2_wt_def  using world_seq_exec_bcase_empty world_seq_exec_deterministic by blast
+next
+  case (Bcase_others3 \<Gamma> P ss Q exp choices)
+  hence "seq_wt \<Gamma> ss "
+    using seq_wt.cases by auto
+  moreover have "nonneg_delay ss"
+    using Bcase_others3 by auto
+  ultimately have " \<Gamma> \<Turnstile> [P] ss [Q]"
+    using Bcase_others3(2) by auto
+  then show ?case 
+    unfolding seq_hoare_valid2_wt_def  using bcase_others_tw_elim by blast 
+next
+  case (Bcase_if3 \<Gamma> P exp exp' ss Q choices)
+  hence "seq_wt \<Gamma> ss" and "seq_wt \<Gamma> (Bcase exp choices)"
+    using seq_wt_cases_bcase by auto
+  moreover obtain ty where ty: "bexp_wt \<Gamma> exp ty \<and> bexp_wt \<Gamma> exp' ty"
+    using Bcase_if3.prems(1) seq_wt_cases_bcase by force
+  moreover have " nonneg_delay ss" and "nonneg_delay (Bcase exp choices)"
+    using Bcase_if3(6) by auto
+  ultimately have 1: "\<Gamma> \<Turnstile> [\<lambda>a. P a \<and> eval_world_raw2 a exp = eval_world_raw2 a exp'] ss [Q]" and 
+    2: "\<Gamma> \<Turnstile> [\<lambda>a. P a \<and> eval_world_raw2 a exp \<noteq> eval_world_raw2 a exp'] Bcase exp choices [Q]"
+    using Bcase_if3(3-4) by auto
+  show ?case 
+    unfolding seq_hoare_valid2_wt_def  world_seq_exec_alt_def[OF Bcase_if3(6), THEN sym]
+  proof (intro allI, intro impI)
+    fix tw tw' :: "nat \<times> ('a \<Rightarrow> val) \<times> ('a \<Rightarrow> nat \<Rightarrow> val)"
+    assume asm: "wityping \<Gamma> (snd tw) \<and> P tw \<and> world_seq_exec_alt tw (Bcase exp ((Explicit exp', ss) # choices)) tw'"
+    hence "world_seq_exec_alt tw (Bcase exp ((Explicit exp', ss) # choices)) tw'"
+      by auto
+    have "eval_world_raw2 tw exp = eval_world_raw2 tw exp' \<or> eval_world_raw2 tw exp \<noteq> eval_world_raw2 tw exp'"
+      by auto
+    moreover
+    { assume "eval_world_raw2 tw exp = eval_world_raw2 tw exp'"
+      obtain res where " beval_world_raw (snd tw) (fst tw) exp res"
+        using eval_world_raw_correctness_if ty asm  by blast
+      obtain res' where "beval_world_raw (snd tw) (fst tw) exp' res'"
+        using eval_world_raw_correctness_if ty asm by blast
+      hence "world_seq_exec_alt tw ss tw'"
+        using world_seq_exec_alt.cases[OF `world_seq_exec_alt tw (Bcase exp ((Explicit exp', ss) # choices)) tw'`]
+        by (smt Pair_inject \<open>eval_world_raw2 tw exp = eval_world_raw2 tw exp'\<close> asm beval_world_raw2_def 
+            choices.inject eval_world_raw_correctness_only_if list.distinct(1) list.inject 
+            seq_stmt.distinct(29) seq_stmt.distinct(9) seq_stmt.inject(5) seq_stmt.simps(23) 
+            seq_stmt.simps(29) seq_stmt.simps(33) ty) 
+      hence "Q tw'"
+        by (metis (mono_tags, lifting) "1" \<open>eval_world_raw2 tw exp = eval_world_raw2 tw exp'\<close> 
+            \<open>nonneg_delay ss\<close> asm seq_hoare_valid2_wt_def world_seq_exec_alt_imp_world_seq_exec) }
+    moreover
+    { assume "eval_world_raw2 tw exp \<noteq> eval_world_raw2 tw exp'"
+      obtain res where " beval_world_raw (snd tw) (fst tw) exp res"
+        using eval_world_raw_correctness_if ty asm  by blast
+      obtain res' where "beval_world_raw (snd tw) (fst tw) exp' res'"
+        using eval_world_raw_correctness_if ty asm by blast    
+      hence "world_seq_exec_alt tw (Bcase exp choices) tw'"
+        using world_seq_exec_alt.cases[OF `world_seq_exec_alt tw (Bcase exp ((Explicit exp', ss) # choices)) tw'`]
+        by (smt Pair_inject \<open>eval_world_raw2 tw exp \<noteq> eval_world_raw2 tw exp'\<close> asm beval_world_raw2_def 
+                choices.distinct(1) choices.inject eval_world_raw_correctness_only_if list.distinct(1) 
+                list.inject seq_stmt.distinct(29) seq_stmt.distinct(9) seq_stmt.inject(5) seq_stmt.simps(23) 
+                seq_stmt.simps(29) seq_stmt.simps(33) ty) 
+      hence "Q tw'"
+        by (smt "2" \<open>eval_world_raw2 tw exp \<noteq> eval_world_raw2 tw exp'\<close> \<open>nonneg_delay (Bcase exp choices)\<close> 
+                asm seq_hoare_valid2_wt_def world_seq_exec_alt_imp_world_seq_exec) }
+    ultimately show "Q tw'"
+      by auto
+  qed
+qed
+
+text \<open>weakest precondition for typed hoare logic\<close>
+
+definition wp3 :: "'signal tyenv \<Rightarrow> 'signal seq_stmt \<Rightarrow> 'signal assn2 \<Rightarrow> 'signal assn2" where
+  "wp3 \<Gamma> ss Q = (\<lambda>tw. wityping \<Gamma> (snd tw) \<and> (\<forall>tw'. (tw, ss \<Rightarrow>\<^sub>s tw') \<longrightarrow> Q tw'))"
+
+lemma wp3_bnull:
+  "wp3 \<Gamma> Bnull Q = (\<lambda>tw. Q tw \<and> wityping \<Gamma> (snd tw))"
+  apply (rule ext)
+  unfolding wp3_def
+  using world_seq_exec_bnull world_seq_exec_deterministic by blast
+
+lemma wp3_bcomp:
+  assumes "seq_wt \<Gamma> (Bcomp ss1 ss2)" and "nonneg_delay (Bcomp ss1 ss2)"
+  shows "wp3 \<Gamma> (Bcomp ss1 ss2) Q = wp3 \<Gamma> ss1 (wp3 \<Gamma> ss2 Q)"
+  apply (rule ext)
+  unfolding wp3_def
+proof (rule, rule, simp, rule, rule, rule)
+  fix x tw' :: "nat \<times> ('a \<Rightarrow> val) \<times> ('a \<Rightarrow> nat \<Rightarrow> val)"
+  have "seq_wt \<Gamma> ss1" and "seq_wt \<Gamma> ss2"
+    using assms by blast+
+  assume asm: "wityping \<Gamma> (snd x) \<and> (\<forall>tw'. x, Bcomp ss1 ss2 \<Rightarrow>\<^sub>s tw' \<longrightarrow> Q tw')" and "x, ss1 \<Rightarrow>\<^sub>s tw'" 
+  thus " wityping \<Gamma> (snd tw')"
+    using soundness_hoare2[OF seq_stmt_preserve_wityping_hoare[OF `seq_wt \<Gamma> ss1`]] assms(2)
+    unfolding seq_hoare_valid2_def  using nonneg_delay.simps(2) by blast
+
+  { fix tw2 
+    assume "tw', ss2 \<Rightarrow>\<^sub>s tw2"
+    hence "x, Bcomp ss1 ss2 \<Rightarrow>\<^sub>s tw2"
+      using `x, ss1 \<Rightarrow>\<^sub>s tw'`  using assms(2) world_seq_exec_comp by blast
+    with asm  have " Q tw2" by blast
+    moreover have "wityping \<Gamma> (snd tw2)"
+      using  `wityping \<Gamma> (snd tw')` `tw', ss2 \<Rightarrow>\<^sub>s tw2` soundness_hoare2[OF seq_stmt_preserve_wityping_hoare[OF `seq_wt \<Gamma> ss2`]] assms(2)
+      unfolding seq_hoare_valid2_def   using nonneg_delay.simps(2) by blast
+    ultimately have "Q tw2 \<and> wityping \<Gamma> (snd tw2)"
+      by auto }
+  thus " \<forall>tw'a. tw', ss2 \<Rightarrow>\<^sub>s tw'a \<longrightarrow> Q tw'a"
+    by auto
+next
+  fix x
+  assume *: " wityping \<Gamma> (snd x) \<and> (\<forall>tw'. x, ss1 \<Rightarrow>\<^sub>s tw' \<longrightarrow> wityping \<Gamma> (snd tw') \<and> (\<forall>tw'a. tw', ss2 \<Rightarrow>\<^sub>s tw'a \<longrightarrow> Q tw'a))"
+  hence "(\<forall>tw'. x, Bcomp ss1 ss2 \<Rightarrow>\<^sub>s tw' \<longrightarrow> Q tw')"
+    by (meson assms(2) nonneg_delay.simps(2) world_seq_exec_alt_cases(2) world_seq_exec_alt_imp_world_seq_exec world_seq_exec_imp_world_seq_exec_alt)
+  moreover have "wityping \<Gamma> (snd x)"
+    using * by auto
+  ultimately show "wityping \<Gamma> (snd x) \<and> (\<forall>tw'. x, Bcomp ss1 ss2 \<Rightarrow>\<^sub>s tw' \<longrightarrow> Q tw')"
+    by auto
+qed
+
+lemma wp3_bguarded:
+  assumes "seq_wt \<Gamma> (Bguarded g ss1 ss2)" and "nonneg_delay (Bguarded g ss1 ss2)"
+  shows "wp3 \<Gamma> (Bguarded g ss1 ss2) Q = (\<lambda>tw. if eval_world_raw2 tw g = Bv True then 
+                                                wp3 \<Gamma> ss1 Q tw 
+                                              else 
+                                                wp3 \<Gamma> ss2 Q tw)"
+  apply (rule ext)
+  unfolding wp3_def
+proof (rule)
+  fix tw
+  obtain ty where bwt: "bexp_wt \<Gamma> g ty" and "seq_wt \<Gamma> ss1" and "seq_wt \<Gamma> ss2"
+    using assms  by blast
+  assume asm: " wityping \<Gamma> (snd tw) \<and> (\<forall>tw'. tw, Bguarded g ss1 ss2 \<Rightarrow>\<^sub>s tw' \<longrightarrow> Q tw')"
+  hence wt: "wityping \<Gamma> (snd tw)" by auto
+  have "eval_world_raw2 tw g = Bv True \<or> eval_world_raw2 tw g \<noteq> Bv True"
+    by auto
+  moreover
+  { assume "eval_world_raw2 tw g = Bv True"
+    hence "beval_world_raw2 tw g (Bv True)"
+      using eval_world_raw_correctness_if[OF _ wt bwt] by (simp add: beval_world_raw2_def)
+    { fix tw'
+      assume "tw, ss1 \<Rightarrow>\<^sub>s tw'"
+      hence "Q tw'"
+        using asm world_seq_exec_guarded[OF `beval_world_raw2 tw g (Bv True)` `tw, ss1 \<Rightarrow>\<^sub>s tw'`]
+        by blast 
+      moreover have "wityping \<Gamma> (snd tw')"
+        using soundness_hoare2[OF seq_stmt_preserve_wityping_hoare[OF `seq_wt \<Gamma> ss1`]] assms(2)
+        unfolding seq_hoare_valid2_def using `tw, ss1 \<Rightarrow>\<^sub>s tw'`  using nonneg_delay.simps(3) wt by blast
+      ultimately have "Q tw' \<and> wityping \<Gamma> (snd tw')"
+        by auto }
+    hence "(\<forall>tw'. tw, ss1 \<Rightarrow>\<^sub>s tw' \<longrightarrow> Q tw' \<and> wityping \<Gamma> (snd tw'))"
+      by auto
+    hence "if eval_world_raw2 tw g = Bv True then wityping \<Gamma> (snd tw) \<and> (\<forall>tw'. tw, ss1 \<Rightarrow>\<^sub>s tw' \<longrightarrow> Q tw' \<and> wityping \<Gamma> (snd tw'))
+          else wityping \<Gamma> (snd tw) \<and> (\<forall>tw'. tw, ss2 \<Rightarrow>\<^sub>s tw' \<longrightarrow> Q tw' \<and> wityping \<Gamma> (snd tw'))"
+      using wt `eval_world_raw2 tw g = Bv True` by auto }
+  moreover
+  { assume "eval_world_raw2 tw g \<noteq> Bv True"
+    hence  "eval_world_raw2 tw g = Bv False"
+      by (metis assms(1) eval_world_raw_bv seq_wt_cases(3) wt)
+    hence "beval_world_raw2 tw g (Bv False)"
+      using eval_world_raw_correctness_if[OF _ wt bwt] by (simp add: beval_world_raw2_def)
+    { fix tw'
+      assume "tw, ss2 \<Rightarrow>\<^sub>s tw'"
+      hence "Q tw'"
+        using asm world_seq_exec_guarded_not[OF `beval_world_raw2 tw g (Bv False)` `tw, ss2 \<Rightarrow>\<^sub>s tw'`]
+        by blast 
+      moreover have "wityping \<Gamma> (snd tw')"
+        using soundness_hoare2[OF seq_stmt_preserve_wityping_hoare[OF `seq_wt \<Gamma> ss2`]] assms(2)
+        unfolding seq_hoare_valid2_def using `tw, ss2 \<Rightarrow>\<^sub>s tw'`  using nonneg_delay.simps(3) wt by blast
+      ultimately have "Q tw' \<and> wityping \<Gamma> (snd tw')"
+        by auto }
+    hence "(\<forall>tw'. tw, ss2 \<Rightarrow>\<^sub>s tw' \<longrightarrow> Q tw' \<and> wityping \<Gamma> (snd tw'))"
+      by auto    
+    hence "if eval_world_raw2 tw g = Bv True then wityping \<Gamma> (snd tw) \<and> (\<forall>tw'. tw, ss1 \<Rightarrow>\<^sub>s tw' \<longrightarrow> Q tw' \<and> wityping \<Gamma> (snd tw'))
+          else wityping \<Gamma> (snd tw) \<and> (\<forall>tw'. tw, ss2 \<Rightarrow>\<^sub>s tw' \<longrightarrow> Q tw' \<and> wityping \<Gamma> (snd tw'))"
+      using wt `eval_world_raw2 tw g = Bv False` by auto }
+  ultimately show "if eval_world_raw2 tw g = Bv True then wityping \<Gamma> (snd tw) \<and> (\<forall>tw'. tw, ss1 \<Rightarrow>\<^sub>s tw' \<longrightarrow> Q tw')
+          else wityping \<Gamma> (snd tw) \<and> (\<forall>tw'. tw, ss2 \<Rightarrow>\<^sub>s tw' \<longrightarrow> Q tw')" by auto
+next
+  fix tw
+  assume *: "if eval_world_raw2 tw g = Bv True then wityping \<Gamma> (snd tw) \<and> (\<forall>tw'. tw, ss1 \<Rightarrow>\<^sub>s tw' \<longrightarrow> Q tw')
+          else wityping \<Gamma> (snd tw) \<and> (\<forall>tw'. tw, ss2 \<Rightarrow>\<^sub>s tw' \<longrightarrow> Q tw')"
+  hence " wityping \<Gamma> (snd tw)"
+    by presburger
+  { fix tw' 
+    assume "tw, Bguarded g ss1 ss2 \<Rightarrow>\<^sub>s tw'"
+    hence "Q tw'"
+      using * 
+      by (smt assms(1) assms(2) beval_world_raw2_def eval_world_raw_correctness_only_if 
+          nonneg_delay.simps(3) seq_wt_cases(3) val.simps(1) world_seq_exec_alt_cases(3) 
+          world_seq_exec_alt_imp_world_seq_exec world_seq_exec_imp_world_seq_exec_alt) }
+  thus "wityping \<Gamma> (snd tw) \<and> (\<forall>tw'. tw, Bguarded g ss1 ss2 \<Rightarrow>\<^sub>s tw' \<longrightarrow> Q tw')"
+    using `wityping \<Gamma> (snd tw)` by auto
+qed
+
+lemma wp3_bcase_empty:
+  "wp3 \<Gamma> (Bcase exp []) Q = (\<lambda>tw. Q tw \<and> wityping \<Gamma> (snd tw))"
+  apply (rule ext)
+  unfolding wp3_def  using world_seq_exec_bcase_empty world_seq_exec_deterministic by blast
+
+lemma wp3_bcase_others:
+  assumes "seq_wt \<Gamma> (Bcase exp ((Others, ss) # choices))" and "nonneg_delay (Bcase exp ((Others, ss) # choices))"
+  shows "wp3 \<Gamma> (Bcase exp ((Others, ss) # choices)) Q = wp3 \<Gamma> ss Q"
+  apply (rule ext)
+  unfolding wp3_def
+proof (rule, rule, simp, rule, rule)
+  fix x tw'
+  have "seq_wt \<Gamma> ss "
+    using assms  seq_wt_cases_bcase by auto
+  assume *: "wityping \<Gamma> (snd x) \<and> (\<forall>tw'. x, Bcase exp ((Others, ss) # choices) \<Rightarrow>\<^sub>s tw' \<longrightarrow> Q tw')" and "x, ss \<Rightarrow>\<^sub>s tw'"
+  thus "Q tw'"
+    using world_seq_exec_bcase_others by blast
+next
+  fix x
+  assume *: " wityping \<Gamma> (snd x) \<and> (\<forall>tw'. x, ss \<Rightarrow>\<^sub>s tw' \<longrightarrow> Q tw') "
+  hence "wityping \<Gamma> (snd x)" by auto
+  { fix tw'
+    assume "x, Bcase exp ((Others, ss) # choices) \<Rightarrow>\<^sub>s tw'"
+    hence "x, ss \<Rightarrow>\<^sub>s tw'" 
+      using bcase_others_tw_elim by blast
+    with * have "Q tw'"  
+      by blast }
+  with `wityping \<Gamma> (snd x)` show " wityping \<Gamma> (snd x) \<and> (\<forall>tw'. x, Bcase exp ((Others, ss) # choices) \<Rightarrow>\<^sub>s tw' \<longrightarrow> Q tw')"
+    by auto
+qed
+
+lemma wp3_bcase_explicit:
+  assumes "seq_wt \<Gamma> (Bcase exp ((Explicit exp', ss) # choices))" and "nonneg_delay (Bcase exp ((Explicit exp', ss) # choices))"
+  shows "wp3 \<Gamma> (Bcase exp ((Explicit exp', ss) # choices)) Q = 
+  (\<lambda>tw. if eval_world_raw2 tw exp = eval_world_raw2 tw exp' then wp3 \<Gamma> ss Q tw  else wp3 \<Gamma> (Bcase exp choices) Q tw)"
+  apply (rule ext)
+  unfolding wp3_def
+proof (rule)
+  fix tw
+  assume *: "wityping \<Gamma> (snd tw) \<and> (\<forall>tw'. tw, Bcase exp ((Explicit exp', ss) # choices) \<Rightarrow>\<^sub>s tw' \<longrightarrow> Q tw')"
+  hence wt : "wityping \<Gamma> (snd tw)" by auto
+  obtain ty where "bexp_wt \<Gamma> exp ty" and " bexp_wt \<Gamma> exp' ty"
+    using assms(1) 
+    by (smt choices.distinct(1) choices.sel fst_conv list.distinct(1) list.sel(1) seq_stmt.inject(5)
+    seq_stmt.simps(15) seq_stmt.simps(23) seq_stmt.simps(29) seq_stmt.simps(33) seq_stmt.simps(35)
+    seq_wt.cases)
+  have "seq_wt \<Gamma> ss" and "nonneg_delay ss" and "seq_wt \<Gamma> (Bcase exp choices)" and "nonneg_delay (Bcase exp choices)"
+    using assms  seq_wt.cases by auto
+  have "eval_world_raw2 tw exp = eval_world_raw2 tw exp' \<or> eval_world_raw2 tw exp \<noteq> eval_world_raw2 tw exp'"
+    by auto
+  moreover
+  { assume "eval_world_raw2 tw exp = eval_world_raw2 tw exp'"
+    then obtain match where match: "beval_world_raw2 tw exp match \<and> beval_world_raw2 tw exp' match"
+      using eval_world_raw_correctness_if[OF _ `wityping \<Gamma> (snd tw)` `bexp_wt \<Gamma> exp ty`]
+      eval_world_raw_correctness_if[OF _ `wityping \<Gamma> (snd tw)` `bexp_wt \<Gamma> exp' ty`] 
+      by (metis beval_world_raw2_def)
+    { fix tw'
+      assume "tw, ss \<Rightarrow>\<^sub>s tw'"
+      hence  "Q tw'"
+        using * world_seq_exec_explicit_match match  by blast 
+      moreover have "wityping \<Gamma> (snd tw')"
+        using soundness_hoare2[ OF seq_stmt_preserve_wityping_hoare[OF `seq_wt \<Gamma> ss`] `nonneg_delay ss`]
+        unfolding seq_hoare_valid2_def using wt `tw, ss\<Rightarrow>\<^sub>s tw'`  by blast
+      ultimately have "Q tw' \<and> wityping \<Gamma> (snd tw')"
+        by auto }
+    hence "if eval_world_raw2 tw exp = eval_world_raw2 tw exp' then wityping \<Gamma> (snd tw) \<and> (\<forall>tw'. tw, ss \<Rightarrow>\<^sub>s tw' \<longrightarrow> Q tw' \<and> wityping \<Gamma> (snd tw'))
+          else wityping \<Gamma> (snd tw) \<and> (\<forall>tw'. tw, Bcase exp choices \<Rightarrow>\<^sub>s tw' \<longrightarrow> Q tw' \<and> wityping \<Gamma> (snd tw'))"
+      using `eval_world_raw2 tw exp = eval_world_raw2 tw exp'` wt  by simp }
+  moreover
+  { assume neq: "eval_world_raw2 tw exp \<noteq> eval_world_raw2 tw exp'"
+    obtain res1 res2 where "eval_world_raw2 tw exp = res1" and "eval_world_raw2 tw exp' = res2"
+      by auto
+    hence neq': "beval_world_raw2 tw exp res1 \<and> beval_world_raw2 tw exp' res2 \<and> res1 \<noteq> res2"
+      using eval_world_raw_correctness_if[OF `eval_world_raw2 tw exp = res1` `wityping \<Gamma> (snd tw)` `bexp_wt \<Gamma> exp ty`]
+      eval_world_raw_correctness_if[OF `eval_world_raw2 tw exp' = res2` `wityping \<Gamma> (snd tw)` `bexp_wt \<Gamma> exp' ty`]
+      neq unfolding beval_world_raw2_def by auto
+    { fix tw' 
+      assume " tw, Bcase exp choices \<Rightarrow>\<^sub>s tw'"
+      hence "Q tw'"
+        using * neq' world_seq_exec_explicit_no_match by blast
+      moreover have "wityping \<Gamma> (snd tw')"
+        using soundness_hoare2[ OF seq_stmt_preserve_wityping_hoare[OF `seq_wt \<Gamma> (Bcase exp choices)`] `nonneg_delay (Bcase exp choices)`]
+        unfolding seq_hoare_valid2_def using wt `tw, Bcase exp choices \<Rightarrow>\<^sub>s tw'`  by blast
+      ultimately have "Q tw' \<and> wityping \<Gamma> (snd tw')"
+        by auto }
+    hence "if eval_world_raw2 tw exp = eval_world_raw2 tw exp' then wityping \<Gamma> (snd tw) \<and> (\<forall>tw'. tw, ss \<Rightarrow>\<^sub>s tw' \<longrightarrow> Q tw' \<and> wityping \<Gamma> (snd tw'))
+          else wityping \<Gamma> (snd tw) \<and> (\<forall>tw'. tw, Bcase exp choices \<Rightarrow>\<^sub>s tw' \<longrightarrow> Q tw' \<and> wityping \<Gamma> (snd tw'))"
+      using `eval_world_raw2 tw exp \<noteq> eval_world_raw2 tw exp'` wt  by simp }
+  ultimately show "if eval_world_raw2 tw exp = eval_world_raw2 tw exp' then wityping \<Gamma> (snd tw) \<and> (\<forall>tw'. tw, ss \<Rightarrow>\<^sub>s tw' \<longrightarrow> Q tw')
+          else wityping \<Gamma> (snd tw) \<and> (\<forall>tw'. tw, Bcase exp choices \<Rightarrow>\<^sub>s tw' \<longrightarrow> Q tw')"
+    by auto
+next
+  fix tw
+  assume *: " if eval_world_raw2 tw exp = eval_world_raw2 tw exp' then wityping \<Gamma> (snd tw) \<and> (\<forall>tw'. tw, ss \<Rightarrow>\<^sub>s tw' \<longrightarrow> Q tw')
+          else wityping \<Gamma> (snd tw) \<and> (\<forall>tw'. tw, Bcase exp choices \<Rightarrow>\<^sub>s tw' \<longrightarrow> Q tw') "
+  hence "wityping \<Gamma> (snd tw)" by presburger
+  obtain ty where "bexp_wt \<Gamma> exp ty" and "bexp_wt \<Gamma> exp' ty" using assms(1)  
+    by (smt choices.distinct(1) choices.sel fst_conv list.distinct(1) list.sel(1) seq_stmt.inject(5)
+    seq_stmt.simps(15) seq_stmt.simps(23) seq_stmt.simps(29) seq_stmt.simps(33) seq_stmt.simps(35)
+    seq_wt.cases)
+  have "nonneg_delay ss" and "nonneg_delay (Bcase exp choices)"
+    using assms(2) by auto
+  { fix tw'
+    assume "tw, Bcase exp ((Explicit exp', ss) # choices) \<Rightarrow>\<^sub>s tw'"
+    hence **: "world_seq_exec_alt tw (Bcase exp ((Explicit exp', ss) # choices)) tw'"
+      using assms(2) world_seq_exec_imp_world_seq_exec_alt by blast
+    have "Q tw'"
+    proof (rule world_seq_exec_alt_cases(6)[OF **])
+      fix x
+      assume "beval_world_raw2 tw exp x" and "beval_world_raw2 tw exp' x"
+      hence "eval_world_raw2 tw exp = x" and "eval_world_raw2 tw exp' = x"
+        using eval_world_raw_correctness_only_if[OF _ `wityping \<Gamma> (snd tw)` `bexp_wt \<Gamma> exp ty`]
+        using eval_world_raw_correctness_only_if[OF _ `wityping \<Gamma> (snd tw)` `bexp_wt \<Gamma> exp' ty`]
+        by (simp add: beval_world_raw2_def)+
+      assume "world_seq_exec_alt tw ss tw'"
+      hence "tw, ss \<Rightarrow>\<^sub>s tw'"
+        using world_seq_exec_alt_imp_world_seq_exec[OF _ `nonneg_delay ss`] by auto
+      thus "Q tw'"
+        using * 
+        by (simp add: \<open>if eval_world_raw2 tw exp = eval_world_raw2 tw exp' then wityping \<Gamma> (snd tw)
+        \<and> (\<forall>tw'. tw, ss \<Rightarrow>\<^sub>s tw' \<longrightarrow> Q tw') else wityping \<Gamma> (snd tw) \<and> (\<forall>tw'.
+        tw, Bcase exp choices \<Rightarrow>\<^sub>s tw' \<longrightarrow> Q tw')\<close> \<open>eval_world_raw2 tw exp = x\<close>
+        \<open>eval_world_raw2 tw exp' = x\<close>)
+    next
+      fix x x'
+      assume "beval_world_raw2 tw exp x" and "beval_world_raw2 tw exp' x'" and "x \<noteq> x'"
+      hence "eval_world_raw2 tw exp = x" and "eval_world_raw2 tw exp' = x'"
+        using eval_world_raw_correctness_only_if[OF _ `wityping \<Gamma> (snd tw)` `bexp_wt \<Gamma> exp ty`]
+        using eval_world_raw_correctness_only_if[OF _ `wityping \<Gamma> (snd tw)` `bexp_wt \<Gamma> exp' ty`]
+        using beval_world_raw2_deterministic  by (simp add: beval_world_raw2_def)+
+      assume "world_seq_exec_alt tw (Bcase exp choices) tw'"
+      hence "tw, Bcase exp choices \<Rightarrow>\<^sub>s tw'"
+        using world_seq_exec_alt_imp_world_seq_exec[OF _ `nonneg_delay (Bcase exp choices)`]
+        by blast
+      thus "Q tw'"
+        using * 
+        by (simp add: \<open>if eval_world_raw2 tw exp = eval_world_raw2 tw exp' then wityping \<Gamma> (snd tw)
+        \<and> (\<forall>tw'. tw, ss \<Rightarrow>\<^sub>s tw' \<longrightarrow> Q tw') else wityping \<Gamma> (snd tw) \<and> (\<forall>tw'.
+        tw, Bcase exp choices \<Rightarrow>\<^sub>s tw' \<longrightarrow> Q tw')\<close> \<open>eval_world_raw2 tw exp = x\<close>
+        \<open>eval_world_raw2 tw exp' = x'\<close> \<open>x \<noteq> x'\<close>)
+    qed }
+  thus "wityping \<Gamma> (snd tw) \<and> (\<forall>tw'. tw, Bcase exp ((Explicit exp', ss) # choices) \<Rightarrow>\<^sub>s tw' \<longrightarrow> Q tw')"
+    using `wityping \<Gamma> (snd tw)` by auto
+qed
+
+lemma wp3_assign_trans:
+  assumes "seq_wt \<Gamma> (Bassign_trans sig exp dly)" and " nonneg_delay (Bassign_trans sig exp dly)"
+  shows "wp3 \<Gamma> (Bassign_trans sig exp dly) Q = (\<lambda>tw. wityping \<Gamma> (snd tw) \<and> Q(tw[sig, dly :=\<^sub>2 eval_world_raw2 tw exp]))"
+  apply (rule ext)
+  unfolding wp3_def
+proof (rule, rule, simp)
+  fix tw
+  assume prem: "wityping \<Gamma> (snd tw) \<and> (\<forall>tw'. tw, Bassign_trans sig exp dly \<Rightarrow>\<^sub>s tw' \<longrightarrow> Q tw')"
+  obtain tw' where "tw, Bassign_trans sig exp dly \<Rightarrow>\<^sub>s tw'"
+    by (metis assms(1) assms(2) beval_world_raw2_def eval_world_raw_correctness_if
+    nonneg_delay.simps(4) prem seq_wt_cases(4) world_seq_exec_trans)
+  have "beval_world_raw2 tw exp (eval_world_raw2 tw exp)"
+    by (metis assms(1) beval_world_raw2_def eval_world_raw_correctness_if prem seq_wt_cases(4))
+  thus "Q tw[ sig, dly :=\<^sub>2 eval_world_raw2 tw exp]"
+    using prem  by (meson assms(2) nonneg_delay.simps(4) world_seq_exec_trans)
+next
+  fix tw
+  assume *: "wityping \<Gamma> (snd tw) \<and> Q tw[ sig, dly :=\<^sub>2 eval_world_raw2 tw exp] "
+  hence wt : "wityping \<Gamma> (snd tw)" by auto
+  { fix tw'
+    assume "tw, Bassign_trans sig exp dly \<Rightarrow>\<^sub>s tw'"
+    hence "Q tw'"
+      using *
+      by (metis assms(1) assms(2) beval_world_raw2_def eval_world_raw_correctness_only_if
+      lift_world_trans_worldline_upd2 nonneg_delay.simps(4) seq_wt_cases(4)) }
+  thus "wityping \<Gamma> (snd tw) \<and> (\<forall>tw'. tw, Bassign_trans sig exp dly \<Rightarrow>\<^sub>s tw' \<longrightarrow> Q tw')"
+    using wt by auto
+qed
+
+lemma wp3_assign_inert:
+  assumes "seq_wt \<Gamma> (Bassign_inert sig exp dly)" and " nonneg_delay (Bassign_inert sig exp dly)"
+  shows "wp3 \<Gamma> (Bassign_inert sig exp dly) Q = (\<lambda>tw. wityping \<Gamma> (snd tw) \<and> Q(tw\<lbrakk>sig, dly :=\<^sub>2 eval_world_raw2 tw exp\<rbrakk>))"
+  apply (rule ext)
+  unfolding wp3_def
+proof (rule, rule, simp)
+  fix tw
+  assume prem: "wityping \<Gamma> (snd tw) \<and> (\<forall>tw'. tw, Bassign_inert sig exp dly \<Rightarrow>\<^sub>s tw' \<longrightarrow> Q tw')"
+  obtain tw' where "tw, Bassign_inert sig exp dly \<Rightarrow>\<^sub>s tw'"
+    by (metis assms(1) assms(2) beval_world_raw2_def eval_world_raw_correctness_if
+    nonneg_delay.simps(5) prem seq_wt_cases(5) world_seq_exec_inert)
+  have "beval_world_raw2 tw exp (eval_world_raw2 tw exp)"
+    by (metis assms(1) beval_world_raw2_def eval_world_raw_correctness_if prem seq_wt_cases(5))
+  thus "Q tw\<lbrakk> sig, dly :=\<^sub>2 eval_world_raw2 tw exp\<rbrakk>"
+    using prem   by (meson assms(2) nonneg_delay.simps(5) world_seq_exec_inert)
+next
+  fix tw
+  assume *: "wityping \<Gamma> (snd tw) \<and> Q tw\<lbrakk>sig, dly :=\<^sub>2 eval_world_raw2 tw exp\<rbrakk> "
+  hence wt : "wityping \<Gamma> (snd tw)" by auto
+  { fix tw'
+    assume "tw, Bassign_inert sig exp dly \<Rightarrow>\<^sub>s tw'"
+    hence "Q tw'"
+      using * 
+      by (metis assms(1) assms(2) beval_world_raw2_def eval_world_raw_correctness_only_if
+      lift_world_inert_worldline_upd2 nonneg_delay.simps(5) seq_wt_cases(5))  }
+  thus "wityping \<Gamma> (snd tw) \<and> (\<forall>tw'. tw, Bassign_inert sig exp dly \<Rightarrow>\<^sub>s tw' \<longrightarrow> Q tw')"
+    using wt by auto
+qed
+
+  
+fun wp3_fun :: "'signal tyenv \<Rightarrow> 'signal seq_stmt \<Rightarrow> 'signal assn2 \<Rightarrow> 'signal assn2" where
+
+  "wp3_fun \<Gamma> Bnull Q = (\<lambda>tw. Q tw \<and> wityping \<Gamma> (snd tw))"
+
+| "wp3_fun \<Gamma> (Bassign_trans sig exp dly) Q = (\<lambda>tw. wityping \<Gamma> (snd tw) \<and> Q(tw[sig, dly :=\<^sub>2 eval_world_raw2 tw exp]))"
+
+| "wp3_fun \<Gamma> (Bassign_inert sig exp dly) Q = (\<lambda>tw. wityping \<Gamma> (snd tw) \<and> Q(tw\<lbrakk>sig, dly :=\<^sub>2 eval_world_raw2 tw exp\<rbrakk>))"
+
+| "wp3_fun \<Gamma> (Bcase exp ((Explicit exp', ss) # choices)) Q = 
+        (\<lambda>tw. if eval_world_raw2 tw exp = eval_world_raw2 tw exp' then wp3_fun \<Gamma> ss Q tw  else wp3_fun \<Gamma> (Bcase exp choices) Q tw)"
+
+| "wp3_fun \<Gamma> (Bcase exp ((Others, ss) # choices)) Q = wp3 \<Gamma> ss Q"
+
+| "wp3_fun \<Gamma> (Bcase exp []) Q = (\<lambda>tw. Q tw \<and> wityping \<Gamma> (snd tw))"
+
+| "wp3_fun \<Gamma> (Bguarded g ss1 ss2) Q = (\<lambda>tw. if eval_world_raw2 tw g = Bv True then  wp3_fun \<Gamma> ss1 Q tw  else  wp3_fun \<Gamma> ss2 Q tw)"
+
+| "wp3_fun \<Gamma> (Bcomp ss1 ss2) Q = wp3_fun \<Gamma> ss1 (wp3_fun \<Gamma> ss2 Q)"
+
+lemma wp3_fun_eq_wp3:
+  assumes "seq_wt \<Gamma> ss" and "nonneg_delay ss"
+  shows "wp3_fun \<Gamma> ss Q = wp3 \<Gamma> ss Q"
+  using assms
+  apply (induction ss arbitrary: Q)
+  by (auto simp add: wp3_bnull wp3_bcomp wp3_bguarded wp3_assign_trans wp3_assign_inert wp3_bcase_empty wp3_bcase_others wp3_bcase_explicit seq_wt.intros)
+
+lemma wp3_fun_is_pre:
+  assumes "seq_wt \<Gamma> ss" and "nonneg_delay ss"
+  shows "\<Gamma> \<turnstile> [wp3_fun \<Gamma> ss Q] ss [Q]"
+  using assms
+proof (induction ss arbitrary:Q)
+  case (1 \<Gamma>)
+  then show ?case using wp3_bnull 
+    by (metis Conseq3 Null3 seq_wt.intros(1) wp3_fun_eq_wp3)
+next
+  case (2 \<Gamma> s1 s2)
+  then show ?case using wp3_fun_eq_wp3 wp3_bcomp 
+    by (metis Comp3 nonneg_delay.simps(2) wp3_fun.simps(8))
+next
+  case (3 \<Gamma> g s1 s2)
+  then show ?case using wp3_fun_eq_wp3 wp3_bguarded
+    by (smt Conseq3 If3 nonneg_delay.simps(3) seq_wt.intros(3) val.inject(1))
+next
+  case (4 \<Gamma> exp sig dly)
+  then show ?case using wp3_fun_eq_wp3 wp3_assign_trans
+    by (smt Conseq3 seq_hoare3.intros(2) wp3_fun.simps(2))
+next
+  case (5 \<Gamma> exp sig dly)
+  then show ?case  using wp3_fun_eq_wp3 wp3_assign_inert
+    by (smt Conseq3 seq_hoare3.intros(3) wp3_fun.simps(3))
+next
+  case (6 \<Gamma> exp ty)
+  then show ?case using wp3_fun_eq_wp3 wp3_bcase_empty
+    by (smt Bcase_empty_choices3 Conseq3 wp3_fun.simps(6))
+next
+  case (7 \<Gamma> exp ty ss choices)
+  hence "nonneg_delay ss"
+    by auto
+  hence IH: " \<Gamma> \<turnstile> [wp3_fun \<Gamma> ss Q] ss [Q]"
+    using 7(3) by auto
+  show ?case
+    apply (rule Conseq3[rotated])
+      apply (rule Bcase_others3)
+      apply (rule IH, simp)
+    by (simp add: "7.hyps"(2) \<open>nonneg_delay ss\<close> wp3_fun_eq_wp3)
+next
+  case (8 \<Gamma> exp ty exp' ss choices) 
+  hence " \<Gamma> \<turnstile> [wp3_fun \<Gamma> ss Q] ss [Q]" and  *:  " \<Gamma> \<turnstile> [wp3_fun \<Gamma> (Bcase exp choices) Q] Bcase exp choices [Q]"
+    by auto
+  hence IH1: "\<Gamma> \<turnstile> [\<lambda>tw. (if eval_world_raw2 tw exp = eval_world_raw2 tw exp' then wp3_fun \<Gamma> ss Q tw else wp3_fun \<Gamma> (Bcase exp choices) Q tw) \<and> eval_world_raw2 tw exp = eval_world_raw2 tw exp'] ss [Q]"
+    by (smt Conseq3)
+  have  IH2: "\<Gamma> \<turnstile> [\<lambda>tw. (if eval_world_raw2 tw exp = eval_world_raw2 tw exp' then wp3_fun \<Gamma> ss Q tw else wp3_fun \<Gamma> (Bcase exp choices) Q tw) \<and> eval_world_raw2 tw exp \<noteq> eval_world_raw2 tw exp'] Bcase exp choices [Q]"
+    using * by (smt Conseq3)
+  have swt: "seq_wt \<Gamma> (Bcase exp ((Explicit exp', ss) # choices))"
+    using 8  seq_wt.intros(8) by blast
+  have nss: "nonneg_delay ss" and not: "nonneg_delay (Bcase exp choices)"
+    using 8 by auto
+  show ?case
+    apply (rule Conseq3[rotated])
+      apply (rule Bcase_if3)
+    apply (rule IH1, rule IH2, simp)
+    unfolding wp3_fun_eq_wp3[OF swt 8(7)] wp3_bcase_explicit[OF swt 8(7)] 
+    wp3_fun_eq_wp3[OF 8(3) nss] wp3_fun_eq_wp3[OF 8(4) not] by auto
+qed
+
+definition
+conc_hoare_valid_wt :: "'signal tyenv \<Rightarrow>'signal assn2 \<Rightarrow> 'signal conc_stmt \<Rightarrow> 'signal assn2 \<Rightarrow> bool" ("(1_) \<Turnstile> \<lbrace>(1_)\<rbrace>/ (_)/ \<lbrace>(1_)\<rbrace>" 50)
+where "\<Gamma> \<Turnstile> \<lbrace>P\<rbrace> c \<lbrace>Q\<rbrace> \<longleftrightarrow>  (\<forall>tw tw'.  wityping \<Gamma> (snd tw) \<and> P tw \<and> (tw, c \<Rightarrow>\<^sub>c tw') \<longrightarrow> Q tw')"
+
+inductive
+  conc_hoare_wt :: "'signal tyenv \<Rightarrow> 'signal assn2 \<Rightarrow> 'signal conc_stmt \<Rightarrow> 'signal assn2 \<Rightarrow> bool"
+  ("(1_) \<turnstile> (\<lbrace>(1_)\<rbrace>/ (_)/ \<lbrace>(1_)\<rbrace>)" 50)
+  where
+   Single:  "\<Gamma> \<turnstile> [\<lambda>tw. P tw \<and> \<not> disjnt sl (event_of tw)] ss [Q] \<Longrightarrow> \<forall>tw. P tw \<and> disjnt sl (event_of tw) \<longrightarrow> Q tw
+    \<Longrightarrow> \<Gamma> \<turnstile> \<lbrace>P\<rbrace> process sl : ss \<lbrace>Q\<rbrace>"
+| Parallel:  "\<Gamma> \<turnstile> \<lbrace>P\<rbrace> cs\<^sub>1 \<lbrace>R\<rbrace> \<Longrightarrow> \<Gamma> \<turnstile> \<lbrace>R\<rbrace> cs\<^sub>2 \<lbrace>Q\<rbrace> \<Longrightarrow> conc_stmt_wf (cs\<^sub>1 || cs\<^sub>2) \<Longrightarrow> \<Gamma> \<turnstile> \<lbrace>P\<rbrace> cs\<^sub>1 || cs\<^sub>2 \<lbrace>Q\<rbrace>"
+| Parallel2: "\<Gamma> \<turnstile> \<lbrace>P\<rbrace> cs\<^sub>2 \<lbrace>R\<rbrace> \<Longrightarrow> \<Gamma> \<turnstile> \<lbrace>R\<rbrace> cs\<^sub>1 \<lbrace>Q\<rbrace> \<Longrightarrow> conc_stmt_wf (cs\<^sub>1 || cs\<^sub>2) \<Longrightarrow> \<Gamma> \<turnstile> \<lbrace>P\<rbrace> cs\<^sub>1 || cs\<^sub>2 \<lbrace>Q\<rbrace>"
+| Conseq': "\<lbrakk>\<forall>w. wityping \<Gamma> (snd w) \<and> P' w \<longrightarrow> P w; \<Gamma> \<turnstile> \<lbrace>P\<rbrace> c \<lbrace>Q\<rbrace>; \<forall>w. Q w \<longrightarrow> Q' w\<rbrakk> \<Longrightarrow> \<Gamma> \<turnstile> \<lbrace>P'\<rbrace> c \<lbrace>Q'\<rbrace>"
+| Conj2: "\<Gamma> \<turnstile> \<lbrace>P\<rbrace> s \<lbrace>Q1\<rbrace> \<Longrightarrow> \<Gamma> \<turnstile> \<lbrace>P\<rbrace> s \<lbrace>Q2\<rbrace> \<Longrightarrow> \<Gamma> \<turnstile> \<lbrace>P\<rbrace> s \<lbrace>\<lambda>tw. Q1 tw \<and> Q2 tw\<rbrace>"
+
+lemma parallel_valid:
+  assumes "\<Gamma> \<Turnstile> \<lbrace>P\<rbrace> c1 \<lbrace>R\<rbrace>" and "\<Gamma> \<Turnstile> \<lbrace>R\<rbrace> c2 \<lbrace>Q\<rbrace>" and "conc_stmt_wf (c1 || c2)"
+  assumes "nonneg_delay_conc (c1 || c2)"
+  assumes "conc_wt \<Gamma> (c1 || c2)"
+  shows "\<Gamma> \<Turnstile> \<lbrace>P\<rbrace> c1 || c2 \<lbrace>Q\<rbrace>"
+  unfolding conc_hoare_valid_wt_def
+proof rule+
+  fix tw tw':: "nat \<times> 'a worldline_init"
+  assume "wityping \<Gamma> (snd tw) \<and> P tw \<and> tw , c1 || c2 \<Rightarrow>\<^sub>c tw'"
+  hence "wityping \<Gamma> (snd tw)" and "P tw" and "tw, c1 || c2 \<Rightarrow>\<^sub>c tw'"
+    by auto
+  then obtain t \<sigma> \<gamma> \<theta> \<tau> def \<tau>' where des: "destruct_worldline tw = (t, \<sigma>, \<gamma>, \<theta>, def, \<tau>)" and
+    *: "t, \<sigma>, \<gamma>, \<theta>, def \<turnstile> <c1 || c2, \<tau>> \<longrightarrow>\<^sub>c \<tau>'" and w'_def: "worldline2 t \<sigma> \<theta> def \<tau>' = tw'" and
+    ci: "context_invariant t \<sigma> \<gamma> \<theta> def \<tau>"
+    using destruct_worldline_exist  by (smt world_conc_exec_cases worldline2_constructible)
+  have "\<And>s. non_stuttering (to_trans_raw_sig \<tau>) \<sigma> s"
+    using destruct_worldline_ensure_non_stuttering[OF des] by auto
+  obtain \<tau>1 where "b_conc_exec t \<sigma> \<gamma> \<theta> def c1 \<tau> \<tau>1"
+    using "*" by blast
+  hence ci1: "context_invariant t \<sigma> \<gamma> \<theta> def \<tau>1"
+    using b_conc_exec_preserves_context_invariant[OF _ ci] assms(4)  by auto
+  have "\<And>n. n \<le> t \<Longrightarrow> \<tau> n = 0"
+    using destruct_worldline_trans_zero_upto_now[OF des] by auto
+  have "\<forall>s. non_stuttering (to_trans_raw_sig \<tau>1) \<sigma> s"
+  proof
+    fix s
+    have "t, \<sigma>, \<gamma>, \<theta>, def \<turnstile> <c1, \<tau>> \<longrightarrow>\<^sub>c \<tau>1"
+      using \<open>t , \<sigma> , \<gamma> , \<theta>, def \<turnstile> <c1 , \<tau>> \<longrightarrow>\<^sub>c \<tau>1\<close> by blast
+    moreover have "non_stuttering (to_trans_raw_sig \<tau>) \<sigma> s"
+      by (simp add: \<open>\<And>s. non_stuttering (to_trans_raw_sig \<tau>) \<sigma> s\<close>)
+    moreover have "conc_stmt_wf c1" and "nonneg_delay_conc c1"
+      using assms by auto
+    ultimately show "non_stuttering (to_trans_raw_sig \<tau>1) \<sigma> s"
+      using b_conc_exec_preserves_non_stuttering[OF _ _ `\<And>n. n \<le> t \<Longrightarrow> \<tau> n = 0`]
+      by auto
+  qed
+  obtain \<tau>2 where "b_conc_exec t \<sigma> \<gamma> \<theta> def c2 \<tau> \<tau>2"
+    using "*" by blast
+  hence ci2: "context_invariant t \<sigma> \<gamma> \<theta> def \<tau>2"
+    using b_conc_exec_preserves_context_invariant[OF _ ci] assms(4) by auto
+  have \<tau>'_def: "b_conc_exec t \<sigma> \<gamma> \<theta> def c2 \<tau>1 \<tau>'"
+    using b_conc_exec_sequential[OF assms(3) * `t, \<sigma>, \<gamma>, \<theta>, def \<turnstile> <c1, \<tau>> \<longrightarrow>\<^sub>c \<tau>1`]
+    by auto
+  define tw1 where "tw1 = worldline2 t \<sigma> \<theta> def \<tau>1"
+  have "tw, c1 \<Rightarrow>\<^sub>c tw1"
+    using des \<open>t , \<sigma> , \<gamma> , \<theta>, def \<turnstile> <c1 , \<tau>> \<longrightarrow>\<^sub>c \<tau>1\<close> tw1_def world_conc_exec.intros by blast
+  hence "R tw1"
+    using assms(1) `P tw` `wityping \<Gamma> (snd tw)` unfolding conc_hoare_valid_wt_def   by presburger
+  have "conc_wt \<Gamma> c1" and "conc_stmt_wf c1" and "nonneg_delay_conc c1"
+    using `conc_wt \<Gamma> (c1 || c2)` `conc_stmt_wf (c1 || c2)` assms(4) by auto
+  hence "wityping \<Gamma> (snd tw1)"
+    using conc_stmt_preserve_wityping_hoare_semantic[OF `conc_wt \<Gamma> c1` `conc_stmt_wf c1`] `tw, c1 \<Rightarrow>\<^sub>c tw1`
+    unfolding conc_hoare_valid_def  using \<open>wityping \<Gamma> (snd tw)\<close> by presburger    
+  have "\<forall>s. non_stuttering (to_trans_raw_sig \<theta>) def s"
+    using des destruct_worldline_ensure_non_stuttering_hist_raw by blast
+  hence des2: "destruct_worldline tw1 = (t, \<sigma>, \<gamma>, \<theta>, def, \<tau>1)"
+    using destruct_worldline_correctness3[OF ci1 `\<forall>s. non_stuttering (to_trans_raw_sig \<tau>1) \<sigma> s`]
+    unfolding tw1_def by auto
+  moreover have "nonneg_delay_conc c2"
+    using assms(4) by auto
+  hence "tw1, c2 \<Rightarrow>\<^sub>c tw'"
+    using des2
+    apply (intro world_conc_exec.intros)
+      apply assumption
+     apply (rule \<tau>'_def)
+    apply (simp add: w'_def)
+    done
+  with `R tw1` show "Q tw'"
+    using assms(2) `wityping \<Gamma> (snd tw1)` unfolding conc_hoare_valid_wt_def 
+    by meson
+qed
+
+lemma soundness_conc_hoare:
+  assumes "\<Gamma> \<turnstile> \<lbrace>P\<rbrace> c \<lbrace>Q\<rbrace>"
+  assumes "conc_wt \<Gamma> c" and "conc_stmt_wf c" and "nonneg_delay_conc c"
+  shows "\<Gamma> \<Turnstile> \<lbrace>P\<rbrace> c \<lbrace>Q\<rbrace>"
+  using assms
+proof (induction rule:conc_hoare_wt.induct)
+  case (Single \<Gamma> P sl ss Q)
+  show ?case 
+    unfolding conc_hoare_valid_wt_def
+  proof (rule, rule, rule)
+    fix tw tw'
+    assume *: "wityping \<Gamma> (snd tw) \<and> P tw \<and> tw, process sl : ss \<Rightarrow>\<^sub>c tw'"
+    hence 0: "world_conc_exec_alt tw (process sl : ss) tw'"
+      using world_conc_exec_eq_world_conc_exec_alt[OF Single(4) Single(5)] by auto
+    have "disjnt sl (event_of tw) \<or> \<not> disjnt sl (event_of tw)"
+      by auto
+    moreover
+    { assume "disjnt sl (event_of tw)"
+      hence "tw' = tw"
+        using 0 
+        by (meson \<open>wityping \<Gamma> (snd tw) \<and> P tw \<and> tw , process sl : ss \<Rightarrow>\<^sub>c tw'\<close> world_conc_exec_deterministic world_conc_exec_disjnt)
+      hence "Q tw'"
+        using Single(2) * `disjnt sl (event_of tw)` by blast }
+    moreover
+    { assume "\<not> disjnt sl (event_of tw)"
+      hence "world_seq_exec_alt tw ss tw'"
+        using 0  by (metis "*" Single.prems(3) event_of_def nonneg_delay_conc.simps(1)
+        world_seq_exec_imp_world_seq_exec_alt wp_conc_def wp_conc_single wp_def) 
+      hence "tw, ss \<Rightarrow>\<^sub>s tw'"
+        using world_seq_exec_alt_imp_world_seq_exec Single(5)  nonneg_delay_conc.simps(1) by blast
+      moreover have "\<Gamma> \<Turnstile> [\<lambda>tw. P tw \<and> \<not> disjnt sl (event_of tw)] ss [Q]"
+        using seq_hoare3_soundness[OF Single(1)] Single(3) Single(5) by auto
+      ultimately have "Q tw'"
+        using `\<not> disjnt sl (event_of tw)` unfolding seq_hoare_valid2_wt_def  using "*" by blast }
+    ultimately show "Q tw'"
+      by auto
+  qed
+next
+  case (Parallel \<Gamma> P cs\<^sub>1 R cs\<^sub>2 Q)
+  then show ?case using parallel_valid 
+    by (metis conc_stmt_wf_def conc_wt_cases(2) distinct_append nonneg_delay_conc.simps(2) signals_from.simps(2))
+next
+  case (Parallel2 \<Gamma> P cs\<^sub>2 R cs\<^sub>1 Q)
+  hence "conc_stmt_wf cs\<^sub>1" and "conc_stmt_wf cs\<^sub>2"
+    by (simp add: conc_stmt_wf_def)+
+  moreover have "nonneg_delay_conc cs\<^sub>1" and "nonneg_delay_conc cs\<^sub>2"
+    using Parallel2 by auto
+  ultimately have cs2: " \<Gamma> \<Turnstile> \<lbrace>P\<rbrace> cs\<^sub>2 \<lbrace>R\<rbrace>" and cs1: " \<Gamma> \<Turnstile> \<lbrace>R\<rbrace> cs\<^sub>1 \<lbrace>Q\<rbrace>"
+    using Parallel2 by auto
+  have "conc_stmt_wf (cs\<^sub>2 || cs\<^sub>1)"
+    using Parallel2(3) unfolding conc_stmt_wf_def by auto
+  moreover have " nonneg_delay_conc (cs\<^sub>2 || cs\<^sub>1) "
+    using Parallel2(8) by auto 
+  moreover have " conc_wt \<Gamma> (cs\<^sub>2 || cs\<^sub>1)"
+    using Parallel2(6)  conc_wt.intros(2) by blast 
+  ultimately have "\<Gamma> \<Turnstile> \<lbrace>P\<rbrace> cs\<^sub>2 || cs\<^sub>1 \<lbrace>Q\<rbrace>"
+    using parallel_valid[OF cs2 cs1] by auto
+  thus ?case
+    using world_conc_exec_commute[OF _ _ Parallel2(3)]  unfolding conc_hoare_valid_wt_def
+    by (smt Parallel2.prems(2) parallel_comp_commute' world_conc_exec.intros world_conc_exec_alt_cases(2))
+next
+  case (Conseq' \<Gamma> P' P c Q Q')
+  then show ?case 
+    unfolding conc_hoare_valid_wt_def by metis
+next
+  case (Conj2 \<Gamma> P s Q1 Q2)
+  then show ?case by (simp add: conc_hoare_valid_wt_def)
+qed
+
+definition wp3_conc :: "'signal tyenv \<Rightarrow> 'signal conc_stmt \<Rightarrow> 'signal assn2 \<Rightarrow> 'signal assn2" where
+  "wp3_conc \<Gamma> cs Q = (\<lambda>tw. wityping \<Gamma> (snd tw) \<and> (\<forall>tw'. (tw, cs \<Rightarrow>\<^sub>c tw') \<longrightarrow> Q tw'))"
+
+lemma wp3_conc_single:
+  "wp3_conc \<Gamma> (process sl : ss) Q =
+  (\<lambda>tw. if disjnt sl (event_of tw) then Q tw \<and> wityping \<Gamma> (snd tw) else wp3 \<Gamma> ss Q tw)"
+  apply (rule ext)
+  unfolding wp3_conc_def wp3_def
+  by (smt conc_cases(1) event_of_def o_apply prod.sel(1) snd_conv world_conc_exec_alt_cases(1)
+  world_conc_exec_disjnt world_conc_exec_not_disjnt world_seq_exec.intros)
+
+lemma wp3_conc_single':
+  assumes "conc_wt \<Gamma> (process sl : ss)" and "nonneg_delay_conc (process sl : ss) "
+  shows "wp3_conc \<Gamma> (process sl : ss) Q =
+  (\<lambda>tw. if disjnt sl (event_of tw) then Q tw \<and> wityping \<Gamma> (snd tw) else wp3_fun \<Gamma> ss Q tw)"
+  unfolding wp3_conc_single using wp3_fun_eq_wp3 assms  by fastforce
+
+lemma exist_middle_worldline:
+  assumes "tw, cs \<Rightarrow>\<^sub>c tw'" and "cs = c1 || c2"
+  assumes "conc_stmt_wf cs" and "nonneg_delay_conc cs"
+  shows   "\<exists>tw_temp. tw, c1 \<Rightarrow>\<^sub>c tw_temp \<and> tw_temp, c2 \<Rightarrow>\<^sub>c tw'"
+  using assms
+proof (induction rule: world_conc_exec.induct)
+  case (1 tw t \<sigma> \<gamma> \<theta> def \<tau> c \<tau>' tw')
+  then obtain \<tau>_temp where \<tau>_temp: " t , \<sigma> , \<gamma> , \<theta>, def  \<turnstile> <c1 , \<tau>> \<longrightarrow>\<^sub>c \<tau>_temp"
+    by auto
+  then obtain tw_temp where "tw, c1 \<Rightarrow>\<^sub>c tw_temp" and "tw_temp = worldline2 t \<sigma> \<theta> def \<tau>_temp"
+    using 1  using world_conc_exec.intros by blast
+  have *: "t , \<sigma> , \<gamma> , \<theta>, def  \<turnstile> <c1 || c2, \<tau>> \<longrightarrow>\<^sub>c \<tau>'"
+    using 1 by auto
+  hence 2: "t , \<sigma> , \<gamma> , \<theta>, def  \<turnstile> <c2 , \<tau>_temp> \<longrightarrow>\<^sub>c \<tau>'" 
+    using b_conc_exec_sequential[OF _ * \<tau>_temp] 1 by auto
+  have "context_invariant t \<sigma> \<gamma> \<theta> def \<tau>"
+    using worldline2_constructible 1  by blast
+  hence "context_invariant t \<sigma> \<gamma> \<theta> def \<tau>_temp"
+    using \<tau>_temp b_conc_exec_preserves_context_invariant 
+    using "1.prems"(1) "1.prems"(3) nonneg_delay_conc.simps(2) by blast
+  have ns: " \<forall>s. non_stuttering (to_trans_raw_sig \<tau>) \<sigma> s"
+    using "1.hyps"(1) destruct_worldline_ensure_non_stuttering by blast
+  have "\<And>n. n \<le> t \<Longrightarrow> \<tau> n = 0"
+    using `context_invariant t \<sigma> \<gamma> \<theta> def \<tau>` unfolding context_invariant_def by auto
+  hence "\<forall>s. non_stuttering (to_trans_raw_sig \<tau>_temp) \<sigma> s"
+    using b_conc_exec_preserves_non_stuttering[OF \<tau>_temp _ _ ] ns 1(5-6) `c = c1 || c2`
+    by (simp add: conc_stmt_wf_def)
+  moreover have " \<forall>s. non_stuttering (to_trans_raw_sig \<theta>) def s"
+    using "1.hyps"(1) destruct_worldline_ensure_non_stuttering_hist_raw by blast
+  ultimately have "destruct_worldline tw_temp = (t, \<sigma>, \<gamma>, \<theta>, def, \<tau>_temp)"
+    using destruct_worldline_correctness2 
+    by (simp add: \<open>context_invariant t \<sigma> \<gamma> \<theta> def \<tau>_temp\<close> \<open>tw_temp = worldline2 t \<sigma> \<theta> def \<tau>_temp\<close>
+    destruct_worldline_correctness3)
+  hence "tw_temp, c2 \<Rightarrow>\<^sub>c tw'"
+    using 2 1(3)  using world_conc_exec.intros by blast
+  thus ?case
+    by (meson \<open>tw , c1 \<Rightarrow>\<^sub>c tw_temp\<close>)
+qed
+
+lemma wp3_conc_parallel:
+  assumes "conc_stmt_wf (cs1 || cs2)" and "nonneg_delay_conc (cs1 || cs2)"
+  assumes "conc_wt \<Gamma> (cs1 || cs2)"
+  shows "wp3_conc \<Gamma> (cs1 || cs2) Q =  wp3_conc \<Gamma> cs1 (wp3_conc \<Gamma> cs2 Q)"
+proof (rule ext, rule)
+  fix x
+  have "conc_stmt_wf cs1" and "conc_stmt_wf cs2"
+    using assms  by (simp add: conc_stmt_wf_def)+
+  have "nonneg_delay_conc cs1" and "nonneg_delay_conc cs2"
+    using assms by auto
+  assume "wp3_conc \<Gamma> (cs1 || cs2) Q x "
+  hence "(\<forall>tw'. x , cs1 || cs2 \<Rightarrow>\<^sub>c tw' \<longrightarrow> Q tw')" and "wityping \<Gamma> (snd x)"
+    unfolding wp3_conc_def by auto  
+  then show " wp3_conc \<Gamma> cs1 (wp3_conc \<Gamma> cs2 Q) x"
+    unfolding wp3_conc_def sym[OF world_conc_exec_eq_world_conc_exec_alt[OF assms(1-2)]]
+    sym[OF world_conc_exec_eq_world_conc_exec_alt[OF `conc_stmt_wf cs1` `nonneg_delay_conc cs1`]]
+    sym[OF world_conc_exec_eq_world_conc_exec_alt[OF `conc_stmt_wf cs2` `nonneg_delay_conc cs2`]]
+  proof (intro conjI, simp, intro allI, intro impI)
+    fix tw'
+    assume "\<forall>tw'. world_conc_exec_alt x (cs1 || cs2) tw' \<longrightarrow> Q tw'"
+    assume "wityping \<Gamma> (snd x)"
+    assume " world_conc_exec_alt x cs1 tw'"
+    hence "x, cs1 \<Rightarrow>\<^sub>c tw'"
+      using world_conc_exec_alt_imp_world_conc_exec[OF _ `conc_stmt_wf cs1` `nonneg_delay_conc cs1`]
+      by auto
+    moreover have "conc_wt \<Gamma> cs1"
+      using assms(3) by auto
+    hence "wityping \<Gamma> (snd tw')"
+      using conc_stmt_preserve_wityping_hoare_semantic[OF `conc_wt \<Gamma> cs1` `conc_stmt_wf cs1` `nonneg_delay_conc cs1`]
+      unfolding conc_hoare_valid_def using `wityping \<Gamma> (snd x)` `x, cs1 \<Rightarrow>\<^sub>c tw'`  by meson
+    moreover have "(\<forall>tw'a. world_conc_exec_alt tw' cs2 tw'a \<longrightarrow> Q tw'a)"
+      using \<open>\<forall>tw'. world_conc_exec_alt x (cs1 || cs2) tw' \<longrightarrow> Q tw'\<close> \<open>world_conc_exec_alt x cs1 tw'\<close> world_conc_exec_alt.intros(3) by blast
+    ultimately show "wityping \<Gamma> (snd tw') \<and> (\<forall>tw'a. world_conc_exec_alt tw' cs2 tw'a \<longrightarrow> Q tw'a)"
+      by auto
+  qed
+next
+  fix x
+  have "conc_stmt_wf cs1" and "conc_stmt_wf cs2"
+    using assms  by (simp add: conc_stmt_wf_def)+
+  have "nonneg_delay_conc cs1" and "nonneg_delay_conc cs2"
+    using assms by auto
+  assume "wp3_conc \<Gamma> cs1 (wp3_conc \<Gamma> cs2 Q) x"
+  hence "\<forall>tw tw'. x , cs1 \<Rightarrow>\<^sub>c tw \<and> tw , cs2 \<Rightarrow>\<^sub>c tw' \<longrightarrow> Q tw'" and "wityping \<Gamma> (snd x)"
+    unfolding wp3_conc_def by meson+
+  thus "wp3_conc \<Gamma> (cs1 || cs2) Q x"
+    unfolding wp3_conc_def sym[OF world_conc_exec_eq_world_conc_exec_alt[OF assms(1-2)]]
+  proof (intro conjI, simp, intro allI, intro impI)
+    fix tw'
+    assume "\<forall>tw tw'. x , cs1 \<Rightarrow>\<^sub>c tw \<and> tw , cs2 \<Rightarrow>\<^sub>c tw' \<longrightarrow> Q tw'"
+    assume " wityping \<Gamma> (snd x)"
+    assume "world_conc_exec_alt x (cs1 || cs2) tw'" 
+    hence "x, (cs1 || cs2) \<Rightarrow>\<^sub>c tw'"
+      using world_conc_exec_alt_imp_world_conc_exec[OF _ `conc_stmt_wf (cs1 || cs2)` `nonneg_delay_conc (cs1 || cs2)`]
+      by auto
+    obtain tw_temp where "x, cs1 \<Rightarrow>\<^sub>c tw_temp \<and> tw_temp, cs2 \<Rightarrow>\<^sub>c tw'"
+      using exist_middle_worldline  by (metis \<open>x , cs1 || cs2 \<Rightarrow>\<^sub>c tw'\<close> assms(1) assms(2))
+    thus "Q tw'"
+      by (simp add: \<open>\<forall>tw tw'. x , cs1 \<Rightarrow>\<^sub>c tw \<and> tw , cs2 \<Rightarrow>\<^sub>c tw' \<longrightarrow> Q tw'\<close>)
+  qed
+qed
+
+lemma wp3_conc_parallel2:
+  assumes "conc_stmt_wf (cs1 || cs2)" and "nonneg_delay_conc (cs1 || cs2)"
+  assumes "conc_wt \<Gamma> (cs1 || cs2)"
+  shows "wp3_conc \<Gamma> (cs1 || cs2) Q =  wp3_conc \<Gamma> cs2 (wp3_conc \<Gamma> cs1 Q)"
+proof (rule ext, rule)
+  fix x
+  have "conc_stmt_wf cs1" and "conc_stmt_wf cs2"
+    using assms  by (simp add: conc_stmt_wf_def)+
+  have "nonneg_delay_conc cs1" and "nonneg_delay_conc cs2"
+    using assms by auto
+  assume "wp3_conc \<Gamma> (cs1 || cs2) Q x"
+  hence "\<forall>tw'. x , cs1 || cs2 \<Rightarrow>\<^sub>c tw' \<longrightarrow> Q tw'" and "wityping \<Gamma> (snd x)"
+    unfolding wp3_conc_def by auto
+  thus" wp3_conc \<Gamma> cs2 (wp3_conc \<Gamma> cs1 Q) x"
+    unfolding wp3_conc_def sym[OF world_conc_exec_eq_world_conc_exec_alt[OF assms(1-2)]]
+    sym[OF world_conc_exec_eq_world_conc_exec_alt[OF `conc_stmt_wf cs1` `nonneg_delay_conc cs1`]]
+    sym[OF world_conc_exec_eq_world_conc_exec_alt[OF `conc_stmt_wf cs2` `nonneg_delay_conc cs2`]]
+  proof (intro conjI, simp, intro allI, intro impI)
+    fix tw'
+    have "conc_stmt_wf (cs2 || cs1)" and "nonneg_delay_conc (cs2 || cs1)"
+      using `conc_stmt_wf (cs1 || cs2)` `nonneg_delay_conc (cs1 || cs2)` unfolding conc_stmt_wf_def by  auto
+    assume "\<forall>tw'. world_conc_exec_alt x (cs1 || cs2) tw' \<longrightarrow> Q tw'"
+    hence  "\<forall>tw'. world_conc_exec_alt x (cs2 || cs1) tw' \<longrightarrow> Q tw'"
+      using  
+      world_conc_exec_alt_imp_world_conc_exec[OF _ `conc_stmt_wf (cs1 || cs2)` `nonneg_delay_conc (cs1 || cs2)`]
+      world_conc_exec_imp_world_conc_exec_alt[OF _ `conc_stmt_wf (cs2 || cs1)` `nonneg_delay_conc (cs2 || cs1)`]
+      by (metis \<open>\<And>tw. world_conc_exec tw cs1 = world_conc_exec_alt tw cs1\<close> \<open>\<And>tw. world_conc_exec tw
+      cs2 = world_conc_exec_alt tw cs2\<close> \<open>conc_stmt_wf (cs2 || cs1)\<close> \<open>nonneg_delay_conc (cs2 || cs1)\<close>
+      exist_middle_worldline world_conc_exec_alt.intros(4) world_conc_exec_alt_imp_world_conc_exec)
+    assume "wityping \<Gamma> (snd x)"
+    assume " world_conc_exec_alt x cs2 tw'"
+    hence "x, cs2 \<Rightarrow>\<^sub>c tw'"
+      using world_conc_exec_alt_imp_world_conc_exec[OF _ `conc_stmt_wf cs2` `nonneg_delay_conc cs2`]
+      by auto
+    moreover have "conc_wt \<Gamma> cs2"
+      using assms(3) by auto
+    hence "wityping \<Gamma> (snd tw')"
+      using conc_stmt_preserve_wityping_hoare_semantic[OF `conc_wt \<Gamma> cs2` `conc_stmt_wf cs2` `nonneg_delay_conc cs2`]
+      unfolding conc_hoare_valid_def using `wityping \<Gamma> (snd x)` `x, cs2 \<Rightarrow>\<^sub>c tw'`  by meson
+    moreover have "(\<forall>tw'a. world_conc_exec_alt tw' cs1 tw'a \<longrightarrow> Q tw'a)"
+      using \<open>\<forall>tw'. world_conc_exec_alt x (cs2 || cs1) tw' \<longrightarrow> Q tw'\<close> \<open>world_conc_exec_alt x cs2 tw'\<close> world_conc_exec_alt.intros(3) 
+      by blast
+    ultimately show "wityping \<Gamma> (snd tw') \<and> (\<forall>tw'a. world_conc_exec_alt tw' cs1 tw'a \<longrightarrow> Q tw'a)"
+      by auto
+  qed
+next
+  fix x
+  have "conc_stmt_wf cs1" and "conc_stmt_wf cs2"
+    using assms  by (simp add: conc_stmt_wf_def)+
+  have "nonneg_delay_conc cs1" and "nonneg_delay_conc cs2"
+    using assms by auto
+  have "conc_stmt_wf (cs2 || cs1)" and "nonneg_delay_conc (cs2 || cs1)"
+    using assms
+    by (metis conc_stmt_wf_def disjoint_iff_not_equal distinct_append signals_from.simps(2))
+       (simp add: \<open>nonneg_delay_conc cs1\<close> \<open>nonneg_delay_conc cs2\<close>)
+  assume "wp3_conc \<Gamma> cs2 (wp3_conc \<Gamma> cs1 Q) x"
+  hence "\<forall>tw tw'. x , cs2 \<Rightarrow>\<^sub>c tw \<and> tw , cs1 \<Rightarrow>\<^sub>c tw' \<longrightarrow> Q tw'" and "wityping \<Gamma> (snd x)"
+    unfolding wp3_conc_def  by metis+
+  hence "wp3_conc \<Gamma> (cs2 || cs1) Q x"
+    unfolding wp3_conc_def
+    using sym[OF world_conc_exec_eq_world_conc_exec_alt[OF `conc_stmt_wf (cs2 || cs1)` `nonneg_delay_conc (cs2 || cs1)`]]
+    by (metis \<open>conc_stmt_wf (cs2 || cs1)\<close> \<open>nonneg_delay_conc (cs2 || cs1)\<close> wp_conc_def wp_conc_parallel)
+  thus "wp3_conc \<Gamma> (cs1 || cs2) Q x"
+    unfolding wp3_conc_def by (smt assms(1) parallel_comp_commute' world_conc_exec.intros world_conc_exec_cases)
+qed
+  
+lemma wp3_conc_is_pre:
+  assumes "conc_stmt_wf cs" and "nonneg_delay_conc cs"
+  assumes "conc_wt \<Gamma> cs"
+  shows "\<Gamma> \<turnstile> \<lbrace>wp3_conc \<Gamma> cs Q\<rbrace> cs \<lbrace>Q\<rbrace>"
+  using assms
+proof (induction cs arbitrary:Q)
+  case (Bpar cs1 cs2)
+  hence "conc_stmt_wf cs1" and "conc_stmt_wf cs2" and "nonneg_delay_conc cs1" and "nonneg_delay_conc cs2"
+    by auto
+  hence "\<And>Q.  \<Gamma> \<turnstile> \<lbrace>wp3_conc \<Gamma> cs1 Q\<rbrace> cs1 \<lbrace>Q\<rbrace>" and "\<And>Q.  \<Gamma> \<turnstile> \<lbrace>wp3_conc \<Gamma> cs2 Q\<rbrace> cs2 \<lbrace>Q\<rbrace>"
+    using Bpar(1-2)  Bpar.prems(3) by blast+
+  then show ?case
+    unfolding wp3_conc_parallel[OF Bpar(3-4)]
+    by (metis Bpar.prems(1) Bpar.prems(3) \<open>\<And>\<Gamma> Q. conc_wt \<Gamma> (cs1 || cs2) \<Longrightarrow> wp3_conc \<Gamma> (cs1 || cs2) Q = wp3_conc \<Gamma> cs1 (wp3_conc \<Gamma> cs2 Q)\<close> conc_hoare_wt.Parallel)
+next
+  case (Bsingle sl ss)
+  hence "nonneg_delay ss"
+    by auto
+  then show ?case  unfolding wp3_conc_single
+    apply (intro Single)
+    by (smt Bsingle.prems(3) Conseq3 conc_wt_cases(1) wp3_fun_eq_wp3 wp3_fun_is_pre) auto
+qed
+
+definition
+sim_hoare_valid_wt :: "'signal tyenv \<Rightarrow> 'signal assn2 \<Rightarrow> 'signal conc_stmt \<Rightarrow> 'signal assn2 \<Rightarrow> bool" ("(1_) \<Turnstile>\<^sub>s \<lbrace>(1_)\<rbrace>/ (_)/ \<lbrace>(1_)\<rbrace>" 50)
+where "\<Gamma> \<Turnstile>\<^sub>s \<lbrace>P\<rbrace> cs \<lbrace>Q\<rbrace> \<longleftrightarrow> (\<forall>tw T tw'. wityping \<Gamma> (snd tw) \<and> P tw \<and> (tw, T, cs \<Rightarrow>\<^sub>S tw') \<longrightarrow> Q tw')"
+
+inductive
+  sim_hoare :: "'signal tyenv \<Rightarrow> 'signal assn2 \<Rightarrow> 'signal conc_stmt \<Rightarrow> 'signal assn2 \<Rightarrow> bool"
+  ("(1_) \<turnstile>\<^sub>s (\<lbrace>(1_)\<rbrace>/ (_)/ \<lbrace>(1_)\<rbrace>)" 50)
+  where
+While_Suc: "\<Gamma> \<turnstile> \<lbrace>\<lambda>tw. P tw\<rbrace> cs \<lbrace> \<lambda>tw. P (fst tw + 1, snd tw)\<rbrace>  \<Longrightarrow> \<Gamma> \<turnstile>\<^sub>s \<lbrace>P\<rbrace> cs \<lbrace>P\<rbrace>" |
+Conseq_sim: "\<forall>tw. wityping \<Gamma> (snd tw) \<and> P' tw \<longrightarrow> P tw \<Longrightarrow> \<Gamma> \<turnstile>\<^sub>s \<lbrace>P\<rbrace> cs \<lbrace>Q\<rbrace> \<Longrightarrow> \<forall>tw. Q tw \<longrightarrow> Q' tw \<Longrightarrow> \<Gamma> \<turnstile>\<^sub>s \<lbrace>P'\<rbrace> cs \<lbrace>Q'\<rbrace>"
+
+lemma while_soundness:
+  assumes "\<Gamma> \<Turnstile> \<lbrace>P\<rbrace> cs \<lbrace>\<lambda>tw. P (fst tw + 1, snd tw)\<rbrace>"
+  assumes "tw, T, cs \<Rightarrow>\<^sub>S tw'"
+  assumes "P tw"      
+  assumes "nonneg_delay_conc cs" and "conc_stmt_wf cs" and "conc_wt \<Gamma> cs" and "wityping \<Gamma> (snd tw)"
+  shows   "P tw'"
+proof -
+  have " world_sim_fin2 tw T cs tw'"
+    using only_context_matters_for_sim_fin2[OF assms(2) assms(4-5)] world_sim_fin_semi_equivalent[OF assms(2) _ assms(4-5)] 
+    by auto
+  hence "world_sim_fin2_alt tw T cs tw'"
+    unfolding world_sim_fin2_eq_world_sim_fin2_alt[OF assms(5) assms(4), THEN sym] by auto
+  thus ?thesis
+    using assms(1) assms(3-7)
+  proof (induction rule: world_sim_fin2_alt.inducts)
+    case (1 tw T cs tw2 tw3)
+    hence "tw, cs \<Rightarrow>\<^sub>c tw2"
+      unfolding world_conc_exec_eq_world_conc_exec_alt[OF ` conc_stmt_wf cs` `nonneg_delay_conc cs`]
+      by auto
+    hence "P (get_time tw2 + 1, snd tw2)"
+      using `\<Gamma> \<Turnstile> \<lbrace>\<lambda>tw. P tw\<rbrace> cs \<lbrace>\<lambda>tw. P (get_time tw + 1, snd tw)\<rbrace>` `fst tw < T` `P tw` `wityping \<Gamma> (snd tw)`
+      unfolding conc_hoare_valid_wt_def  by presburger
+    moreover have "wityping \<Gamma> (snd (get_time tw2 + 1, snd tw2))"
+      using `wityping \<Gamma> (snd tw)` conc_stmt_preserve_wityping_hoare_semantic[OF `conc_wt \<Gamma> cs` `conc_stmt_wf cs` `nonneg_delay_conc cs`]
+      unfolding conc_hoare_valid_def using `tw, cs\<Rightarrow>\<^sub>c tw2`  by (metis snd_conv)
+    ultimately show ?case 
+      using 1(4)[OF `\<Gamma> \<Turnstile> \<lbrace>\<lambda>tw. P tw\<rbrace> cs \<lbrace>\<lambda>tw. P (get_time tw + 1, snd tw)\<rbrace>`]
+      using "1.prems"(3) "1.prems"(4) ` conc_wt \<Gamma> cs` by auto
+  next
+    case (2 tw T cs)
+    then show ?case by auto
+  qed
+qed
+
+lemma conc_sim_soundness:
+  assumes "\<Gamma> \<turnstile>\<^sub>s \<lbrace>P\<rbrace> cs \<lbrace>Q\<rbrace>"
+  assumes "nonneg_delay_conc cs" and "conc_stmt_wf cs" and "conc_wt \<Gamma> cs"
+  shows "\<Gamma> \<Turnstile>\<^sub>s \<lbrace>P\<rbrace> cs \<lbrace>Q\<rbrace>"
+  using assms
+proof (induction rule:sim_hoare.induct)
+  case (While_Suc \<Gamma> P cs)
+  hence " \<Gamma> \<Turnstile> \<lbrace>\<lambda>tw. P tw\<rbrace> cs \<lbrace>\<lambda>tw. P (fst tw + 1, snd tw)\<rbrace>"
+    using soundness_conc_hoare[OF While_Suc(1)]  by auto
+  then show ?case 
+    unfolding sim_hoare_valid_wt_def using while_soundness4[OF _ _ _ While_Suc(2-3)]
+    by (metis (mono_tags, lifting) While_Suc.prems(1) While_Suc.prems(2) While_Suc.prems(3) while_soundness)
+next
+  case (Conseq_sim \<Gamma> P' P cs Q Q')
+  then show ?case 
+    by (smt sim_hoare_valid_wt_def)
+qed
+
+inductive
+  init_hoare :: "'signal tyenv \<Rightarrow> 'signal assn2 \<Rightarrow> 'signal conc_stmt \<Rightarrow> 'signal assn2 \<Rightarrow> bool"
+  ("(1_) \<turnstile>\<^sub>I (\<lbrace>(1_)\<rbrace>/ (_)/ \<lbrace>(1_)\<rbrace>)" 50)
+  where
+  SingleI:    "\<Gamma> \<turnstile> [P] ss [Q] \<Longrightarrow> \<Gamma> \<turnstile>\<^sub>I \<lbrace>P\<rbrace> process sl : ss \<lbrace>Q\<rbrace>"
+| ParallelI:  "\<Gamma> \<turnstile>\<^sub>I \<lbrace>P\<rbrace> cs\<^sub>1 \<lbrace>R\<rbrace> \<Longrightarrow> \<Gamma> \<turnstile>\<^sub>I \<lbrace>R\<rbrace> cs\<^sub>2 \<lbrace>Q\<rbrace> \<Longrightarrow> conc_stmt_wf (cs\<^sub>1 || cs\<^sub>2) \<Longrightarrow> \<Gamma> \<turnstile>\<^sub>I \<lbrace>P\<rbrace> cs\<^sub>1 || cs\<^sub>2 \<lbrace>Q\<rbrace>"
+| ParallelI2: "\<Gamma> \<turnstile>\<^sub>I \<lbrace>P\<rbrace> cs\<^sub>2 \<lbrace>R\<rbrace> \<Longrightarrow> \<Gamma> \<turnstile>\<^sub>I \<lbrace>R\<rbrace> cs\<^sub>1 \<lbrace>Q\<rbrace> \<Longrightarrow> conc_stmt_wf (cs\<^sub>1 || cs\<^sub>2) \<Longrightarrow> \<Gamma> \<turnstile>\<^sub>I \<lbrace>P\<rbrace> cs\<^sub>1 || cs\<^sub>2 \<lbrace>Q\<rbrace>"
+| ConseqI:    "\<lbrakk>\<forall>w. P' w \<longrightarrow> P w; \<Gamma> \<turnstile>\<^sub>I \<lbrace>P\<rbrace> cs \<lbrace>Q\<rbrace>; \<forall>w. Q w \<longrightarrow> Q' w\<rbrakk> \<Longrightarrow> \<Gamma> \<turnstile>\<^sub>I \<lbrace>P'\<rbrace> cs \<lbrace>Q\<rbrace>"
+| ConjI:      "\<Gamma> \<turnstile>\<^sub>I \<lbrace>P\<rbrace> cs \<lbrace>Q1\<rbrace> \<Longrightarrow> \<Gamma> \<turnstile>\<^sub>I \<lbrace>P\<rbrace> cs \<lbrace>Q2\<rbrace> \<Longrightarrow> \<Gamma> \<turnstile>\<^sub>I \<lbrace>P\<rbrace> cs \<lbrace>\<lambda>tw. Q1 tw \<and> Q2 tw\<rbrace>"
+
+definition
+  init_hoare_valid_wt :: "'signal tyenv \<Rightarrow> 'signal assn2 \<Rightarrow> 'signal conc_stmt \<Rightarrow> 'signal assn2 \<Rightarrow> bool" ("(1_) \<Turnstile>\<^sub>I \<lbrace>(1_)\<rbrace>/ (_)/ \<lbrace>(1_)\<rbrace>" 50)
+  where "\<Gamma> \<Turnstile>\<^sub>I \<lbrace>P\<rbrace> cs \<lbrace>Q\<rbrace> \<longleftrightarrow>  (\<forall>tw tw'.  wityping \<Gamma> (snd tw) \<and> P tw \<and> (tw, cs \<Rightarrow>\<^sub>I tw') \<longrightarrow> Q tw')"
+
+lemma exist_middle_worldline_init:
+  assumes "tw, cs \<Rightarrow>\<^sub>I tw'" and "cs = c1 || c2"
+  assumes "conc_stmt_wf cs" and "nonneg_delay_conc cs"
+  shows   "\<exists>tw_temp. tw, c1 \<Rightarrow>\<^sub>I tw_temp \<and> tw_temp, c2 \<Rightarrow>\<^sub>I tw'"
+  using assms
+proof (induction rule: world_init_exec.induct)
+  case (1 tw t \<sigma> \<gamma> \<theta> def \<tau> cs \<tau>' tw')
+  then obtain \<tau>_temp where \<tau>_temp: " init' t  \<sigma>  \<gamma>  \<theta> def c1  \<tau> \<tau>_temp"
+    by auto
+  then obtain tw_temp where "tw, c1 \<Rightarrow>\<^sub>I tw_temp" and "tw_temp = worldline2 t \<sigma> \<theta> def \<tau>_temp"
+    using 1  using world_init_exec.intros by blast
+  have *: "init' t  \<sigma>  \<gamma>  \<theta> def  (c1 || c2) \<tau> \<tau>'"
+    using 1 by auto
+  hence 2: "init' t \<sigma> \<gamma> \<theta> def c2 \<tau>_temp \<tau>'"
+    using init'_sequential[OF _ * \<tau>_temp] 1 by auto
+  have "context_invariant t \<sigma> \<gamma> \<theta> def \<tau>"
+    using worldline2_constructible 1  by blast
+  hence "context_invariant t \<sigma> \<gamma> \<theta> def \<tau>_temp"
+    using \<tau>_temp init'_preserves_context_invariant 
+    using "1.prems"(1) "1.prems"(3) nonneg_delay_conc.simps(2) by blast
+  have ns: " \<forall>s. non_stuttering (to_trans_raw_sig \<tau>) \<sigma> s"
+    using "1.hyps"(1) destruct_worldline_ensure_non_stuttering by blast
+  have "\<And>n. n \<le> t \<Longrightarrow> \<tau> n = 0"
+    using `context_invariant t \<sigma> \<gamma> \<theta> def \<tau>` unfolding context_invariant_def by auto
+  hence "\<forall>s. non_stuttering (to_trans_raw_sig \<tau>_temp) \<sigma> s"
+    using init'_preserves_non_stuttering[OF \<tau>_temp _ _ ] ns 1(5-6) `cs = c1 || c2`
+    by (simp add: conc_stmt_wf_def)
+  moreover have " \<forall>s. non_stuttering (to_trans_raw_sig \<theta>) def s"
+    using "1.hyps"(1) destruct_worldline_ensure_non_stuttering_hist_raw by blast
+  ultimately have "destruct_worldline tw_temp = (t, \<sigma>, \<gamma>, \<theta>, def, \<tau>_temp)"
+    using destruct_worldline_correctness2 
+    by (simp add: \<open>context_invariant t \<sigma> \<gamma> \<theta> def \<tau>_temp\<close> \<open>tw_temp = worldline2 t \<sigma> \<theta> def \<tau>_temp\<close>
+    destruct_worldline_correctness3)
+  hence "tw_temp, c2 \<Rightarrow>\<^sub>I tw'"
+    using 2 1(3)  using world_init_exec.intros by blast
+  thus ?case
+    by (meson \<open>tw , c1 \<Rightarrow>\<^sub>I tw_temp\<close>)
+qed
+
+lemma parallelI_valid:
+  assumes "\<Gamma> \<Turnstile>\<^sub>I \<lbrace>P\<rbrace> c1 \<lbrace>R\<rbrace>" and "\<Gamma> \<Turnstile>\<^sub>I \<lbrace>R\<rbrace> c2 \<lbrace>Q\<rbrace>" and "conc_stmt_wf (c1 || c2)"
+  assumes "nonneg_delay_conc (c1 || c2)" and "conc_wt \<Gamma> (c1 || c2)"
+  shows "\<Gamma> \<Turnstile>\<^sub>I \<lbrace>P\<rbrace> c1 || c2 \<lbrace>Q\<rbrace>"
+  unfolding init_hoare_valid_wt_def
+proof (rule, rule, rule)
+  fix tw tw'
+  assume *: "wityping \<Gamma> (snd tw) \<and> P tw \<and> tw , c1 || c2 \<Rightarrow>\<^sub>I tw'"
+  then obtain tw_temp where "tw, c1 \<Rightarrow>\<^sub>I tw_temp" and "tw_temp, c2 \<Rightarrow>\<^sub>I tw'"
+    using exist_middle_worldline_init[OF _ _ `conc_stmt_wf (c1 || c2)` `nonneg_delay_conc (c1 || c2)`]
+    by metis
+  hence "R tw_temp"
+    using assms(1) *  unfolding init_hoare_valid_wt_def by blast
+  have "wityping \<Gamma> (snd tw_temp)"
+    using init_preserve_wityping_semantic `conc_wt \<Gamma> (c1 || c2)` `conc_stmt_wf (c1 || c2)` `nonneg_delay_conc (c1 || c2)` *
+    `tw, c1 \<Rightarrow>\<^sub>I tw_temp` unfolding init_hoare_valid_def conc_stmt_wf_def 
+  proof -
+    assume "distinct (signals_from (c1 || c2))"
+    then show ?thesis
+      by (metis (no_types) "*" \<open>conc_wt \<Gamma> (c1 || c2)\<close> \<open>nonneg_delay_conc (c1 || c2)\<close> \<open>tw , c1 \<Rightarrow>\<^sub>I tw_temp\<close> conc_stmt_wf_def conc_wt_cases(2) distinct_append init_hoare_valid_def init_preserve_wityping_semantic nonneg_delay_conc.simps(2) signals_from.simps(2))
+  qed
+  thus "Q tw'"
+    using assms(2) `R tw_temp` `tw_temp, c2 \<Rightarrow>\<^sub>I tw'` unfolding init_hoare_valid_wt_def by blast
+qed
+  
+lemma soundness_init_hoare:
+  assumes "\<Gamma> \<turnstile>\<^sub>I \<lbrace>P\<rbrace> c \<lbrace>Q\<rbrace>"
+  assumes "conc_stmt_wf c" and "nonneg_delay_conc c" and "conc_wt \<Gamma> c"
+  shows   "\<Gamma> \<Turnstile>\<^sub>I \<lbrace>P\<rbrace> c \<lbrace>Q\<rbrace>"
+  using assms
+proof (induction rule:init_hoare.induct)
+  case (SingleI \<Gamma> P ss Q sl)
+  hence " \<Gamma> \<Turnstile> [P] ss [Q]"
+    using seq_hoare3_soundness by auto
+  then show ?case 
+    unfolding init_hoare_valid_wt_def seq_hoare_valid2_wt_def using world_seq_exec.intros by fastforce
+next
+  case (ParallelI \<Gamma> P cs\<^sub>1 R cs\<^sub>2 Q)
+  hence "\<Gamma> \<Turnstile>\<^sub>I \<lbrace>P\<rbrace> cs\<^sub>1 \<lbrace>R\<rbrace>" and "\<Gamma> \<Turnstile>\<^sub>I \<lbrace>R\<rbrace> cs\<^sub>2 \<lbrace>Q\<rbrace>"
+    unfolding conc_stmt_wf_def by auto
+  then show ?case 
+    using parallelI_valid 
+    by (metis ParallelI.prems(1) ParallelI.prems(2) ParallelI.prems(3))
+next
+  case (ParallelI2 \<Gamma> P cs\<^sub>2 R cs\<^sub>1 Q)
+  hence "\<Gamma> \<Turnstile>\<^sub>I \<lbrace>P\<rbrace> cs\<^sub>2 \<lbrace>R\<rbrace>" and "\<Gamma> \<Turnstile>\<^sub>I \<lbrace>R\<rbrace> cs\<^sub>1 \<lbrace>Q\<rbrace>"
+    unfolding conc_stmt_wf_def by auto
+  have "\<Gamma> \<Turnstile>\<^sub>I \<lbrace>P\<rbrace> cs\<^sub>2 || cs\<^sub>1 \<lbrace>Q\<rbrace>"
+    using parallelI_valid[OF `\<Gamma> \<Turnstile>\<^sub>I \<lbrace>P\<rbrace> cs\<^sub>2 \<lbrace>R\<rbrace>` `\<Gamma> \<Turnstile>\<^sub>I \<lbrace>R\<rbrace> cs\<^sub>1 \<lbrace>Q\<rbrace>`]
+    `conc_stmt_wf (cs\<^sub>1 || cs\<^sub>2)` ` nonneg_delay_conc (cs\<^sub>1 || cs\<^sub>2)` `conc_wt \<Gamma> (cs\<^sub>1 || cs\<^sub>2)`
+    unfolding conc_stmt_wf_def 
+    by (metis conc_wt.intros(2) conc_wt_cases(2) disjoint_iff_not_equal distinct_append
+    nonneg_delay_conc.simps(2) signals_from.simps(2))
+  thus ?case
+    using world_init_exec_commute
+    unfolding init_hoare_valid_wt_def 
+    by (smt ParallelI2.prems(1) parallelI_comp_commute' world_init_exec.intros world_init_exec_cases(2))
+next
+  case (ConseqI \<Gamma> P' P cs Q Q')
+  then show ?case 
+    by (smt init_hoare_valid_wt_def)
+next
+  case (ConjI \<Gamma> P cs Q1 Q2)
+  then show ?case 
+    by (simp add: init_hoare_valid_wt_def)
+qed
+
+definition wp3_init :: "'signal tyenv \<Rightarrow> 'signal conc_stmt \<Rightarrow> 'signal assn2 \<Rightarrow> 'signal assn2" where
+  "wp3_init \<Gamma> cs Q = (\<lambda>tw. wityping \<Gamma> (snd tw) \<and> (\<forall>tw'. (tw, cs \<Rightarrow>\<^sub>I tw') \<longrightarrow> Q tw'))"
+
+lemma wp3_init_single:
+  "wp3_init \<Gamma> (process sl : ss) Q = wp3 \<Gamma> ss Q"
+  apply (rule ext)
+  unfolding wp3_init_def wp3_def
+  by (smt init'_cases(1) world_init_exec_cases(1) world_init_exec_process world_seq_exec.intros)
+
+lemma wp3_init_parallel:
+  assumes "conc_stmt_wf (cs1 || cs2)" and "nonneg_delay_conc (cs1 || cs2)" and "conc_wt \<Gamma> (cs1 || cs2)"
+  shows   "wp3_init \<Gamma> (cs1 || cs2) Q = wp3_init \<Gamma> cs1 (wp3_init \<Gamma> cs2 Q)"
+  unfolding wp3_init_def
+proof (rule, rule, rule_tac[!] conjI, simp, rule, rule, rule)
+  fix tw tw'
+  assume *: "wityping \<Gamma> (snd tw) \<and> (\<forall>tw'. tw , cs1 || cs2 \<Rightarrow>\<^sub>I tw' \<longrightarrow> Q tw')"
+  assume "tw, cs1 \<Rightarrow>\<^sub>I tw'"
+  thus   "wityping \<Gamma> (snd tw')"
+    using init_preserve_wityping_semantic * unfolding init_hoare_valid_def 
+    by (metis (no_types) \<open>tw , cs1 \<Rightarrow>\<^sub>I tw'\<close> assms(1) assms(2) assms(3) conc_stmt_wf_def
+    conc_wt_cases(2) distinct_append init_hoare_valid_def init_preserve_wityping_semantic
+    nonneg_delay_conc.simps(2) signals_from.simps(2))
+  { fix tw2 
+    assume "tw', cs2 \<Rightarrow>\<^sub>I tw2"
+    hence "Q tw2"
+      using * `tw, cs1 \<Rightarrow>\<^sub>I tw'` 
+      by (metis assms(1) assms(2) conc_stmt_wf_def distinct_append nonneg_delay_conc.simps(2)
+      signals_from.simps(2) world_init_equality world_init_exec_alt.intros(2)) }
+  thus " \<forall>tw'a. tw' , cs2 \<Rightarrow>\<^sub>I tw'a \<longrightarrow> Q tw'a"
+    by auto
+next
+  fix tw
+  assume *: "wityping \<Gamma> (snd tw) \<and> (\<forall>tw'. tw , cs1 \<Rightarrow>\<^sub>I tw' \<longrightarrow> wityping \<Gamma> (snd tw') \<and> (\<forall>tw'a. tw' , cs2 \<Rightarrow>\<^sub>I tw'a \<longrightarrow> Q tw'a))"
+  thus "wityping \<Gamma> (snd tw)"
+    by auto
+  { fix tw' 
+    assume "tw, cs1 || cs2 \<Rightarrow>\<^sub>I tw'"
+    hence "Q tw'"
+      using *  by (meson assms(1) assms(2) exist_middle_worldline_init)  }
+  thus "\<forall>tw'. tw , cs1 || cs2 \<Rightarrow>\<^sub>I tw' \<longrightarrow> Q tw'"
+    by auto
+qed
+
+fun wp3_init_fun :: "'signal tyenv \<Rightarrow> 'signal conc_stmt \<Rightarrow> 'signal assn2 \<Rightarrow> 'signal assn2" where
+  "wp3_init_fun \<Gamma> (process sl : ss) Q = wp3 \<Gamma> ss Q"
+| "wp3_init_fun \<Gamma> (cs1 || cs2) Q = wp3_init_fun \<Gamma> cs1 (wp3_init_fun \<Gamma> cs2 Q)"
+
+lemma wp3_init_fun_is_wp3_init:
+  assumes "conc_stmt_wf cs" and "nonneg_delay_conc cs" and "conc_wt \<Gamma> cs"
+  shows   "wp3_init_fun \<Gamma> cs Q = wp3_init \<Gamma> cs Q"
+  using assms
+  apply (induction cs arbitrary: Q)
+  using wp3_init_parallel 
+  apply (metis conc_stmt_wf_def conc_wt_cases(2) distinct_append nonneg_delay_conc.simps(2) signals_from.simps(2) wp3_init_fun.simps(2))
+  by (simp add: wp3_init_single)
+
+definition init_sim2_valid_wt :: "'signal tyenv \<Rightarrow> 'signal assn2 \<Rightarrow> 'signal conc_stmt \<Rightarrow> 'signal assn2 \<Rightarrow> bool" where
+  "init_sim2_valid_wt \<Gamma> P cs Q = (\<forall>tw tw'. wityping \<Gamma> (snd tw) \<and> P tw \<and> init_sim2 tw cs tw' \<longrightarrow> Q tw')"
+
+inductive
+  init_sim2_hoare_wt :: "'signal tyenv \<Rightarrow> 'signal assn2 \<Rightarrow> 'signal conc_stmt \<Rightarrow> 'signal assn2 \<Rightarrow> bool" where
+AssignI_suc: "\<Gamma> \<turnstile>\<^sub>I \<lbrace>P\<rbrace> cs \<lbrace>\<lambda>tw. Q (fst tw + 1, snd tw)\<rbrace>  \<Longrightarrow> init_sim2_hoare_wt \<Gamma> P cs Q" |
+ConseqI_suc_sim: "\<forall>tw. P' tw \<longrightarrow> P tw \<Longrightarrow> init_sim2_hoare_wt \<Gamma> P cs Q \<Longrightarrow> \<forall>tw. Q tw \<longrightarrow> Q' tw \<Longrightarrow> init_sim2_hoare_wt \<Gamma> P' cs Q'" |
+ConjI_suc_sim: "init_sim2_hoare_wt \<Gamma> P cs Q1 \<Longrightarrow> init_sim2_hoare_wt \<Gamma> P cs Q2 \<Longrightarrow> init_sim2_hoare_wt \<Gamma> P cs (\<lambda>tw. Q1 tw \<and> Q2 tw)"
+
+lemma init_sim2_hoare_wt_soundness:
+  assumes "init_sim2_hoare_wt \<Gamma> P cs Q"
+  assumes "conc_stmt_wf cs" and "nonneg_delay_conc cs" and "conc_wt \<Gamma> cs"
+  shows "init_sim2_valid_wt \<Gamma> P cs Q"
+  using assms
+proof (induction rule:init_sim2_hoare_wt.induct)
+  case (AssignI_suc \<Gamma> P cs Q)
+  have *: "\<Gamma> \<Turnstile>\<^sub>I \<lbrace>P\<rbrace> cs \<lbrace>\<lambda>tw. Q (fst tw + 1, snd tw)\<rbrace>"
+    using soundness_init_hoare[OF AssignI_suc] by auto
+  { fix tw tw'
+    assume "P tw"
+    assume "wityping \<Gamma> (snd tw)"
+    assume "tw, cs \<Rightarrow>\<^sub>I tw'"
+    hence "Q (fst tw' + 1, snd tw')" (is ?imp1)
+      using * \<open>P tw\<close> `wityping \<Gamma> (snd tw)` unfolding init_hoare_valid_wt_def by blast
+    have "init_sim2 tw cs (fst tw' + 1, snd tw')" (is ?imp2)
+      using \<open>tw, cs \<Rightarrow>\<^sub>I tw'\<close>   using init_sim2.intros by blast
+    hence "?imp1 \<and> ?imp2"
+      using \<open>?imp1\<close> by auto }
+  then show ?case
+    unfolding init_sim2_valid_wt_def by auto
+next
+  case (ConseqI_suc_sim \<Gamma> P' P cs Q Q')
+  then show ?case
+    by (smt init_sim2_valid_wt_def)
+next
+  case (ConjI_suc_sim \<Gamma> P cs Q1 Q2)
+  then show ?case   by (simp add: init_sim2_valid_wt_def)
+qed
+
+lemma init_sim2_preserves_wityping:
+  assumes "init_sim2 tw cs tw'" and "conc_wt \<Gamma> cs" and "conc_stmt_wf cs" and "nonneg_delay_conc cs"
+  assumes "wityping \<Gamma> (snd tw)"
+  shows   "wityping \<Gamma> (snd tw')"
+  using assms
+proof (induction cs arbitrary: tw tw')
+  case (Bpar cs1 cs2)
+  then obtain tw2 where "tw, (cs1 || cs2) \<Rightarrow>\<^sub>I tw2" and "tw' = (fst tw2 + 1, snd tw2)"
+    by (meson init_sim2.cases)
+  then obtain tw_temp where "tw, cs1 \<Rightarrow>\<^sub>I tw_temp" and "tw_temp, cs2 \<Rightarrow>\<^sub>I tw2"
+    by (meson Bpar.prems(3) Bpar.prems(4) exist_middle_worldline_init)
+  hence "init_sim2 tw cs1 (fst tw_temp + 1, snd tw_temp)"
+    using init_sim2.intros by blast
+  note IH = Bpar(1)[OF this]
+  hence " wityping \<Gamma> (snd tw_temp)"
+    using Bpar unfolding conc_stmt_wf_def by auto
+  have "init_sim2 tw_temp cs2 tw'"
+    using `tw_temp, cs2 \<Rightarrow>\<^sub>I tw2` 
+    using \<open>tw' = (get_time tw2 + 1, snd tw2)\<close> init_sim2.intros by blast
+  note IH2 = Bpar(2)[OF this]
+  thus "wityping \<Gamma> (snd tw')"
+    using Bpar `wityping \<Gamma> (snd tw_temp)` unfolding conc_stmt_wf_def by auto    
+next
+  case (Bsingle sl ss)
+  then obtain tw2 where *: "tw, process sl : ss \<Rightarrow>\<^sub>I tw2" and "tw' = (fst tw2 + 1, snd tw2)"
+    by (meson init_sim2.cases)
+  have "seq_wt \<Gamma> ss" using Bsingle by auto
+  hence "wityping \<Gamma> (snd tw2)"
+    using * VHDL_Hoare_Complete.soundness_init_hoare[OF single_conc_stmt_preserve_wityping_init_hoare[OF `seq_wt \<Gamma> ss`]]
+    Bsingle(3-) unfolding init_hoare_valid_def  by meson
+  thus ?case
+    using `tw' = (fst tw2 + 1 , snd tw2)` by auto
+qed
+
+lemma grand_correctness:
+  assumes "sim_fin2 w (i + 1) cs tw'" and "wityping \<Gamma> w"
+  assumes "conc_stmt_wf cs" and "conc_wt \<Gamma> cs" and "nonneg_delay_conc cs"
+  assumes "\<Gamma> \<turnstile>\<^sub>s \<lbrace>Inv\<rbrace> cs \<lbrace>Inv\<rbrace>"
+  assumes "init_sim2_hoare_wt \<Gamma> (\<lambda>tw. fst tw = 0) cs Inv"
+  shows   "Inv tw'"
+proof -
+  obtain tw where "init_sim2 (0, w) cs tw" and  "tw, i + 1, cs \<Rightarrow>\<^sub>S tw'"
+    using sim_fin2.cases[OF `sim_fin2 w (i + 1) cs tw'`]  by metis
+  hence "i + 1 = fst tw'"
+    using world_maxtime_lt_fst_tres  by blast
+  have "wityping \<Gamma> (snd tw)"
+    using init_sim2_preserves_wityping 
+    by (metis \<open>init_sim2 (0, w) cs tw\<close> assms(2-5) snd_conv)
+  have "init_sim2_valid_wt \<Gamma> (\<lambda>tw. fst tw = 0) cs Inv"
+    using init_sim2_hoare_wt_soundness[OF assms(7)] assms(2-5)  by auto
+  hence "Inv tw"
+    using \<open>init_sim2 (0, w) cs tw\<close> fst_conv assms(2) unfolding init_sim2_valid_wt_def
+    by (metis snd_conv)    
+  moreover have "\<Gamma> \<Turnstile>\<^sub>s \<lbrace>Inv\<rbrace> cs \<lbrace>Inv\<rbrace>"
+    using conc_sim_soundness[OF assms(6)] assms(2-5) by auto
+  ultimately have "Inv tw'"
+    using \<open>tw, i + 1, cs \<Rightarrow>\<^sub>S tw'\<close> `wityping \<Gamma> (snd tw)` unfolding sim_hoare_valid_wt_def 
+    by blast
+  thus ?thesis
+    by auto
+qed
+
+lemma grand_correctness2:
+  assumes "sim_fin2 w endtime cs tw'" and "wityping \<Gamma> w"
+  assumes "conc_stmt_wf cs" and "conc_wt \<Gamma> cs" and "nonneg_delay_conc cs"
+  assumes "\<Gamma> \<turnstile>\<^sub>s \<lbrace>Inv\<rbrace> cs \<lbrace>Inv\<rbrace>"
+  assumes "Q (0, w)"
+  assumes "init_sim2_hoare_wt \<Gamma> (\<lambda>tw. fst tw = 0 \<and> Q tw) cs Inv"
+  shows   "Inv tw'"
+proof -
+  obtain tw where "init_sim2 (0, w) cs tw" and  "tw, endtime, cs \<Rightarrow>\<^sub>S tw'"
+    using sim_fin2.cases[OF `sim_fin2 w endtime cs tw'`]  by metis
+  hence "endtime = fst tw'"
+    using world_maxtime_lt_fst_tres  by blast  
+  have "wityping \<Gamma> (snd tw)"
+    using init_sim2_preserves_wityping 
+    by (metis \<open>init_sim2 (0, w) cs tw\<close> assms(2-5) snd_conv)  
+  have "init_sim2_valid_wt \<Gamma> (\<lambda>tw. fst tw = 0 \<and> Q tw) cs Inv"
+    using init_sim2_hoare_wt_soundness[OF assms(8)] assms(2-5)  by auto
+  hence "Inv tw"
+    using \<open>init_sim2 (0, w) cs tw\<close> fst_conv assms(2) unfolding init_sim2_valid_wt_def
+    by (metis assms(7) snd_conv)
+  moreover have "\<Gamma> \<Turnstile>\<^sub>s \<lbrace>Inv\<rbrace> cs \<lbrace>Inv\<rbrace>"
+    using conc_sim_soundness[OF assms(6)] assms(2-5) by auto
+  ultimately have "Inv tw'"
+    using \<open>tw, endtime, cs \<Rightarrow>\<^sub>S tw'\<close> `wityping \<Gamma> (snd tw)` unfolding sim_hoare_valid_wt_def 
+    by blast
+  thus ?thesis
+    by auto
+qed
 
 end
