Decoder_Typed.thy
@@ -1,0 +1,296 @@
+(*
+ * Copyright 2019, NTU
+ *
+ * This software may be distributed and modified according to the terms of
+ * the BSD 2-Clause license. Note that NO WARRANTY is provided.
+ * See "LICENSE_BSD2.txt" for details.
+ *
+ *  Author: Albert Rizaldi, NTU Singapore
+ *)
+
+theory Decoder_Typed
+  imports VHDL_Hoare_Typed
+begin
+
+datatype sig = IN | OUT
+
+abbreviation dec_list :: "(sig choices \<times> sig seq_stmt) list" where
+  "dec_list \<equiv>
+[ (Explicit (Bliteral Neu (to_bl (0b00 :: 2 word))), Bassign_trans OUT (Bliteral Neu (to_bl (0x1:: 4 word))) 1)
+, (Explicit (Bliteral Neu (to_bl (0b01 :: 2 word))), Bassign_trans OUT (Bliteral Neu (to_bl (0x2:: 4 word))) 1)
+, (Explicit (Bliteral Neu (to_bl (0b10 :: 2 word))), Bassign_trans OUT (Bliteral Neu (to_bl (0x4:: 4 word))) 1)
+, (Explicit (Bliteral Neu (to_bl (0b11 :: 2 word))), Bassign_trans OUT (Bliteral Neu (to_bl (0x8:: 4 word))) 1)
+]"
+
+definition dec :: "sig conc_stmt" where
+  "dec = process {IN} : Bcase (Bsig IN) dec_list"
+
+lemma potential_tyenv:
+  assumes "seq_wt \<Gamma> (Bcase (Bsig IN) dec_list)"
+  shows   "\<Gamma> IN = Lty Neu 2 \<and> \<Gamma> OUT = Lty Neu 4"
+proof (rule seq_wt_cases_bcase[OF assms, rotated 2])
+  fix ty exp' ss choices
+  assume "bexp_wt \<Gamma> (Bsig IN) ty"
+  assume "bexp_wt \<Gamma> exp' ty"
+  assume "seq_wt \<Gamma> ss"
+  assume "seq_wt \<Gamma> (Bcase (Bsig IN) choices)"
+  assume "dec_list = ((Explicit exp', ss) # choices)"
+  hence "exp' = Bliteral Neu (to_bl (0b00 :: 2 word))" and "choices = tl dec_list" and
+        ss_def: "ss = Bassign_trans OUT (Bliteral Neu (to_bl (0x1 :: 4 word))) 1"
+    by auto
+  hence 0: "bexp_wt \<Gamma> (Bliteral Neu (to_bl (0b000 :: 2 word))) ty"
+    using \<open>bexp_wt \<Gamma> exp' ty\<close> by auto
+  have "ty = Lty Neu 2"
+    by (rule bexp_wt_cases_lit[OF 0]) auto
+  with \<open>bexp_wt \<Gamma> (Bsig IN) ty\<close> have "\<Gamma> IN = Lty Neu 2"
+    by (metis bexp_wt_cases(9))
+  hence 1: "seq_wt \<Gamma> (Bassign_trans OUT (Bliteral Neu (to_bl (0x1 :: 4 word))) 1)"
+    using \<open>seq_wt \<Gamma> ss\<close> unfolding ss_def by auto
+  have "\<Gamma> OUT = Lty Neu 4"
+    apply (rule seq_wt_cases(4)[OF 1])
+    apply (erule bexp_wt_cases_lit)
+    by auto
+  thus ?thesis
+    using \<open>\<Gamma> IN = Lty Neu 2\<close> by auto
+qed auto
+
+abbreviation "lof_wline tw sig t \<equiv> lval_of (wline_of tw sig t)"
+
+locale decoder =
+  fixes \<Gamma> :: "sig tyenv"
+  assumes tyin: "\<Gamma> IN =  Lty Neu 2" and tyout: "\<Gamma> OUT = Lty Neu 4"
+begin
+
+definition dec_inv :: "sig assn2" where
+  "dec_inv \<equiv> \<lambda>tw. bl_to_bin (lof_wline tw OUT (fst tw)) = 2 ^ nat (bl_to_bin (lof_wline tw IN (fst tw - 1)))"
+
+definition dec_inv2 :: "sig assn2" where
+  "dec_inv2 \<equiv> \<lambda>tw. disjnt {IN} (event_of tw) \<longrightarrow> (\<forall>i > fst tw.  lof_wline tw OUT i = lof_wline tw OUT (fst tw))"
+
+abbreviation "ntime tw \<equiv> next_time_world tw"
+
+lemma one_encoding:
+  "to_bl (1 :: 2 word) = [False, True]"
+  by eval
+
+lemma conc_stmt_wf_dec:
+  "conc_stmt_wf dec"
+  unfolding dec_def conc_stmt_wf_def by auto  
+
+lemma nonneg_delay_conc_dec:
+  "nonneg_delay_conc dec"
+  unfolding dec_def by auto
+
+lemma nonneg_delay_conc_dec':
+  "nonneg_delay_conc (process {IN} : Bcase (Bsig IN) dec_list)"
+  using nonneg_delay_conc_dec unfolding dec_def by auto
+
+lemma len4:
+  "length (to_bl (n :: 4 word)) = 4"
+  by simp
+
+lemma len2:
+  "length (to_bl (n :: 2 word)) = 2"
+  by simp
+
+lemma seq_wt_dec:
+  "seq_wt \<Gamma> (Bcase (Bsig IN) dec_list)"
+  using tyin tyout 
+  by (metis bexp_wt.intros(26) bexp_wt.intros(3) len2 len4 seq_wt.intros(4) seq_wt.intros(6)
+  seq_wt.intros(8) tyin tyout)
+
+lemma conc_wt_dec:
+  "conc_wt \<Gamma> dec"
+  unfolding dec_def using seq_wt_dec conc_wt.intros(1) by blast 
+  
+lemma conc_wt_dec':
+  "conc_wt \<Gamma> ( process {IN} : Bcase (Bsig IN) dec_list)"
+  using conc_wt_dec unfolding dec_def by auto
+
+lemma one_encoding4:
+  "to_bl (1 :: 4 word) = [False, False, False, True]"
+  by eval
+
+lemma case0:
+  assumes "eval_world_raw2 tw (Bsig IN) = eval_world_raw2 tw (Bliteral Neu (to_bl (0 :: 2 word)))"
+  defines "v \<equiv> eval_world_raw2 tw (Bliteral Neu (to_bl (1 :: 4 word)))"
+  defines "tw' \<equiv> tw[ OUT, 1 :=\<^sub>2 v]"
+  assumes "wityping \<Gamma> (snd tw)"
+  shows   "dec_inv (fst tw' + 1, snd tw')"
+proof -
+  have "lof_wline tw' OUT (fst tw + 1) = lval_of v"
+    unfolding tw'_def worldline_upd2_def worldline_upd_def by auto
+  also have "... = [False, False, False, True]"
+    using one_encoding4 unfolding v_def by auto
+  finally have *: "bl_to_bin (lof_wline tw' OUT (fst tw + 1)) = 1"
+    by simp eval
+  have "lof_wline tw' IN (fst tw) = lof_wline tw IN (fst tw)"
+    unfolding tw'_def worldline_upd2_def worldline_upd_def by auto
+  also have "... = [False, False]"
+    using assms(1) by auto
+  finally have "bl_to_bin (lof_wline tw' IN (fst tw)) = 0"
+    by simp 
+  thus ?thesis
+    using * unfolding dec_inv_def  by (simp add: tw'_def)
+qed
+
+lemma case1:
+  assumes "eval_world_raw2 tw (Bsig IN) = eval_world_raw2 tw (Bliteral Neu (to_bl (1 :: 2 word)))"
+  defines "v \<equiv> eval_world_raw2 tw (Bliteral Neu (to_bl (2 :: 4 word)))"
+  defines "tw' \<equiv> tw[ OUT, 1 :=\<^sub>2 v]"
+  assumes "wityping \<Gamma> (snd tw)"
+  shows   "dec_inv (fst tw' + 1, snd tw')"
+proof -
+  have "lof_wline tw' OUT (fst tw + 1) = lval_of v"
+    unfolding tw'_def worldline_upd2_def worldline_upd_def by auto
+  also have "... = [False, False, True, False]"
+    using one_encoding4 unfolding v_def by auto
+  finally have *: "bl_to_bin (lof_wline tw' OUT (fst tw + 1)) = 2"
+    by simp eval
+  have "lof_wline tw' IN (fst tw) = lof_wline tw IN (fst tw)"
+    unfolding tw'_def worldline_upd2_def worldline_upd_def by auto
+  also have "... = [False, True]"
+    using assms(1) by auto eval
+  finally have "bl_to_bin (lof_wline tw' IN (fst tw)) = 1"
+    by simp eval
+  thus ?thesis
+    using * unfolding dec_inv_def  by (simp add: tw'_def)
+qed
+
+lemma case2:
+  assumes "eval_world_raw2 tw (Bsig IN) = eval_world_raw2 tw (Bliteral Neu (to_bl (2 :: 2 word)))"
+  defines "v \<equiv> eval_world_raw2 tw (Bliteral Neu (to_bl (4 :: 4 word)))"
+  defines "tw' \<equiv> tw[ OUT, 1 :=\<^sub>2 v]"
+  assumes "wityping \<Gamma> (snd tw)"
+  shows   "dec_inv (fst tw' + 1, snd tw')"
+proof -
+  have "lof_wline tw' OUT (fst tw + 1) = lval_of v"
+    unfolding tw'_def worldline_upd2_def worldline_upd_def by auto
+  also have "... = [False, True, False, False]"
+    using one_encoding4 unfolding v_def by auto
+  finally have *: "bl_to_bin (lof_wline tw' OUT (fst tw + 1)) = 4"
+    by simp eval
+  have "lof_wline tw' IN (fst tw) = lof_wline tw IN (fst tw)"
+    unfolding tw'_def worldline_upd2_def worldline_upd_def by auto
+  also have "... = [True, False]"
+    using assms(1) by auto
+  finally have "bl_to_bin (lof_wline tw' IN (fst tw)) = 2"
+    by simp eval
+  thus ?thesis
+    using * unfolding dec_inv_def  by (simp add: tw'_def)
+qed
+
+lemma case3:
+  assumes "eval_world_raw2 tw (Bsig IN) = eval_world_raw2 tw (Bliteral Neu (to_bl (3 :: 2 word)))"
+  defines "v \<equiv> eval_world_raw2 tw (Bliteral Neu (to_bl (8 :: 4 word)))"
+  defines "tw' \<equiv> tw[ OUT, 1 :=\<^sub>2 v]"
+  assumes "wityping \<Gamma> (snd tw)"
+  shows   "dec_inv (fst tw' + 1, snd tw')"
+proof -
+  have "lof_wline tw' OUT (fst tw + 1) = lval_of v"
+    unfolding tw'_def worldline_upd2_def worldline_upd_def by auto
+  also have "... = [True, False, False, False]"
+    using one_encoding4 unfolding v_def by auto
+  finally have *: "bl_to_bin (lof_wline tw' OUT (fst tw + 1)) = 8"
+    by simp eval
+  have "lof_wline tw' IN (fst tw) = lof_wline tw IN (fst tw)"
+    unfolding tw'_def worldline_upd2_def worldline_upd_def by auto
+  also have "... = [True, True]"
+    using assms(1) by auto
+  finally have "bl_to_bin (lof_wline tw' IN (fst tw)) = 3"
+    by simp eval
+  thus ?thesis
+    using * unfolding dec_inv_def  by (simp add: tw'_def)
+qed
+
+lemma dec_inv2_next_time:
+  fixes tw v
+  defines "tw' \<equiv> tw[OUT, 1 :=\<^sub>2 v]"
+  shows   "dec_inv2 (fst tw' + 1, snd tw')"
+  unfolding dec_inv2_def tw'_def worldline_upd2_def worldline_upd_def by auto
+
+lemma dec_conc_hoare:
+  "\<And>tw. dec_inv tw \<and> dec_inv2 tw \<and> disjnt {IN} (event_of tw) \<Longrightarrow> dec_inv (fst tw + 1, snd tw)"
+proof -
+  fix tw
+  assume "dec_inv tw \<and> dec_inv2 tw \<and> disjnt {IN} (event_of tw)"
+  hence "dec_inv tw" and "dec_inv2 tw" and "disjnt {IN} (event_of tw)"
+    by auto
+  have "lof_wline tw OUT (fst tw + 1) = lof_wline tw OUT (fst tw)"
+    using `dec_inv2 tw` `disjnt {IN} (event_of tw)` unfolding dec_inv2_def by auto 
+  also have "bl_to_bin ... = 2 ^ nat (bl_to_bin (lof_wline tw IN (get_time tw - 1)))"
+    using `dec_inv tw` unfolding dec_inv_def by auto
+  also have "... = 2 ^ nat (bl_to_bin (lof_wline tw IN (get_time tw)))"
+    using `disjnt {IN} (event_of tw)`  unfolding event_of_alt_def  
+    by (smt diff_0_eq_0 disjnt_insert1 mem_Collect_eq)
+  finally show "dec_inv (fst tw + 1, snd tw)"
+    unfolding dec_inv_def by auto
+qed
+
+lemma dec_conc_hoare2:
+  "\<And>tw. dec_inv2 tw \<and> disjnt {IN} (event_of tw) \<Longrightarrow> dec_inv2 (fst tw + 1, snd tw)"
+  unfolding dec_inv2_def by auto
+
+
+lemma cases: 
+  assumes "wityping \<Gamma> (snd tw)"
+  shows "eval_world_raw2 tw (Bsig IN) = Lv Neu [False, False] \<or> eval_world_raw2 tw (Bsig IN) = Lv Neu [False, True]
+      \<or> eval_world_raw2 tw (Bsig IN) = Lv Neu [True, False] \<or> eval_world_raw2 tw (Bsig IN) = Lv Neu [True, True]"
+proof -
+  have "bexp_wt \<Gamma> (Bsig IN) (Lty Neu 2)"
+    using tyin by (metis bexp_wt.intros(3))
+  then obtain xs where *: "eval_world_raw2 tw (Bsig IN) = Lv Neu xs" and "length xs = 2"
+    using eval_world_raw_lv[OF _ assms] by blast
+  have "xs = [False, False] \<or> xs = [False, True] \<or> xs = [True, False] \<or> xs = [True, True]"
+    using \<open>length xs = 2\<close>
+  proof (induction xs)
+    case Nil
+    then show ?case by auto
+  next
+    case (Cons a xs)
+    have "a = True \<or> a = False"
+      by auto
+    hence "length xs = 1"
+      using Cons by auto
+    hence "xs = [True] \<or> xs = [False]"
+      by (metis (full_types) One_nat_def length_0_conv length_Suc_conv)
+    then show ?case
+      using \<open>a = True \<or> a = False\<close> by auto
+  qed
+  thus ?thesis
+    using * by auto
+qed
+
+lemma dec_sim:
+  "\<Gamma> \<turnstile>\<^sub>s \<lbrace>\<lambda>tw. dec_inv tw \<and> dec_inv2 tw\<rbrace> dec \<lbrace>\<lambda>tw. dec_inv tw \<and> dec_inv2 tw\<rbrace>"
+  apply (rule While_Suc)
+  apply (rule Conseq'[where P="wp3_conc \<Gamma> dec (\<lambda>tw. dec_inv  (fst tw + 1, snd tw) \<and> 
+                                                    dec_inv2 (fst tw + 1, snd tw))", rotated])
+    apply (rule wp3_conc_is_pre[OF conc_stmt_wf_dec nonneg_delay_conc_dec conc_wt_dec], simp)
+  unfolding dec_def  wp3_conc_single'[OF conc_wt_dec' nonneg_delay_conc_dec'] wp3_fun.simps
+  using case0 case1 case2 case3 cases dec_inv2_next_time dec_conc_hoare dec_conc_hoare2 one_encoding
+  by auto fastforce+
+
+text \<open>Initialisation preserves the invariant\<close>
+
+lemma nonneg_delay_dec:
+  "nonneg_delay (Bcase (Bsig IN) dec_list)"
+  by auto
+
+lemma init_sat_nand_inv_comb:
+  "init_sim2_hoare_wt \<Gamma> (\<lambda>tw. fst tw = 0) dec (\<lambda>tw. dec_inv tw \<and> dec_inv2 tw)"
+  unfolding dec_def
+  apply (rule AssignI_suc, rule SingleI)
+  apply (rule Conseq3[where Q="\<lambda>tw. dec_inv (fst tw + 1, snd tw) \<and> dec_inv2 (fst tw + 1, snd tw)", rotated])
+  apply (rule wp3_fun_is_pre[OF seq_wt_dec nonneg_delay_dec], simp)
+  unfolding wp3_fun.simps using one_encoding  case0 case1 case2 case3 cases dec_inv2_next_time
+  by auto fastforce+
+
+lemma nand_correctness:
+  assumes "sim_fin2 w (i + 1) dec tw'" and "wityping \<Gamma> w"
+  shows   "bl_to_bin (lof_wline tw' OUT (i + 1)) = 2 ^ nat (bl_to_bin (lof_wline tw' IN i))"
+  using grand_correctness[OF assms conc_stmt_wf_dec conc_wt_dec nonneg_delay_conc_dec dec_sim init_sat_nand_inv_comb]
+  unfolding dec_inv_def  by (metis (no_types, lifting) add_diff_cancel_right' assms(1)
+  sim_fin2.cases world_maxtime_lt_fst_tres)
+
+end
