Multiplexer_Hoare_Typed.thy
@@ -1,0 +1,199 @@
+(*
+ * Copyright 2019, NTU
+ *
+ * This software may be distributed and modified according to the terms of
+ * the BSD 2-Clause license. Note that NO WARRANTY is provided.
+ * See "LICENSE_BSD2.txt" for details.
+ *
+ *  Author: Albert Rizaldi, NTU Singapore
+ *)
+
+theory Multiplexer_Hoare_Typed
+  imports VHDL_Hoare_Typed
+begin
+
+text \<open>Define the new datatype for the all signals occurred in a multiplexer. A multiplexer has three
+inputs: in0, in1, and a selector.\<close>
+
+datatype sig = IN0 | IN1 | SEL | OUT
+
+\<comment> \<open>We put suffix 2 because it only selects between two inputs\<close>
+definition mux2 :: "sig conc_stmt" where
+  "mux2 = process {IN0, IN1, SEL} : Bguarded (Bsig SEL)
+                                      (Bassign_trans OUT (Bsig IN1) 1)
+                                      (Bassign_trans OUT (Bsig IN0) 1)"
+
+lemma potential_tyenv:
+  assumes "seq_wt \<Gamma> (Bguarded (Bsig SEL)
+                                      (Bassign_trans OUT (Bsig IN1) 1)
+                                      (Bassign_trans OUT (Bsig IN0) 1))"
+  shows "\<exists>ki len. \<Gamma> IN0 = Bty \<and> \<Gamma> IN1 = Bty \<and> \<Gamma> SEL = Bty \<and> \<Gamma> OUT = Bty
+             \<or> \<Gamma> IN0 = Lty ki len \<and> \<Gamma> IN1 = Lty ki len \<and> \<Gamma> SEL = Bty \<and> \<Gamma> OUT = Lty ki len"
+proof  (rule seq_wt_cases(3)[OF assms])
+  assume "bexp_wt \<Gamma> (Bsig SEL) Bty"
+  assume "seq_wt \<Gamma> (Bassign_trans OUT (Bsig IN1) 1)"
+  assume "seq_wt \<Gamma> (Bassign_trans OUT (Bsig IN0) 1)"
+  have "\<Gamma> SEL = Bty"
+    by (rule bexp_wt_cases_all[OF \<open>bexp_wt \<Gamma> (Bsig SEL) Bty\<close>]) auto
+  have " bexp_wt \<Gamma> (Bsig IN1) (\<Gamma> OUT)"
+    using seq_wt_cases(4)[OF \<open>seq_wt \<Gamma> (Bassign_trans OUT (Bsig IN1) 1)\<close>] by auto
+  hence "\<Gamma> IN1 = \<Gamma> OUT"
+    by (rule bexp_wt_cases_all) auto
+  have "bexp_wt \<Gamma> (Bsig IN0) (\<Gamma> OUT)"
+    using seq_wt_cases(4)[OF \<open>seq_wt \<Gamma> (Bassign_trans OUT (Bsig IN0) 1)\<close>] by auto
+  hence "\<Gamma> IN0 = \<Gamma> OUT"
+    by (rule bexp_wt_cases_all) auto
+  obtain ki len where "\<Gamma> OUT = Bty \<or> \<Gamma> OUT = Lty ki len"
+    using ty.exhaust by meson
+  moreover
+  { assume "\<Gamma> OUT = Bty"
+    hence "\<Gamma> IN0 = Bty"
+      by (simp add: \<open>\<Gamma> IN0 = \<Gamma> OUT\<close>)
+    moreover have "\<Gamma> IN1 = Bty"
+      using \<open>\<Gamma> IN1 = \<Gamma> OUT\<close> \<open>\<Gamma> OUT = Bty\<close> by auto
+    ultimately have ?thesis
+      using \<open>\<Gamma> OUT = Bty\<close> \<open>\<Gamma> SEL = Bty\<close> by blast }
+  moreover
+  { assume "\<Gamma> OUT = Lty ki len"
+    moreover hence "\<Gamma> IN0 = Lty ki len" and "\<Gamma> IN1 = Lty ki len"
+      using \<open>\<Gamma> IN0 = \<Gamma> OUT\<close> \<open>\<Gamma> IN1 = \<Gamma> OUT\<close> by auto
+    ultimately have ?thesis
+      using \<open>\<Gamma> SEL = Bty\<close> by blast }
+  ultimately show ?thesis
+    by auto
+qed
+
+abbreviation "bval_of_wline tw sig t \<equiv> bval_of (wline_of tw sig t)"
+
+locale multiplexer_typed = 
+  fixes \<Gamma> :: "sig tyenv" and len :: nat and ki :: "signedness"
+  assumes tyin0: "\<Gamma> IN0 = Lty ki len" and tyin1: "\<Gamma> IN1 = Lty ki len " and tysel: " \<Gamma> SEL = Bty" and tyout: "\<Gamma> OUT = Lty ki len"  
+begin
+
+definition inv :: "sig assn2" where
+  "inv \<equiv> \<lambda>tw. (wline_of tw OUT (fst tw) = (if bval_of_wline tw SEL (fst tw - 1) then wline_of tw IN1 (fst tw - 1) else wline_of tw IN0 (fst tw - 1)))"
+
+definition inv2 :: "sig assn2" where
+  "inv2 \<equiv> (\<lambda>tw. disjnt {IN0, IN1, SEL} (event_of tw) \<longrightarrow> (\<forall>i > fst tw. wline_of tw OUT i = wline_of tw OUT (fst tw)))"
+
+lemma inv_next_time_true:
+  fixes tw
+  defines "v \<equiv> eval_world_raw2 tw (Bsig IN1)"
+  assumes "eval_world_raw2 tw (Bsig SEL) = Bv True"
+  defines "tw' \<equiv> tw[OUT, 1 :=\<^sub>2 v]"
+  shows   "inv (fst tw' + 1, snd tw')"
+proof - 
+  have bexpIN1: "bexp_wt \<Gamma> (Bsig SEL) (Bty)" 
+    using multiplexer_typed_axioms unfolding multiplexer_typed_def by (metis bexp_wt.intros(3))+
+  have "wline_of tw' OUT (fst tw + 1) = v"
+    unfolding tw'_def worldline_upd2_def worldline_upd_def by auto
+  also have "... = (if bval_of_wline tw SEL (fst tw) then wline_of tw IN1 (fst tw) else wline_of tw IN0 (fst tw))"
+    using assms(2) unfolding v_def eval_world_raw.simps eval_arith.simps  Let_def comp_def by auto
+  finally show ?thesis
+    unfolding inv_def tw'_def worldline_upd2_def worldline_upd_def  by auto
+qed
+
+lemma inv_next_time_false:
+  fixes tw
+  defines "v \<equiv> eval_world_raw2 tw (Bsig IN0)"
+  assumes "eval_world_raw2 tw (Bsig SEL) \<noteq> Bv True"
+  defines "tw' \<equiv> tw[OUT, 1 :=\<^sub>2 v]"
+  assumes "wityping \<Gamma> (snd tw)"
+  shows   "inv (fst tw' + 1, snd tw')"
+proof - 
+  have bexpIN1: "bexp_wt \<Gamma> (Bsig SEL) (Bty)" 
+    using multiplexer_typed_axioms unfolding multiplexer_typed_def by (metis bexp_wt.intros(3))+
+  hence "eval_world_raw2 tw (Bsig SEL) = Bv False"
+    using eval_world_raw_bv[OF bexpIN1 assms(4)] assms(2) by metis
+  have "wline_of tw' OUT (fst tw + 1) = v"
+    unfolding tw'_def worldline_upd2_def worldline_upd_def by auto
+  also have "... = (if bval_of_wline tw SEL (fst tw) then wline_of tw IN1 (fst tw) else wline_of tw IN0 (fst tw))"
+    using `eval_world_raw2 tw (Bsig SEL) = Bv False` unfolding v_def eval_world_raw.simps eval_arith.simps  Let_def comp_def by auto
+  finally show ?thesis
+    unfolding inv_def tw'_def worldline_upd2_def worldline_upd_def  by auto
+qed
+
+lemma inv2_next_time:
+  fixes tw v
+  defines "tw' \<equiv> tw[OUT, 1 :=\<^sub>2 v]"
+  shows   "inv2 (fst tw' + 1, snd tw')"
+  unfolding inv2_def tw'_def worldline_upd2_def worldline_upd_def by auto
+
+lemma mult_conc_hoare:
+  "\<And>tw. inv tw \<and> inv2 tw \<and> disjnt {IN0, IN1, SEL} (event_of tw) \<Longrightarrow> inv (fst tw + 1, snd tw)"
+proof -
+  fix tw
+  assume "inv tw \<and> inv2 tw \<and> disjnt {IN0, IN1, SEL} (event_of tw)"
+  hence "inv tw" and "inv2 tw" and "disjnt {IN0, IN1, SEL} (event_of tw)"
+    by auto
+  have "wline_of tw OUT (fst tw + 1) = wline_of tw OUT (fst tw)"
+    using `inv2 tw` `disjnt {IN0, IN1, SEL} (event_of tw)` unfolding inv2_def by auto 
+  also have "... = (if bval_of_wline tw SEL (get_time tw - 1) then wline_of tw IN1 (get_time tw - 1) else wline_of tw IN0 (get_time tw - 1))"
+    using `inv tw` unfolding inv_def by auto
+  also have "... = (if bval_of_wline tw SEL (fst tw) then wline_of tw IN1 (fst tw) else wline_of tw IN0 (fst tw))"
+    using `disjnt {IN0, IN1, SEL} (event_of tw)`  unfolding event_of_alt_def  
+    by (smt diff_0_eq_0 disjnt_insert1 mem_Collect_eq)
+  finally show "inv (fst tw + 1, snd tw)"
+    unfolding inv_def by auto
+qed
+
+lemma mult_conc_hoare2:
+  "\<And>tw. inv2 tw \<and> disjnt {IN0, IN1, SEL} (event_of tw) \<Longrightarrow> inv2 (fst tw + 1, snd tw)"
+  unfolding inv2_def by auto
+
+lemma conc_stmt_wf_mult:
+  "conc_stmt_wf mux2"
+  unfolding mux2_def conc_stmt_wf_def by auto  
+
+lemma nonneg_delay_conc_mult:
+  "nonneg_delay_conc mux2"
+  unfolding mux2_def by auto
+
+lemma nonneg_delay_conc_mult':
+  "nonneg_delay_conc ( process {IN0, IN1, SEL} : Bguarded (Bsig SEL) (Bassign_trans OUT (Bsig IN1) 1) (Bassign_trans OUT (Bsig IN0) 1))"
+  using nonneg_delay_conc_mult unfolding mux2_def by auto
+
+lemma well_typed:
+  "seq_wt \<Gamma> (Bguarded (Bsig SEL) (Bassign_trans OUT (Bsig IN1) 1) (Bassign_trans OUT (Bsig IN0) 1))"
+  by (metis bexp_wt.intros(3) seq_wt.intros(3) seq_wt.intros(4) tyin0 tyin1 tyout tysel)
+
+lemma conc_wt_mult:
+  "conc_wt \<Gamma> mux2"
+  unfolding mux2_def by (meson conc_wt.intros(1) well_typed)
+
+lemma conc_wt_mult':
+  "conc_wt \<Gamma> ( process {IN0, IN1, SEL} : Bguarded (Bsig SEL) (Bassign_trans OUT (Bsig IN1) 1) (Bassign_trans OUT (Bsig IN0) 1))"
+  using conc_wt_mult unfolding mux2_def by auto
+
+lemma mult_conc_sim2':
+  "\<Gamma> \<turnstile>\<^sub>s \<lbrace>\<lambda>tw. inv tw \<and> inv2 tw\<rbrace> mux2 \<lbrace>\<lambda>tw. inv tw \<and> inv2 tw\<rbrace>"
+  apply (rule While_Suc)
+  apply (rule Conseq'[where P="wp3_conc \<Gamma> mux2 (\<lambda>tw. inv  (fst tw + 1, snd tw) \<and> 
+                                                     inv2 (fst tw + 1, snd tw))", rotated])
+  apply (rule wp3_conc_is_pre, rule conc_stmt_wf_mult, rule nonneg_delay_conc_mult, rule conc_wt_mult, simp)
+  unfolding mux2_def  wp3_conc_single'[OF conc_wt_mult' nonneg_delay_conc_mult'] wp3_fun.simps  
+  using inv_next_time_true inv_next_time_false inv2_next_time mult_conc_hoare mult_conc_hoare2 by presburger
+
+text \<open>Initialisation preserves the invariant\<close>
+
+lemma nonneg_delay_mult:
+  "nonneg_delay ( Bguarded (Bsig SEL) (Bassign_trans OUT (Bsig IN1) 1) (Bassign_trans OUT (Bsig IN0) 1))"
+  using nonneg_delay_conc_mult' by auto
+
+lemma init_sat_nand_inv_comb:
+  "init_sim2_hoare_wt \<Gamma> (\<lambda>tw. fst tw = 0) mux2 (\<lambda>tw. inv tw \<and> inv2 tw)"
+  unfolding mux2_def
+  apply (rule AssignI_suc, rule SingleI)
+  apply (rule Conseq3[where Q="\<lambda>tw. inv (fst tw + 1, snd tw) \<and> inv2 (fst tw + 1, snd tw)", rotated])
+  apply (rule wp3_fun_is_pre[OF well_typed nonneg_delay_mult], simp)
+  unfolding wp3_fun.simps using inv_next_time_true inv_next_time_false inv2_next_time by auto
+
+lemma correctness:
+  assumes "sim_fin2 w (i + 1) mux2 tw'" and "wityping \<Gamma> w"
+  shows "wline_of tw' OUT (i + 1) = (if bval_of_wline tw' SEL (i) then wline_of tw' IN1 (i) else wline_of tw' IN0 (i))"
+  using grand_correctness[OF assms conc_stmt_wf_mult conc_wt_mult nonneg_delay_conc_mult mult_conc_sim2' init_sat_nand_inv_comb]
+  unfolding mux2_def inv_def by (metis (no_types, lifting) add_diff_cancel_right' assms(1)
+  sim_fin2.cases world_maxtime_lt_fst_tres)
+end
+
+end
