NAND_Hoare_Typed.thy
@@ -1,0 +1,138 @@
+(*
+ * Copyright 2019, NTU
+ *
+ * This software may be distributed and modified according to the terms of
+ * the BSD 2-Clause license. Note that NO WARRANTY is provided.
+ * See "LICENSE_BSD2.txt" for details.
+ *
+ *  Author: Albert Rizaldi, NTU Singapore
+ *)
+
+theory NAND_Hoare_Typed
+  imports VHDL_Hoare_Typed NAND_Femto
+begin
+
+subsection \<open>Proving @{term "nand3"}: NAND with transport delay \<close>
+
+abbreviation "bval_of_wline tw sig n \<equiv> bval_of (wline_of tw sig n)"
+abbreviation "lof_wline tw sig n \<equiv> lval_of (wline_of tw sig n)"
+
+locale scalar_type_nand3 =
+  fixes \<Gamma> :: "sig tyenv"
+  assumes "\<Gamma> A = Bty" and "\<Gamma> B = Bty" and "\<Gamma> C = Bty"
+begin
+
+text \<open>Invariant for NAND: at all times @{term "i"}, the signal @{term "C :: sig"} at @{term "i"} 
+should be the NAND value of @{term "A :: sig"} and @{term "B :: sig"} at time @{term "i - 1"}.\<close>
+
+definition nand_inv :: "sig assn2" where
+  "nand_inv \<equiv> (\<lambda>tw. bval_of_wline tw C (fst tw) \<longleftrightarrow> \<not> (bval_of_wline tw A (fst tw - 1) \<and> bval_of_wline tw B (fst tw - 1)))"
+
+definition nand_inv2 :: "sig assn2" where
+  "nand_inv2 \<equiv> (\<lambda>tw. disjnt {A, B} (event_of tw) \<longrightarrow> (\<forall>i > fst tw. bval_of_wline tw C i \<longleftrightarrow> bval_of_wline tw C (fst tw)))"
+
+lemma nand_inv_next_time:
+  fixes tw
+  defines "v \<equiv> eval_world_raw2 tw (Bnand (Bsig A) (Bsig B))"
+  defines "tw' \<equiv> tw[C, 1 :=\<^sub>2 v]"
+  assumes "wityping \<Gamma> (snd tw)"
+  shows   "nand_inv (fst tw' + 1, snd tw')"
+proof -
+  have bexpA: "bexp_wt \<Gamma> (Bsig A) Bty" and bexpB: "bexp_wt \<Gamma> (Bsig B) Bty" 
+    using scalar_type_nand3_axioms unfolding scalar_type_nand3_def  by (metis bexp_wt.intros(3))+
+  have "bval_of_wline tw' C (fst tw + 1) \<longleftrightarrow> bval_of v"
+    unfolding tw'_def worldline_upd2_def worldline_upd_def by auto
+  also have "... \<longleftrightarrow> \<not> (bval_of_wline tw A (fst tw) \<and> bval_of_wline tw B (fst tw))"
+    using eval_world_raw_bv[OF bexpA `wityping \<Gamma> (snd tw)`]  eval_world_raw_bv[OF bexpB `wityping \<Gamma> (snd tw)`] 
+    unfolding v_def by (auto split:val.split)(metis val.distinct(1))+
+  finally show ?thesis
+    unfolding nand_inv_def  
+    by (metis (no_types, lifting) add_diff_cancel_right' comp_apply fst_conv less_add_one snd_conv
+    tw'_def worldline_upd2_before_dly worldline_upd2_def)
+qed
+
+lemma nand_inv2_next_time:
+  fixes tw
+  defines "v \<equiv> eval_world_raw2 tw (Bnand (Bsig A) (Bsig B))" 
+  defines "tw' \<equiv> tw[C, 1 :=\<^sub>2 v]"
+  shows   "nand_inv2 (fst tw' + 1, snd tw')"
+  using assms unfolding nand_inv2_def tw'_def worldline_upd2_def worldline_upd_def by auto 
+ 
+lemma pre_nand_conc_hoare':
+  "\<And>tw. nand_inv tw \<and> nand_inv2 tw \<and> disjnt {A, B} (event_of tw) \<Longrightarrow> nand_inv (fst tw + 1, snd tw)"
+proof -
+  fix tw
+  assume "nand_inv tw \<and> nand_inv2 tw \<and> disjnt {A, B} (event_of tw)"
+  hence "nand_inv tw" and "nand_inv2 tw" and "disjnt {A, B} (event_of tw)"
+    by auto
+  have "bval_of_wline tw C (fst tw + 1) \<longleftrightarrow> bval_of_wline tw C (fst tw)"
+    using `nand_inv2 tw` `disjnt {A, B} (event_of tw)` unfolding nand_inv2_def 
+    by (simp add: next_time_world_at_least) 
+  also have "... \<longleftrightarrow> \<not> (bval_of_wline tw A (fst tw - 1) \<and> bval_of_wline tw B (fst tw - 1))"
+    using `nand_inv tw` unfolding nand_inv_def by auto
+  also have "... \<longleftrightarrow> \<not> (bval_of_wline tw A (fst tw) \<and> bval_of_wline tw B (fst tw))"
+    using `disjnt {A, B} (event_of tw)`  unfolding event_of_alt_def   
+    by (smt diff_0_eq_0 disjnt_insert1 mem_Collect_eq)
+  finally show "nand_inv (fst tw + 1, snd tw)"
+    unfolding nand_inv_def by auto
+qed
+
+lemma nand_conc_hoare2:
+  "\<And>tw. nand_inv2 tw \<and> disjnt {A, B} (event_of tw) \<Longrightarrow> nand_inv2 (fst tw + 1, snd tw)"
+  unfolding nand_inv2_def by auto
+
+lemma conc_stmt_wf_nand3:
+  "conc_stmt_wf nand3"
+  unfolding nand3_def conc_stmt_wf_def by auto  
+
+lemma nonneg_delay_conc_nand3:
+  "nonneg_delay_conc nand3"
+  unfolding nand3_def by auto
+
+lemma nonneg_delay_conc_nand3':
+  "nonneg_delay_conc ( process {A, B} : Bassign_trans C (Bnand (Bsig A) (Bsig B)) 1)"
+  using nonneg_delay_conc_nand3 unfolding nand3_def by auto
+
+lemma conc_wt_nand3:
+  "conc_wt \<Gamma> nand3"
+  unfolding nand3_def by (metis bexp_wt.intros(3) bexp_wt.intros(9) conc_wt.intros(1)
+  scalar_type_nand3_axioms scalar_type_nand3_def seq_wt.intros(4))
+
+lemma conc_wt_nand3':
+  "conc_wt \<Gamma> ( process {A, B} : Bassign_trans C (Bnand (Bsig A) (Bsig B)) 1)"
+  using conc_wt_nand3 unfolding nand3_def by auto
+
+lemma nand_conc_sim2':
+  "\<Gamma> \<turnstile>\<^sub>s \<lbrace>\<lambda>tw. nand_inv tw \<and> nand_inv2 tw\<rbrace> nand3 \<lbrace>\<lambda>tw. nand_inv tw \<and> nand_inv2 tw\<rbrace>"
+  apply (rule While_Suc)
+  apply (rule Conseq'[where P="wp3_conc \<Gamma> nand3 (\<lambda>tw. nand_inv  (fst tw + 1, snd tw) \<and> 
+                                                      nand_inv2 (fst tw + 1, snd tw))", rotated])
+  apply (rule wp3_conc_is_pre, rule conc_stmt_wf_nand3, rule nonneg_delay_conc_nand3, rule conc_wt_nand3, simp)
+  unfolding nand3_def  wp3_conc_single'[OF conc_wt_nand3' nonneg_delay_conc_nand3'] wp3_fun.simps
+  using nand_conc_hoare2 nand_inv2_next_time nand_inv_next_time pre_nand_conc_hoare' by presburger
+
+text \<open>Initialisation preserves the invariant\<close>
+
+lemma seq_wt_nand3':
+  "seq_wt \<Gamma> (Bassign_trans C (Bnand (Bsig A) (Bsig B)) 1)"
+  using conc_wt_nand3' by auto
+
+lemma nonneg_delay_nand3:
+  " nonneg_delay (Bassign_trans C (Bnand (Bsig A) (Bsig B)) 1)"
+  using nonneg_delay_conc_nand3' by auto
+
+lemma init_sat_nand_inv_comb:
+  "init_sim2_hoare_wt \<Gamma> (\<lambda>tw. fst tw = 0) nand3 (\<lambda>tw. nand_inv tw \<and> nand_inv2 tw)"
+  unfolding nand3_def
+  apply (rule AssignI_suc, rule SingleI)
+  apply (rule Conseq3[where Q="\<lambda>tw. nand_inv (fst tw + 1, snd tw) \<and> nand_inv2 (fst tw + 1, snd tw)", rotated])
+  apply (rule wp3_fun_is_pre[OF seq_wt_nand3' nonneg_delay_nand3], simp)
+  unfolding wp3_fun.simps using nand_inv_next_time nand_inv2_next_time by blast
+
+lemma nand_correctness:
+  assumes "sim_fin2 w (i + 1) nand3 tw'" and "wityping \<Gamma> w"
+  shows "bval_of_wline tw' C (i + 1) \<longleftrightarrow> \<not> (bval_of_wline tw' A i \<and> bval_of_wline tw' B i)"
+  using grand_correctness[OF assms conc_stmt_wf_nand3 conc_wt_nand3 nonneg_delay_conc_nand3 nand_conc_sim2' init_sat_nand_inv_comb]
+  unfolding nand_inv_def by (metis (no_types, lifting) add_diff_cancel_right' assms(1) sim_fin2.cases world_maxtime_lt_fst_tres)
+
+end
