Shift_Right_Hoare_Pos_Typed.thy
@@ -1,0 +1,145 @@
+(*
+ * Copyright 2019, NTU
+ *
+ * This software may be distributed and modified according to the terms of
+ * the BSD 2-Clause license. Note that NO WARRANTY is provided.
+ * See "LICENSE_BSD2.txt" for details.
+ *
+ *  Author: Albert Rizaldi, NTU Singapore
+ *)
+
+theory Shift_Right_Hoare_Pos_Typed
+  imports VHDL_Hoare_Typed Bits_Int_Aux
+begin
+
+datatype sig = IN | OUT
+
+definition shiftr :: "nat \<Rightarrow> sig conc_stmt" where
+  "shiftr n \<equiv> process {IN} : Bassign_trans OUT (Bshiftr (Bsig IN) n) 1"
+
+lemma potential_tyenv:
+  assumes "seq_wt \<Gamma> (Bassign_trans OUT (Bshiftr (Bsig IN) n) 1)"
+  shows "\<exists>len>0. \<Gamma> IN = Lty Uns len \<and> \<Gamma> OUT = Lty Uns len \<or> \<Gamma> IN = Lty Sig len \<and> \<Gamma> OUT = Lty Sig len"
+  by (rule seq_wt_cases(4)[OF assms])
+     (metis bexp_wt_cases(15) bexp_wt_cases(9))
+
+locale unsigned_shift_right =
+  fixes \<Gamma> :: "sig tyenv"
+  fixes len :: nat
+  fixes amount :: nat
+  assumes "0 < len"
+  assumes "\<Gamma> IN = Lty Uns len \<and> \<Gamma> OUT = Lty Uns len"
+begin
+
+lemma well_typed:
+  "seq_wt \<Gamma> (Bassign_trans OUT (Bshiftr (Bsig IN) n) 1)"
+  by (rule seq_wt.intros(4))
+     (metis (full_types) bexp_wt.intros(23) bexp_wt.intros(3) unsigned_shift_right_axioms
+     unsigned_shift_right_def)
+
+abbreviation "lof_wline tw sig n \<equiv> lval_of (wline_of tw sig n)"
+
+definition inv :: "sig assn2" where
+  "inv tw \<equiv> (lof_wline tw OUT (fst tw) = take len (replicate amount False @ lof_wline tw IN (fst tw - 1)))"
+
+definition inv2 :: "sig assn2" where
+  "inv2 tw \<equiv> (disjnt {IN} (event_of tw) \<longrightarrow> (\<forall>i > fst tw. lof_wline tw OUT i = lof_wline tw OUT (fst tw)))"
+
+lemma inv_next_time:
+  fixes tw
+  defines "v \<equiv> eval_world_raw2 tw (Bshiftr (Bsig IN) amount)"
+  defines "tw' \<equiv> tw[OUT, 1 :=\<^sub>2 v]"
+  assumes "wityping \<Gamma> (snd tw)"
+  shows   "inv (fst tw' + 1, snd tw')"
+proof - 
+  have bexpIN: "bexp_wt \<Gamma> (Bsig IN) (Lty Uns len)" 
+    using unsigned_shift_right_axioms unfolding unsigned_shift_right_def by (metis bexp_wt.intros(3))+
+  obtain bsIN where evalIN: "eval_world_raw (fst tw) (snd tw) (Bsig IN) = Lv Uns bsIN" and" length bsIN = len "
+      using eval_world_raw_lv[OF bexpIN `wityping \<Gamma> (snd tw)`] by blast
+  have "lof_wline tw' OUT (fst tw + 1) = lval_of v"
+    unfolding tw'_def worldline_upd2_def worldline_upd_def by auto
+  also have "... = take len (replicate amount False   @ lof_wline tw IN (fst tw))"
+    using evalIN `length bsIN = len` unfolding v_def eval_world_raw.simps eval_arith.simps Let_def by auto
+  finally show ?thesis
+    unfolding inv_def tw'_def worldline_upd2_def worldline_upd_def  by auto
+qed
+
+lemma inv2_next_time:
+  fixes tw v
+  defines "tw' \<equiv> tw[OUT, 1 :=\<^sub>2 v]"
+  shows   "inv2 (fst tw' + 1, snd tw')"
+  unfolding inv2_def tw'_def worldline_upd2_def worldline_upd_def by auto
+
+lemma conc_hoare:
+  "\<And>tw. inv tw \<and> inv2 tw \<and> disjnt {IN} (event_of tw) \<Longrightarrow> inv (fst tw + 1, snd tw)"
+proof -
+  fix tw
+  assume "inv tw \<and> inv2 tw \<and> disjnt {IN} (event_of tw)"
+  hence "inv tw" and "inv2 tw" and "disjnt {IN} (event_of tw)"
+    by auto
+  have "lof_wline tw OUT (fst tw + 1) = lof_wline tw OUT (fst tw)"
+    using `inv2 tw` `disjnt {IN} (event_of tw)` unfolding inv2_def by auto 
+  also have "... = take len (replicate amount False @ lval_of (wline_of tw IN (get_time tw - 1)))"
+    using `inv tw` unfolding inv_def by auto
+  also have "... = take len (replicate amount False @ lval_of (wline_of tw IN (get_time tw)))"
+    using `disjnt {IN} (event_of tw)`  unfolding event_of_alt_def   by (smt diff_0_eq_0 disjnt_insert1 mem_Collect_eq)
+  finally show "inv (fst tw + 1, snd tw)"
+    unfolding inv_def by auto
+qed
+
+lemma conc_hoare2:
+  "\<And>tw. inv2 tw \<and> disjnt {IN} (event_of tw) \<Longrightarrow> inv2 (fst tw + 1, snd tw)"
+  unfolding inv2_def by auto
+
+lemma conc_stmt_wf:
+  "conc_stmt_wf (shiftr amount)"
+  unfolding shiftr_def conc_stmt_wf_def by auto  
+
+lemma nonneg_delay_conc:
+  "nonneg_delay_conc (shiftr amount)"
+  unfolding shiftr_def by auto
+
+lemma nonneg_delay_conc':
+  "nonneg_delay_conc ( process {IN} : Bassign_trans OUT (Bshiftr (Bsig IN) amount) 1)"
+  using nonneg_delay_conc unfolding shiftr_def by auto
+
+lemma conc_wt:
+  "conc_wt \<Gamma> (shiftr amount)"
+  unfolding shiftr_def  by (meson conc_wt.intros(1) well_typed)
+
+lemma conc_wt':
+  "conc_wt \<Gamma> ( process {IN} : Bassign_trans OUT (Bshiftr (Bsig IN) amount) 1)"
+  using conc_wt unfolding shiftr_def by auto
+
+lemma conc_sim2':
+  "\<Gamma> \<turnstile>\<^sub>s \<lbrace>\<lambda>tw. inv tw \<and> inv2 tw\<rbrace> shiftr amount \<lbrace>\<lambda>tw. inv tw \<and> inv2 tw\<rbrace>"
+  apply (rule While_Suc)
+  apply (rule Conseq'[where P="wp3_conc \<Gamma> (shiftr amount) (\<lambda>tw. inv  (fst tw + 1, snd tw) \<and> 
+                                                              inv2 (fst tw + 1, snd tw))", rotated])
+  apply (rule wp3_conc_is_pre, rule conc_stmt_wf, rule nonneg_delay_conc, rule conc_wt, simp)
+  unfolding shiftr_def wp3_conc_single'[OF conc_wt' nonneg_delay_conc'] wp3_fun.simps
+  using inv_next_time inv2_next_time conc_hoare conc_hoare2 by presburger
+
+lemma nonneg_delay_add:
+  " nonneg_delay (Bassign_trans OUT (Bshiftr (Bsig IN) amount) 1)"
+  using nonneg_delay_conc' by auto
+
+lemma init_sat_nand_inv_comb:
+  "init_sim2_hoare_wt \<Gamma> (\<lambda>tw. fst tw = 0) (shiftr amount) (\<lambda>tw. inv tw \<and> inv2 tw)"
+  unfolding shiftr_def
+  apply (rule AssignI_suc, rule SingleI)
+  apply (rule Conseq3[where Q="\<lambda>tw. inv (fst tw + 1, snd tw) \<and> inv2 (fst tw + 1, snd tw)", rotated])
+  apply (rule wp3_fun_is_pre[OF well_typed nonneg_delay_add], simp)
+  unfolding wp3_fun.simps using inv_next_time inv2_next_time by blast
+
+lemma correctness:
+  assumes "sim_fin2 w (i + 1) (shiftr amount) tw'" and "wityping \<Gamma> w"
+  shows "lof_wline tw' OUT (i + 1) = take len (replicate amount False @ lof_wline tw' IN (i))"
+  using grand_correctness[OF assms conc_stmt_wf conc_wt nonneg_delay_conc conc_sim2' init_sat_nand_inv_comb]
+  unfolding shiftr_def inv_def  by (metis (no_types, lifting) add_diff_cancel_right' assms(1)
+  sim_fin2.cases world_maxtime_lt_fst_tres)
+
+end
+
+end
+
