Signed_Mult_Typed.thy
@@ -1,0 +1,163 @@
+(*
+ * Copyright 2019, NTU
+ *
+ * This software may be distributed and modified according to the terms of
+ * the BSD 2-Clause license. Note that NO WARRANTY is provided.
+ * See "LICENSE_BSD2.txt" for details.
+ *
+ *  Author: Albert Rizaldi, NTU Singapore
+ *)
+
+theory Signed_Mult_Typed
+  imports VHDL_Hoare_Typed Bits_Int_Aux
+begin
+
+datatype sig = A | B | C
+
+definition mult :: "sig conc_stmt" where
+  "mult \<equiv> process {A, B} : Bassign_trans C (Bmult (Bsig A) (Bsig B)) 1"
+
+lemma potential_tyenv:
+  assumes "seq_wt \<Gamma> (Bassign_trans C (Bmult (Bsig A) (Bsig B)) 1)"
+  shows "\<exists>len1>0. \<exists>len2>0. \<Gamma> A = Lty Uns len1 \<and> \<Gamma> B = Lty Uns len2 \<and> \<Gamma> C = Lty Uns (len1 + len2)
+                   \<or> \<Gamma> A = Lty Sig len1 \<and> \<Gamma> B = Lty Sig len2 \<and> \<Gamma> C = Lty Sig (len1 + len2)"
+proof (rule seq_wt_cases(4)[OF assms])
+  assume "bexp_wt \<Gamma> (Bmult (Bsig A) (Bsig B)) (\<Gamma> C)"
+  obtain len1 len2 where " \<Gamma> A = Lty Uns len1 \<and> \<Gamma> B = Lty Uns len2 \<and> \<Gamma> C = Lty Uns (len1 + len2)
+                              \<or> \<Gamma> A = Lty Sig len1 \<and> \<Gamma> B = Lty Sig len2 \<and> \<Gamma> C = Lty Sig (len1 + len2)"
+    and "0 < len1" and "0 < len2"
+    by (rule bexp_wt_cases(12)[OF \<open>bexp_wt \<Gamma> (Bmult (Bsig A) (Bsig B)) (\<Gamma> C)\<close>])
+       (metis bexp_wt_cases(9))+
+  thus ?thesis
+    by auto
+qed
+
+locale signed_multiplication =
+  fixes \<Gamma> :: "sig tyenv"
+  fixes len len1 len2 :: nat
+  assumes len_def: "len = len1 + len2"
+  assumes atype: "\<Gamma> A = Lty Sig len1" and btype: "\<Gamma> B = Lty Sig len2" and ctype: "\<Gamma> C = Lty Sig len"
+  assumes len1: "0 < len1" and len2: "0 < len2"
+begin
+
+lemma well_typed:
+  "seq_wt \<Gamma> (Bassign_trans C (Bmult (Bsig A) (Bsig B)) 1)"
+  apply (rule seq_wt.intros(4))
+  unfolding ctype len_def apply (rule bexp_wt.intros(18))
+  unfolding atype[THEN sym] btype[THEN sym] apply (rule bexp_wt.intros(3))+
+  using len1 len2 by auto
+
+abbreviation "lof_wline tw sig n \<equiv> lval_of (wline_of tw sig n)"
+
+definition inv :: "sig assn2" where
+  "inv tw \<equiv> (lof_wline tw C (fst tw) =
+                  bin_to_bl len (sbl_to_bin (lof_wline tw A (fst tw - 1)) * sbl_to_bin (lof_wline tw B (fst tw - 1))))"
+
+definition inv2 :: "sig assn2" where
+  "inv2 tw \<equiv> (disjnt {A, B} (event_of tw) \<longrightarrow> (\<forall>i > fst tw. lof_wline tw C i = lof_wline tw C (fst tw)))"
+
+lemma inv_next_time:
+  fixes tw
+  defines "v \<equiv> eval_world_raw2 tw (Bmult (Bsig A) (Bsig B))"
+  defines "tw' \<equiv> tw[C, 1 :=\<^sub>2 v]"
+  assumes "wityping \<Gamma> (snd tw)"
+  shows   "inv (fst tw' + 1, snd tw')"
+proof - 
+  have bexpA: "bexp_wt \<Gamma> (Bsig A) (Lty Sig len1)" and bexpB: "bexp_wt \<Gamma> (Bsig B) (Lty Sig len2)"
+    using signed_multiplication_axioms unfolding signed_multiplication_def by (metis bexp_wt.intros(3))+
+  obtain bsA bsB where evalA: "eval_world_raw (fst tw) (snd tw) (Bsig A) = Lv Sig bsA" and" length bsA = len1 " and
+                       evalB: "eval_world_raw (fst tw) (snd tw) (Bsig B) = Lv Sig bsB" and" length bsB = len2 "
+      using eval_world_raw_lv[OF bexpA `wityping \<Gamma> (snd tw)`] eval_world_raw_lv[OF bexpB `wityping \<Gamma> (snd tw)`] by blast
+  have "lof_wline tw' C (fst tw + 1) = lval_of v"
+    unfolding tw'_def worldline_upd2_def worldline_upd_def by auto
+  also have "... = bin_to_bl len (sbl_to_bin (lof_wline tw A (fst tw)) * sbl_to_bin (lof_wline tw B (fst tw)))"
+    using evalA evalB `length bsA = len1` `length bsB = len2`
+    unfolding v_def eval_world_raw.simps eval_arith.simps len_def Let_def by auto
+  finally show ?thesis
+    unfolding inv_def tw'_def worldline_upd2_def worldline_upd_def  by auto
+qed
+
+lemma inv2_next_time:
+  fixes tw v
+  defines "tw' \<equiv> tw[C, 1 :=\<^sub>2 v]"
+  shows   "inv2 (fst tw' + 1, snd tw')"
+  unfolding inv2_def tw'_def worldline_upd2_def worldline_upd_def by auto
+
+lemma mult_conc_hoare:
+  "\<And>tw. inv tw \<and> inv2 tw \<and> disjnt {A, B} (event_of tw) \<Longrightarrow> inv (fst tw + 1, snd tw)"
+proof -
+  fix tw
+  assume "inv tw \<and> inv2 tw \<and> disjnt {A, B} (event_of tw)"
+  hence "inv tw" and "inv2 tw" and "disjnt {A, B} (event_of tw)"
+    by auto
+  have "lof_wline tw C (fst tw + 1) = lof_wline tw C (fst tw)"
+    using `inv2 tw` `disjnt {A, B} (event_of tw)` unfolding inv2_def by auto 
+  also have "... = bin_to_bl len (sbl_to_bin (lval_of (wline_of tw A (get_time tw - 1))) * sbl_to_bin (lval_of (wline_of tw B (get_time tw - 1))))"
+    using `inv tw` unfolding inv_def by auto
+  also have "... = bin_to_bl len (sbl_to_bin (lval_of (wline_of tw A (fst tw))) * sbl_to_bin (lval_of (wline_of tw B (fst tw))))"
+    using `disjnt {A, B} (event_of tw)`  unfolding event_of_alt_def  
+    by (smt diff_0_eq_0 disjnt_insert1 mem_Collect_eq)
+  finally show "inv (fst tw + 1, snd tw)"
+    unfolding inv_def by auto
+qed
+
+lemma mult_conc_hoare2:
+  "\<And>tw. inv2 tw \<and> disjnt {A, B} (event_of tw) \<Longrightarrow> inv2 (fst tw + 1, snd tw)"
+  unfolding inv2_def by auto
+
+lemma conc_stmt_wf_mult:
+  "conc_stmt_wf mult"
+  unfolding mult_def conc_stmt_wf_def by auto  
+
+lemma nonneg_delay_conc_mult:
+  "nonneg_delay_conc mult"
+  unfolding mult_def by auto
+
+lemma nonneg_delay_conc_mult':
+  "nonneg_delay_conc ( process {A, B} : Bassign_trans C (Bmult (Bsig A) (Bsig B)) 1)"
+  using nonneg_delay_conc_mult unfolding mult_def by auto
+
+lemma conc_wt_mult:
+  "conc_wt \<Gamma> mult"
+  unfolding mult_def  by (meson conc_wt.intros(1) well_typed)
+
+lemma conc_wt_mult':
+  "conc_wt \<Gamma> ( process {A, B} : Bassign_trans C (Bmult (Bsig A) (Bsig B)) 1)"
+  using conc_wt_mult unfolding mult_def by auto
+
+lemma mult_conc_sim2':
+  "\<Gamma> \<turnstile>\<^sub>s \<lbrace>\<lambda>tw. inv tw \<and> inv2 tw\<rbrace> mult \<lbrace>\<lambda>tw. inv tw \<and> inv2 tw\<rbrace>"
+  apply (rule While_Suc)
+  apply (rule Conseq'[where P="wp3_conc \<Gamma> mult (\<lambda>tw. inv  (fst tw + 1, snd tw) \<and> 
+                                                      inv2 (fst tw + 1, snd tw))", rotated])
+  apply (rule wp3_conc_is_pre, rule conc_stmt_wf_mult, rule nonneg_delay_conc_mult, rule conc_wt_mult, simp)
+  unfolding mult_def  wp3_conc_single'[OF conc_wt_mult' nonneg_delay_conc_mult'] wp3_fun.simps
+  using inv_next_time inv2_next_time mult_conc_hoare mult_conc_hoare2 by presburger
+
+text \<open>Initialisation preserves the invariant\<close>
+
+lemma nonneg_delay_mult:
+  " nonneg_delay (Bassign_trans C (Bmult (Bsig A) (Bsig B)) 1)"
+  using nonneg_delay_conc_mult' by auto
+
+lemma seq_wt:
+  "seq_wt \<Gamma> (Bassign_trans C (Bmult (Bsig A) (Bsig B)) 1)"
+  using well_typed by blast
+
+lemma init_sat_nand_inv_comb:
+  "init_sim2_hoare_wt \<Gamma> (\<lambda>tw. fst tw = 0) mult (\<lambda>tw. inv tw \<and> inv2 tw)"
+  unfolding mult_def
+  apply (rule AssignI_suc, rule SingleI)
+  apply (rule Conseq3[where Q="\<lambda>tw. inv (fst tw + 1, snd tw) \<and> inv2 (fst tw + 1, snd tw)", rotated])
+  apply (rule wp3_fun_is_pre[OF well_typed nonneg_delay_mult], simp)
+  unfolding wp3_fun.simps using inv_next_time inv2_next_time by blast
+
+lemma correctness:
+  assumes "sim_fin2 w (i + 1) mult tw'" and "wityping \<Gamma> w"
+  shows "lof_wline tw' C (i + 1) = bin_to_bl len (sbl_to_bin (lof_wline tw' A i) * sbl_to_bin (lof_wline tw' B i))"
+  using grand_correctness[OF assms conc_stmt_wf_mult conc_wt_mult nonneg_delay_conc_mult mult_conc_sim2' init_sat_nand_inv_comb]
+  unfolding mult_def inv_def by (metis (no_types, lifting) add_diff_cancel_right' assms(1)
+  sim_fin2.cases world_maxtime_lt_fst_tres)
+end
+
+end
